<?xml version="1.0"?>
<rdf:RDF xmlns="https://purl.org/ffdr-ontology#"
     xml:base="https://purl.org/ffdr-ontology"
     xmlns:owl="http://www.w3.org/2002/07/owl#"
     xmlns:rdf="http://www.w3.org/1999/02/22-rdf-syntax-ns#"
     xmlns:xml="http://www.w3.org/XML/1998/namespace"
     xmlns:xsd="http://www.w3.org/2001/XMLSchema#"
     xmlns:rdfs="http://www.w3.org/2000/01/rdf-schema#"
     xmlns:terms="http://purl.org/dc/terms/"
     xmlns:ffdr-ontology="https://purl.org/ffdr-ontology#">
    <owl:Ontology rdf:about="https://purl.org/ffdr-ontology">
        <owl:versionIRI rdf:resource="https://purl.org/ffdr-ontology/1.0.0"/>
        <terms:abstract xml:lang="en">Abstract

Firefighters require accurate and timely information regarding a building and its
environment to perform their duty safely and effectively during a fire emergency. However, due to the chaotic nature of building fires, firefighters often receive erroneous, conflicting, or delayed information that can affect the outcome of a hazard. In this paper, we propose a solution in the form of an ontology that defines building and environmental data needed by firefighters during a building
fire emergency. The ontology can be a basis for developing intelligent tools and systems that collect building and environmental data from different data sources and provide comprehensive information to firefighters. It can also facilitate the data exchange process between the different personnel involved in emergency response. The ontology was developed by following the METHONTOLOGY method, and it was implemented using the web ontology language (OWL) in
Protégé 5.5.0.</terms:abstract>
        <terms:creator xml:lang="en">Eyosias Guyo

Technische Universität Berlin, Germany
Trimble Solutions Oy, Finland

eyosias.guyo@trimble.com</terms:creator>
        <terms:creator xml:lang="en">Timo Hartmann

Technische Universität Berlin, Germany</terms:creator>
        <terms:language xml:lang="en">English</terms:language>
        <terms:license xml:lang="en">This work is licensed under a Creative Commons Attribution-NonCommercial 4.0 International.
 
License: https://creativecommons.org/licenses/by-nc/4.0/</terms:license>
        <terms:title xml:lang="en">Firefighters&apos; Data Requirements Ontology</terms:title>
        <rdfs:comment xml:lang="en">Domain: 

Building fire emergency</rdfs:comment>
        <rdfs:comment xml:lang="en">Intended use:

The ontology can be a basis for developing tools and systems that gather essential data about a building and its surroundings and provide the collected data to firefighters in an integrated form. 
It can also facilitate the data exchange process between different personnel involved in emergency response.</rdfs:comment>
        <rdfs:comment xml:lang="en">Purpose:

Building an ontology to represent data regarding several features and components of a building and its surroundings that firefighters need when responding to building fires.</rdfs:comment>
        <rdfs:comment xml:lang="en">Scope:

The focus is on data about an affected building, its different components, and its surrounding.</rdfs:comment>
        <rdfs:label xml:lang="en">Firefighters&apos; Data Requirements Ontology</rdfs:label>
        <owl:versionInfo xml:lang="en">V 1.0.0</owl:versionInfo>
    </owl:Ontology>
    


    <!-- 
    ///////////////////////////////////////////////////////////////////////////////////////
    //
    // Annotation properties
    //
    ///////////////////////////////////////////////////////////////////////////////////////
     -->


    


    <!-- http://purl.org/dc/terms/abstract -->


    <owl:AnnotationProperty rdf:about="http://purl.org/dc/terms/abstract"/>
    


    <!-- http://purl.org/dc/terms/creator -->


    <owl:AnnotationProperty rdf:about="http://purl.org/dc/terms/creator"/>
    


    <!-- http://purl.org/dc/terms/description -->


    <owl:AnnotationProperty rdf:about="http://purl.org/dc/terms/description"/>
    


    <!-- http://purl.org/dc/terms/language -->


    <owl:AnnotationProperty rdf:about="http://purl.org/dc/terms/language"/>
    


    <!-- http://purl.org/dc/terms/license -->


    <owl:AnnotationProperty rdf:about="http://purl.org/dc/terms/license"/>
    


    <!-- http://purl.org/dc/terms/title -->


    <owl:AnnotationProperty rdf:about="http://purl.org/dc/terms/title"/>
    


    <!-- 
    ///////////////////////////////////////////////////////////////////////////////////////
    //
    // Object Properties
    //
    ///////////////////////////////////////////////////////////////////////////////////////
     -->


    


    <!-- https://purl.org/ffdr-ontology#contains -->


    <owl:ObjectProperty rdf:about="https://purl.org/ffdr-ontology#contains">
        <rdfs:subPropertyOf rdf:resource="http://www.w3.org/2002/07/owl#topObjectProperty"/>
        <owl:inverseOf rdf:resource="https://purl.org/ffdr-ontology#isContainedBy"/>
        <rdfs:domain>
            <owl:Class>
                <owl:unionOf rdf:parseType="Collection">
                    <rdf:Description rdf:about="https://purl.org/ffdr-ontology#FireCommandCenter"/>
                    <rdf:Description rdf:about="https://purl.org/ffdr-ontology#IncidentSite"/>
                </owl:unionOf>
            </owl:Class>
        </rdfs:domain>
        <rdfs:range>
            <owl:Class>
                <owl:unionOf rdf:parseType="Collection">
                    <rdf:Description rdf:about="https://purl.org/ffdr-ontology#ControlPanel"/>
                    <rdf:Description rdf:about="https://purl.org/ffdr-ontology#FireCommandCenter"/>
                    <rdf:Description rdf:about="https://purl.org/ffdr-ontology#IncidentBuilding"/>
                    <rdf:Description rdf:about="https://purl.org/ffdr-ontology#SurroundingStructure"/>
                    <rdf:Description rdf:about="https://purl.org/ffdr-ontology#SurroundingTerrain"/>
                </owl:unionOf>
            </owl:Class>
        </rdfs:range>
        <rdfs:comment xml:lang="en">The &apos;contains&apos; object property represents a relationship where an entity contains another entity.</rdfs:comment>
        <rdfs:label xml:lang="en">contains</rdfs:label>
    </owl:ObjectProperty>
    


    <!-- https://purl.org/ffdr-ontology#hasAddress -->


    <owl:ObjectProperty rdf:about="https://purl.org/ffdr-ontology#hasAddress">
        <owl:inverseOf rdf:resource="https://purl.org/ffdr-ontology#isAddressOf"/>
        <rdfs:domain>
            <owl:Class>
                <owl:unionOf rdf:parseType="Collection">
                    <rdf:Description rdf:about="https://purl.org/ffdr-ontology#BuildingUtilitySystem"/>
                    <rdf:Description rdf:about="https://purl.org/ffdr-ontology#EmergencyServiceProvider"/>
                    <rdf:Description rdf:about="https://purl.org/ffdr-ontology#IncidentBuilding"/>
                    <rdf:Description rdf:about="https://purl.org/ffdr-ontology#IncidentSite"/>
                </owl:unionOf>
            </owl:Class>
        </rdfs:domain>
        <rdfs:range>
            <owl:Class>
                <owl:unionOf rdf:parseType="Collection">
                    <rdf:Description rdf:about="https://purl.org/ffdr-ontology#Address"/>
                    <rdf:Description rdf:about="https://purl.org/ffdr-ontology#EmergencyServiceProviderContactAddress"/>
                    <rdf:Description rdf:about="https://purl.org/ffdr-ontology#PublicSafetyAgencyContactAddress"/>
                    <rdf:Description rdf:about="https://purl.org/ffdr-ontology#UtilityContactAddress"/>
                </owl:unionOf>
            </owl:Class>
        </rdfs:range>
        <rdfs:comment xml:lang="en">The &apos;hasAddress&apos; object property represents a relationship between an entity and its address.</rdfs:comment>
        <rdfs:label xml:lang="en">hasAddress</rdfs:label>
    </owl:ObjectProperty>
    


    <!-- https://purl.org/ffdr-ontology#hasBuildingPlan -->


    <owl:ObjectProperty rdf:about="https://purl.org/ffdr-ontology#hasBuildingPlan">
        <owl:inverseOf rdf:resource="https://purl.org/ffdr-ontology#isBuildingPlanOf"/>
        <rdfs:domain rdf:resource="https://purl.org/ffdr-ontology#IncidentBuilding"/>
        <rdfs:range rdf:resource="https://purl.org/ffdr-ontology#BuildingPlan"/>
        <rdfs:comment xml:lang="en">The &apos;hasBuildingPlan&apos; object property represents a relationship between a building and its plan.</rdfs:comment>
        <rdfs:label xml:lang="en">hasBuildingPlan</rdfs:label>
    </owl:ObjectProperty>
    


    <!-- https://purl.org/ffdr-ontology#hasComponent -->


    <owl:ObjectProperty rdf:about="https://purl.org/ffdr-ontology#hasComponent">
        <owl:inverseOf rdf:resource="https://purl.org/ffdr-ontology#isComponentOf"/>
        <rdfs:domain rdf:resource="https://purl.org/ffdr-ontology#IncidentBuilding"/>
        <rdfs:range rdf:resource="https://purl.org/ffdr-ontology#BuildingComponent"/>
        <rdfs:comment xml:lang="en">The &apos;hasComponent&apos; object property represents a relationship between a building and its components.</rdfs:comment>
        <rdfs:label xml:lang="en">hasComponent</rdfs:label>
    </owl:ObjectProperty>
    


    <!-- https://purl.org/ffdr-ontology#hasConnectionWith -->


    <owl:ObjectProperty rdf:about="https://purl.org/ffdr-ontology#hasConnectionWith">
        <rdf:type rdf:resource="http://www.w3.org/2002/07/owl#SymmetricProperty"/>
        <rdfs:domain>
            <owl:Class>
                <owl:unionOf rdf:parseType="Collection">
                    <rdf:Description rdf:about="https://purl.org/ffdr-ontology#AutomaticFireExtinguishingSystem"/>
                    <rdf:Description rdf:about="https://purl.org/ffdr-ontology#FireAlarmSystem"/>
                </owl:unionOf>
            </owl:Class>
        </rdfs:domain>
        <rdfs:range>
            <owl:Class>
                <owl:unionOf rdf:parseType="Collection">
                    <rdf:Description rdf:about="https://purl.org/ffdr-ontology#AutomaticFireExtinguishingSystem"/>
                    <rdf:Description rdf:about="https://purl.org/ffdr-ontology#FireAlarmSystem"/>
                </owl:unionOf>
            </owl:Class>
        </rdfs:range>
        <rdfs:comment xml:lang="en">The &apos;hasConnectionWith&apos; object property represents a relationship where two elements or systems are connected.</rdfs:comment>
        <rdfs:label xml:lang="en">hasConnectionWith</rdfs:label>
    </owl:ObjectProperty>
    


    <!-- https://purl.org/ffdr-ontology#hasConstructionType -->


    <owl:ObjectProperty rdf:about="https://purl.org/ffdr-ontology#hasConstructionType">
        <owl:inverseOf rdf:resource="https://purl.org/ffdr-ontology#isConstructionTypeOf"/>
        <rdfs:domain rdf:resource="https://purl.org/ffdr-ontology#IncidentBuilding"/>
        <rdfs:range rdf:resource="https://purl.org/ffdr-ontology#ConstructionType"/>
        <rdfs:comment xml:lang="en">The &apos;hasConstructionType&apos; object property represents a relationship between a building and its construction type.</rdfs:comment>
        <rdfs:label xml:lang="en">hasConstructionType</rdfs:label>
    </owl:ObjectProperty>
    


    <!-- https://purl.org/ffdr-ontology#hasControlPanel -->


    <owl:ObjectProperty rdf:about="https://purl.org/ffdr-ontology#hasControlPanel">
        <owl:inverseOf rdf:resource="https://purl.org/ffdr-ontology#isControlPanelOf"/>
        <rdfs:domain>
            <owl:Class>
                <owl:unionOf rdf:parseType="Collection">
                    <rdf:Description rdf:about="https://purl.org/ffdr-ontology#BuildingUtilitySystem"/>
                    <rdf:Description rdf:about="https://purl.org/ffdr-ontology#Door"/>
                    <rdf:Description rdf:about="https://purl.org/ffdr-ontology#Elevator"/>
                    <rdf:Description rdf:about="https://purl.org/ffdr-ontology#FarsFillStation"/>
                    <rdf:Description rdf:about="https://purl.org/ffdr-ontology#FireAlarmSystem"/>
                    <rdf:Description rdf:about="https://purl.org/ffdr-ontology#MassNotificationSystem"/>
                    <rdf:Description rdf:about="https://purl.org/ffdr-ontology#SmokeControlSystem"/>
                </owl:unionOf>
            </owl:Class>
        </rdfs:domain>
        <rdfs:range>
            <owl:Class>
                <owl:unionOf rdf:parseType="Collection">
                    <rdf:Description rdf:about="https://purl.org/ffdr-ontology#AlarmSystemAnnunciatorPanel"/>
                    <rdf:Description rdf:about="https://purl.org/ffdr-ontology#DoorUnlockingSystemControlPanel"/>
                    <rdf:Description rdf:about="https://purl.org/ffdr-ontology#ElevatorOverrideControlPanel"/>
                    <rdf:Description rdf:about="https://purl.org/ffdr-ontology#FarsControlPanel"/>
                    <rdf:Description rdf:about="https://purl.org/ffdr-ontology#MassNotificationSystemControlPanel"/>
                    <rdf:Description rdf:about="https://purl.org/ffdr-ontology#SmokeControlSystemControlPanel"/>
                    <rdf:Description rdf:about="https://purl.org/ffdr-ontology#UtilityControlPanel"/>
                </owl:unionOf>
            </owl:Class>
        </rdfs:range>
        <rdfs:comment xml:lang="en">The &apos;hasControlPanel&apos; object property represents a relationship between a system or an element and its control panel.</rdfs:comment>
        <rdfs:label xml:lang="en">hasControlPanel</rdfs:label>
    </owl:ObjectProperty>
    


    <!-- https://purl.org/ffdr-ontology#hasFireExtinguishingSystem -->


    <owl:ObjectProperty rdf:about="https://purl.org/ffdr-ontology#hasFireExtinguishingSystem">
        <owl:inverseOf rdf:resource="https://purl.org/ffdr-ontology#isFireExtinguishingSystemOf"/>
        <rdfs:domain>
            <owl:Class>
                <owl:unionOf rdf:parseType="Collection">
                    <rdf:Description rdf:about="https://purl.org/ffdr-ontology#ConcealedSpace"/>
                    <rdf:Description rdf:about="https://purl.org/ffdr-ontology#Elevator"/>
                    <rdf:Description rdf:about="https://purl.org/ffdr-ontology#Ramp"/>
                    <rdf:Description rdf:about="https://purl.org/ffdr-ontology#Stairway"/>
                </owl:unionOf>
            </owl:Class>
        </rdfs:domain>
        <rdfs:range rdf:resource="https://purl.org/ffdr-ontology#AutomaticFireExtinguishingSystem"/>
        <rdfs:comment xml:lang="en">The &apos;hasFireExtinguishingSystem&apos; object property represents a relationship between an area or an element and its fire extinguishing system.</rdfs:comment>
        <rdfs:label xml:lang="en">hasFireExtinguishingSystem</rdfs:label>
    </owl:ObjectProperty>
    


    <!-- https://purl.org/ffdr-ontology#hasHoseConnection -->


    <owl:ObjectProperty rdf:about="https://purl.org/ffdr-ontology#hasHoseConnection">
        <owl:inverseOf rdf:resource="https://purl.org/ffdr-ontology#isHoseConnectionOf"/>
        <rdfs:domain>
            <owl:Class>
                <owl:unionOf rdf:parseType="Collection">
                    <rdf:Description rdf:about="https://purl.org/ffdr-ontology#FireDepartmentConnection"/>
                    <rdf:Description rdf:about="https://purl.org/ffdr-ontology#FireHoseConnection"/>
                    <rdf:Description rdf:about="https://purl.org/ffdr-ontology#FireHydrant"/>
                </owl:unionOf>
            </owl:Class>
        </rdfs:domain>
        <rdfs:range rdf:resource="https://purl.org/ffdr-ontology#HoseConnection"/>
        <rdfs:comment xml:lang="en">The &apos;hasHoseConnection&apos; object property represents a relationship between an element and its hose connection.</rdfs:comment>
        <rdfs:label xml:lang="en">hasHoseConnection</rdfs:label>
    </owl:ObjectProperty>
    


    <!-- https://purl.org/ffdr-ontology#hasMaterial -->


    <owl:ObjectProperty rdf:about="https://purl.org/ffdr-ontology#hasMaterial">
        <owl:inverseOf rdf:resource="https://purl.org/ffdr-ontology#isMaterialOf"/>
        <rdfs:domain>
            <owl:Class>
                <owl:unionOf rdf:parseType="Collection">
                    <rdf:Description rdf:about="https://purl.org/ffdr-ontology#FireandSmokeProtectionElement"/>
                    <rdf:Description rdf:about="https://purl.org/ffdr-ontology#NonStructuralElement"/>
                    <rdf:Description rdf:about="https://purl.org/ffdr-ontology#Road"/>
                    <rdf:Description rdf:about="https://purl.org/ffdr-ontology#StructuralElement"/>
                </owl:unionOf>
            </owl:Class>
        </rdfs:domain>
        <rdfs:range rdf:resource="https://purl.org/ffdr-ontology#Material"/>
        <rdfs:comment xml:lang="en">The &apos;hasMaterial&apos; object property represents a relationship between an element and the material its made of.</rdfs:comment>
        <rdfs:label xml:lang="en">hasMaterial</rdfs:label>
    </owl:ObjectProperty>
    


    <!-- https://purl.org/ffdr-ontology#hasOccupancy -->


    <owl:ObjectProperty rdf:about="https://purl.org/ffdr-ontology#hasOccupancy">
        <owl:inverseOf rdf:resource="https://purl.org/ffdr-ontology#isOccupancyOf"/>
        <rdfs:domain rdf:resource="https://purl.org/ffdr-ontology#IncidentBuilding"/>
        <rdfs:range rdf:resource="https://purl.org/ffdr-ontology#BuildingOccupancy"/>
        <rdfs:comment xml:lang="en">The &apos;hasOccupancy&apos; object property represents a relationship between a building and its occupancy.</rdfs:comment>
        <rdfs:label xml:lang="en">hasOccupancy</rdfs:label>
    </owl:ObjectProperty>
    


    <!-- https://purl.org/ffdr-ontology#hasShaftEnclosure -->


    <owl:ObjectProperty rdf:about="https://purl.org/ffdr-ontology#hasShaftEnclosure">
        <owl:inverseOf rdf:resource="https://purl.org/ffdr-ontology#isShaftEnclosureOf"/>
        <rdfs:domain rdf:resource="https://purl.org/ffdr-ontology#VerticalOpening"/>
        <rdfs:range rdf:resource="https://purl.org/ffdr-ontology#ShaftEnclosure"/>
        <rdfs:comment xml:lang="en">The &apos;hasShaftEnclosure&apos; object property represents a relationship between a shaft (vertical opening) and its enclosure.</rdfs:comment>
        <rdfs:label xml:lang="en">hasShaftEnclosure</rdfs:label>
    </owl:ObjectProperty>
    


    <!-- https://purl.org/ffdr-ontology#hasWaterSource -->


    <owl:ObjectProperty rdf:about="https://purl.org/ffdr-ontology#hasWaterSource">
        <owl:inverseOf rdf:resource="https://purl.org/ffdr-ontology#isWaterSourceOf"/>
        <rdfs:domain>
            <owl:Class>
                <owl:unionOf rdf:parseType="Collection">
                    <rdf:Description rdf:about="https://purl.org/ffdr-ontology#AutomaticSprinklerSystem"/>
                    <rdf:Description rdf:about="https://purl.org/ffdr-ontology#FireDepartmentConnection"/>
                    <rdf:Description rdf:about="https://purl.org/ffdr-ontology#FireHoseConnection"/>
                    <rdf:Description rdf:about="https://purl.org/ffdr-ontology#FireHydrant"/>
                    <rdf:Description rdf:about="https://purl.org/ffdr-ontology#StandpipeSystem"/>
                </owl:unionOf>
            </owl:Class>
        </rdfs:domain>
        <rdfs:range>
            <owl:Class>
                <owl:unionOf rdf:parseType="Collection">
                    <rdf:Description rdf:about="https://purl.org/ffdr-ontology#StandpipeSystem"/>
                    <rdf:Description rdf:about="https://purl.org/ffdr-ontology#WaterSource"/>
                </owl:unionOf>
            </owl:Class>
        </rdfs:range>
        <rdfs:comment xml:lang="en">The &apos;hasWaterSource&apos; object property represents a relationship between an element or a system and its water source.</rdfs:comment>
        <rdfs:label xml:lang="en">hasWaterSource</rdfs:label>
    </owl:ObjectProperty>
    


    <!-- https://purl.org/ffdr-ontology#hasWeatherCondition -->


    <owl:ObjectProperty rdf:about="https://purl.org/ffdr-ontology#hasWeatherCondition">
        <owl:inverseOf rdf:resource="https://purl.org/ffdr-ontology#isWeatherConditionOf"/>
        <rdfs:domain rdf:resource="https://purl.org/ffdr-ontology#IncidentSite"/>
        <rdfs:range rdf:resource="https://purl.org/ffdr-ontology#WeatherCondition"/>
        <rdfs:comment xml:lang="en">The &apos;hasWeatherCondition&apos; object property represents a relationship between a site and its weather condition.</rdfs:comment>
        <rdfs:label xml:lang="en">hasWeatherCondition</rdfs:label>
    </owl:ObjectProperty>
    


    <!-- https://purl.org/ffdr-ontology#isAddressOf -->


    <owl:ObjectProperty rdf:about="https://purl.org/ffdr-ontology#isAddressOf">
        <rdfs:domain>
            <owl:Class>
                <owl:unionOf rdf:parseType="Collection">
                    <rdf:Description rdf:about="https://purl.org/ffdr-ontology#Address"/>
                    <rdf:Description rdf:about="https://purl.org/ffdr-ontology#EmergencyServiceProviderContactAddress"/>
                    <rdf:Description rdf:about="https://purl.org/ffdr-ontology#PublicSafetyAgencyContactAddress"/>
                    <rdf:Description rdf:about="https://purl.org/ffdr-ontology#UtilityContactAddress"/>
                </owl:unionOf>
            </owl:Class>
        </rdfs:domain>
        <rdfs:range>
            <owl:Class>
                <owl:unionOf rdf:parseType="Collection">
                    <rdf:Description rdf:about="https://purl.org/ffdr-ontology#BuildingUtilitySystem"/>
                    <rdf:Description rdf:about="https://purl.org/ffdr-ontology#EmergencyServiceProvider"/>
                    <rdf:Description rdf:about="https://purl.org/ffdr-ontology#IncidentBuilding"/>
                    <rdf:Description rdf:about="https://purl.org/ffdr-ontology#IncidentSite"/>
                </owl:unionOf>
            </owl:Class>
        </rdfs:range>
        <rdfs:label xml:lang="en">isAddressOf</rdfs:label>
    </owl:ObjectProperty>
    


    <!-- https://purl.org/ffdr-ontology#isBuildingPlanOf -->


    <owl:ObjectProperty rdf:about="https://purl.org/ffdr-ontology#isBuildingPlanOf">
        <rdfs:domain rdf:resource="https://purl.org/ffdr-ontology#BuildingPlan"/>
        <rdfs:range rdf:resource="https://purl.org/ffdr-ontology#IncidentBuilding"/>
        <rdfs:label xml:lang="en">isBuildingPlanOf</rdfs:label>
    </owl:ObjectProperty>
    


    <!-- https://purl.org/ffdr-ontology#isComponentOf -->


    <owl:ObjectProperty rdf:about="https://purl.org/ffdr-ontology#isComponentOf">
        <rdfs:domain rdf:resource="https://purl.org/ffdr-ontology#BuildingComponent"/>
        <rdfs:range rdf:resource="https://purl.org/ffdr-ontology#IncidentBuilding"/>
        <rdfs:label xml:lang="en">isComponentOf</rdfs:label>
    </owl:ObjectProperty>
    


    <!-- https://purl.org/ffdr-ontology#isConstructionTypeOf -->


    <owl:ObjectProperty rdf:about="https://purl.org/ffdr-ontology#isConstructionTypeOf">
        <rdfs:domain rdf:resource="https://purl.org/ffdr-ontology#ConstructionType"/>
        <rdfs:range rdf:resource="https://purl.org/ffdr-ontology#IncidentBuilding"/>
        <rdfs:label xml:lang="en">isConstructionTypeOf</rdfs:label>
    </owl:ObjectProperty>
    


    <!-- https://purl.org/ffdr-ontology#isContainedBy -->


    <owl:ObjectProperty rdf:about="https://purl.org/ffdr-ontology#isContainedBy">
        <rdfs:domain>
            <owl:Class>
                <owl:unionOf rdf:parseType="Collection">
                    <rdf:Description rdf:about="https://purl.org/ffdr-ontology#ControlPanel"/>
                    <rdf:Description rdf:about="https://purl.org/ffdr-ontology#FireCommandCenter"/>
                    <rdf:Description rdf:about="https://purl.org/ffdr-ontology#IncidentBuilding"/>
                    <rdf:Description rdf:about="https://purl.org/ffdr-ontology#SurroundingStructure"/>
                    <rdf:Description rdf:about="https://purl.org/ffdr-ontology#SurroundingTerrain"/>
                </owl:unionOf>
            </owl:Class>
        </rdfs:domain>
        <rdfs:range>
            <owl:Class>
                <owl:unionOf rdf:parseType="Collection">
                    <rdf:Description rdf:about="https://purl.org/ffdr-ontology#FireCommandCenter"/>
                    <rdf:Description rdf:about="https://purl.org/ffdr-ontology#IncidentSite"/>
                </owl:unionOf>
            </owl:Class>
        </rdfs:range>
        <rdfs:label xml:lang="en">isContainedBy</rdfs:label>
    </owl:ObjectProperty>
    


    <!-- https://purl.org/ffdr-ontology#isControlPanelOf -->


    <owl:ObjectProperty rdf:about="https://purl.org/ffdr-ontology#isControlPanelOf">
        <rdfs:domain>
            <owl:Class>
                <owl:unionOf rdf:parseType="Collection">
                    <rdf:Description rdf:about="https://purl.org/ffdr-ontology#AlarmSystemAnnunciatorPanel"/>
                    <rdf:Description rdf:about="https://purl.org/ffdr-ontology#DoorUnlockingSystemControlPanel"/>
                    <rdf:Description rdf:about="https://purl.org/ffdr-ontology#ElevatorOverrideControlPanel"/>
                    <rdf:Description rdf:about="https://purl.org/ffdr-ontology#FarsControlPanel"/>
                    <rdf:Description rdf:about="https://purl.org/ffdr-ontology#MassNotificationSystemControlPanel"/>
                    <rdf:Description rdf:about="https://purl.org/ffdr-ontology#SmokeControlSystemControlPanel"/>
                    <rdf:Description rdf:about="https://purl.org/ffdr-ontology#UtilityControlPanel"/>
                </owl:unionOf>
            </owl:Class>
        </rdfs:domain>
        <rdfs:range>
            <owl:Class>
                <owl:unionOf rdf:parseType="Collection">
                    <rdf:Description rdf:about="https://purl.org/ffdr-ontology#BuildingUtilitySystem"/>
                    <rdf:Description rdf:about="https://purl.org/ffdr-ontology#Door"/>
                    <rdf:Description rdf:about="https://purl.org/ffdr-ontology#Elevator"/>
                    <rdf:Description rdf:about="https://purl.org/ffdr-ontology#FarsFillStation"/>
                    <rdf:Description rdf:about="https://purl.org/ffdr-ontology#FireAlarmSystem"/>
                    <rdf:Description rdf:about="https://purl.org/ffdr-ontology#MassNotificationSystem"/>
                    <rdf:Description rdf:about="https://purl.org/ffdr-ontology#SmokeControlSystem"/>
                </owl:unionOf>
            </owl:Class>
        </rdfs:range>
        <rdfs:label xml:lang="en">isControlPanelOf</rdfs:label>
    </owl:ObjectProperty>
    


    <!-- https://purl.org/ffdr-ontology#isFireExtinguishingSystemOf -->


    <owl:ObjectProperty rdf:about="https://purl.org/ffdr-ontology#isFireExtinguishingSystemOf">
        <rdfs:domain rdf:resource="https://purl.org/ffdr-ontology#AutomaticFireExtinguishingSystem"/>
        <rdfs:range>
            <owl:Class>
                <owl:unionOf rdf:parseType="Collection">
                    <rdf:Description rdf:about="https://purl.org/ffdr-ontology#ConcealedSpace"/>
                    <rdf:Description rdf:about="https://purl.org/ffdr-ontology#Elevator"/>
                    <rdf:Description rdf:about="https://purl.org/ffdr-ontology#Ramp"/>
                    <rdf:Description rdf:about="https://purl.org/ffdr-ontology#Stairway"/>
                </owl:unionOf>
            </owl:Class>
        </rdfs:range>
        <rdfs:label xml:lang="en">isFireExtinguishingSystemOf</rdfs:label>
    </owl:ObjectProperty>
    


    <!-- https://purl.org/ffdr-ontology#isHoseConnectionOf -->


    <owl:ObjectProperty rdf:about="https://purl.org/ffdr-ontology#isHoseConnectionOf">
        <rdfs:domain rdf:resource="https://purl.org/ffdr-ontology#HoseConnection"/>
        <rdfs:range>
            <owl:Class>
                <owl:unionOf rdf:parseType="Collection">
                    <rdf:Description rdf:about="https://purl.org/ffdr-ontology#FireDepartmentConnection"/>
                    <rdf:Description rdf:about="https://purl.org/ffdr-ontology#FireHoseConnection"/>
                    <rdf:Description rdf:about="https://purl.org/ffdr-ontology#FireHydrant"/>
                </owl:unionOf>
            </owl:Class>
        </rdfs:range>
        <rdfs:label xml:lang="en">isHoseConnectionOf</rdfs:label>
    </owl:ObjectProperty>
    


    <!-- https://purl.org/ffdr-ontology#isMaterialOf -->


    <owl:ObjectProperty rdf:about="https://purl.org/ffdr-ontology#isMaterialOf">
        <rdfs:domain rdf:resource="https://purl.org/ffdr-ontology#Material"/>
        <rdfs:range>
            <owl:Class>
                <owl:unionOf rdf:parseType="Collection">
                    <rdf:Description rdf:about="https://purl.org/ffdr-ontology#FireandSmokeProtectionElement"/>
                    <rdf:Description rdf:about="https://purl.org/ffdr-ontology#NonStructuralElement"/>
                    <rdf:Description rdf:about="https://purl.org/ffdr-ontology#Road"/>
                    <rdf:Description rdf:about="https://purl.org/ffdr-ontology#StructuralElement"/>
                </owl:unionOf>
            </owl:Class>
        </rdfs:range>
        <rdfs:label xml:lang="en">isMaterialOf</rdfs:label>
    </owl:ObjectProperty>
    


    <!-- https://purl.org/ffdr-ontology#isOccupancyOf -->


    <owl:ObjectProperty rdf:about="https://purl.org/ffdr-ontology#isOccupancyOf">
        <rdfs:domain rdf:resource="https://purl.org/ffdr-ontology#BuildingOccupancy"/>
        <rdfs:range rdf:resource="https://purl.org/ffdr-ontology#IncidentBuilding"/>
        <rdfs:label xml:lang="en">isOccupancyOf</rdfs:label>
    </owl:ObjectProperty>
    


    <!-- https://purl.org/ffdr-ontology#isShaftEnclosureOf -->


    <owl:ObjectProperty rdf:about="https://purl.org/ffdr-ontology#isShaftEnclosureOf">
        <rdfs:domain rdf:resource="https://purl.org/ffdr-ontology#ShaftEnclosure"/>
        <rdfs:range rdf:resource="https://purl.org/ffdr-ontology#VerticalOpening"/>
        <rdfs:label xml:lang="en">isShaftEnclosureOf</rdfs:label>
    </owl:ObjectProperty>
    


    <!-- https://purl.org/ffdr-ontology#isWaterSourceOf -->


    <owl:ObjectProperty rdf:about="https://purl.org/ffdr-ontology#isWaterSourceOf">
        <rdfs:domain>
            <owl:Class>
                <owl:unionOf rdf:parseType="Collection">
                    <rdf:Description rdf:about="https://purl.org/ffdr-ontology#StandpipeSystem"/>
                    <rdf:Description rdf:about="https://purl.org/ffdr-ontology#WaterSource"/>
                </owl:unionOf>
            </owl:Class>
        </rdfs:domain>
        <rdfs:range>
            <owl:Class>
                <owl:unionOf rdf:parseType="Collection">
                    <rdf:Description rdf:about="https://purl.org/ffdr-ontology#AutomaticSprinklerSystem"/>
                    <rdf:Description rdf:about="https://purl.org/ffdr-ontology#FireDepartmentConnection"/>
                    <rdf:Description rdf:about="https://purl.org/ffdr-ontology#FireHoseConnection"/>
                    <rdf:Description rdf:about="https://purl.org/ffdr-ontology#FireHydrant"/>
                    <rdf:Description rdf:about="https://purl.org/ffdr-ontology#StandpipeSystem"/>
                </owl:unionOf>
            </owl:Class>
        </rdfs:range>
        <rdfs:label xml:lang="en">isWaterSourceOf</rdfs:label>
    </owl:ObjectProperty>
    


    <!-- https://purl.org/ffdr-ontology#isWeatherConditionOf -->


    <owl:ObjectProperty rdf:about="https://purl.org/ffdr-ontology#isWeatherConditionOf">
        <rdfs:domain rdf:resource="https://purl.org/ffdr-ontology#WeatherCondition"/>
        <rdfs:range rdf:resource="https://purl.org/ffdr-ontology#IncidentSite"/>
        <rdfs:label xml:lang="en">isWeatherConditionOf</rdfs:label>
    </owl:ObjectProperty>
    


    <!-- 
    ///////////////////////////////////////////////////////////////////////////////////////
    //
    // Data properties
    //
    ///////////////////////////////////////////////////////////////////////////////////////
     -->


    


    <!-- https://purl.org/ffdr-ontology#hasAccessBarrierType -->


    <owl:DatatypeProperty rdf:about="https://purl.org/ffdr-ontology#hasAccessBarrierType">
        <rdfs:domain rdf:resource="https://purl.org/ffdr-ontology#FireLane"/>
        <rdfs:range rdf:resource="http://www.w3.org/2001/XMLSchema#string"/>
        <rdfs:comment xml:lang="en">Access barrier type could be a gate, bollards, or none.</rdfs:comment>
        <rdfs:comment xml:lang="en">The &apos;hasAccessBarrierType&apos; data property represents the types of barriers that can block access.</rdfs:comment>
        <rdfs:label xml:lang="en">hasAccessBarrierType</rdfs:label>
    </owl:DatatypeProperty>
    


    <!-- https://purl.org/ffdr-ontology#hasAnglesOfApproach -->


    <owl:DatatypeProperty rdf:about="https://purl.org/ffdr-ontology#hasAnglesOfApproach">
        <rdfs:domain rdf:resource="https://purl.org/ffdr-ontology#FireLane"/>
        <rdfs:range rdf:resource="http://www.w3.org/2001/XMLSchema#double"/>
        <rdfs:comment xml:lang="en">The &apos;hasAnglesOfApproach&apos; data property represents a given road&apos;s angle of approach or departure.</rdfs:comment>
        <rdfs:label xml:lang="en">hasAnglesOfApproach</rdfs:label>
    </owl:DatatypeProperty>
    


    <!-- https://purl.org/ffdr-ontology#hasArea -->


    <owl:DatatypeProperty rdf:about="https://purl.org/ffdr-ontology#hasArea">
        <rdfs:domain rdf:resource="https://purl.org/ffdr-ontology#ParkingLot"/>
        <rdfs:range rdf:resource="http://www.w3.org/2001/XMLSchema#double"/>
        <rdfs:comment xml:lang="en">The &apos;hasArea&apos; data property represents the area of a given space.</rdfs:comment>
        <rdfs:label xml:lang="en">hasArea</rdfs:label>
    </owl:DatatypeProperty>
    


    <!-- https://purl.org/ffdr-ontology#hasBuildingArea -->


    <owl:DatatypeProperty rdf:about="https://purl.org/ffdr-ontology#hasBuildingArea">
        <rdfs:domain rdf:resource="https://purl.org/ffdr-ontology#IncidentBuilding"/>
        <rdfs:range rdf:resource="http://www.w3.org/2001/XMLSchema#double"/>
        <rdfs:comment xml:lang="en">The &apos;hasBuildingArea&apos; data property represents a building&apos;s area.</rdfs:comment>
        <rdfs:label xml:lang="en">hasBuildingArea</rdfs:label>
    </owl:DatatypeProperty>
    


    <!-- https://purl.org/ffdr-ontology#hasBuildingHeight -->


    <owl:DatatypeProperty rdf:about="https://purl.org/ffdr-ontology#hasBuildingHeight">
        <rdfs:domain rdf:resource="https://purl.org/ffdr-ontology#IncidentBuilding"/>
        <rdfs:range rdf:resource="http://www.w3.org/2001/XMLSchema#double"/>
        <rdfs:comment xml:lang="en">The &apos;hasBuildingHeight&apos; data property represents a building&apos;s height.</rdfs:comment>
        <rdfs:label xml:lang="en">hasBuildingHeight</rdfs:label>
    </owl:DatatypeProperty>
    


    <!-- https://purl.org/ffdr-ontology#hasCapacity -->


    <owl:DatatypeProperty rdf:about="https://purl.org/ffdr-ontology#hasCapacity">
        <rdfs:domain>
            <owl:Class>
                <owl:unionOf rdf:parseType="Collection">
                    <rdf:Description rdf:about="https://purl.org/ffdr-ontology#AreaOfRefuge"/>
                    <rdf:Description rdf:about="https://purl.org/ffdr-ontology#Balcony"/>
                    <rdf:Description rdf:about="https://purl.org/ffdr-ontology#Elevator"/>
                    <rdf:Description rdf:about="https://purl.org/ffdr-ontology#Hallway"/>
                    <rdf:Description rdf:about="https://purl.org/ffdr-ontology#Ramp"/>
                    <rdf:Description rdf:about="https://purl.org/ffdr-ontology#Stairway"/>
                </owl:unionOf>
            </owl:Class>
        </rdfs:domain>
        <rdfs:range rdf:resource="http://www.w3.org/2001/XMLSchema#int"/>
        <rdfs:comment xml:lang="en">The &apos;hasCapacity&apos; data property represents the number of people a given area or room can support.</rdfs:comment>
        <rdfs:label xml:lang="en">hasCapacity</rdfs:label>
    </owl:DatatypeProperty>
    


    <!-- https://purl.org/ffdr-ontology#hasClass -->


    <owl:DatatypeProperty rdf:about="https://purl.org/ffdr-ontology#hasClass">
        <rdfs:domain rdf:resource="https://purl.org/ffdr-ontology#StandpipeSystem"/>
        <rdfs:range rdf:resource="http://www.w3.org/2001/XMLSchema#string"/>
        <rdfs:comment xml:lang="en">The &apos;hasClass&apos; data property represents the class of a given system.</rdfs:comment>
        <rdfs:label xml:lang="en">hasClass</rdfs:label>
    </owl:DatatypeProperty>
    


    <!-- https://purl.org/ffdr-ontology#hasCondition -->


    <owl:DatatypeProperty rdf:about="https://purl.org/ffdr-ontology#hasCondition">
        <rdfs:domain>
            <owl:Class>
                <owl:unionOf rdf:parseType="Collection">
                    <rdf:Description rdf:about="https://purl.org/ffdr-ontology#IncidentBuilding"/>
                    <rdf:Description rdf:about="https://purl.org/ffdr-ontology#Road"/>
                </owl:unionOf>
            </owl:Class>
        </rdfs:domain>
        <rdfs:range rdf:resource="http://www.w3.org/2001/XMLSchema#string"/>
        <rdfs:comment xml:lang="en">The &apos;hasCondition&apos; data property represents the state of a given structure.</rdfs:comment>
        <rdfs:label xml:lang="en">hasCondition</rdfs:label>
    </owl:DatatypeProperty>
    


    <!-- https://purl.org/ffdr-ontology#hasCoverageZone -->


    <owl:DatatypeProperty rdf:about="https://purl.org/ffdr-ontology#hasCoverageZone">
        <rdfs:domain>
            <owl:Class>
                <owl:unionOf rdf:parseType="Collection">
                    <rdf:Description rdf:about="https://purl.org/ffdr-ontology#AutomaticFireExtinguishingSystem"/>
                    <rdf:Description rdf:about="https://purl.org/ffdr-ontology#FireAlarmSystem"/>
                    <rdf:Description rdf:about="https://purl.org/ffdr-ontology#FireDepartmentConnection"/>
                    <rdf:Description rdf:about="https://purl.org/ffdr-ontology#MassNotificationSystem"/>
                    <rdf:Description rdf:about="https://purl.org/ffdr-ontology#SensorDetector"/>
                    <rdf:Description rdf:about="https://purl.org/ffdr-ontology#SmokeControlSystem"/>
                    <rdf:Description rdf:about="https://purl.org/ffdr-ontology#StandpipeSystem"/>
                </owl:unionOf>
            </owl:Class>
        </rdfs:domain>
        <rdfs:range rdf:resource="http://www.w3.org/2001/XMLSchema#string"/>
        <rdfs:comment xml:lang="en">The &apos;hasCoverageZone&apos; data property represents a zone covered by a given system.</rdfs:comment>
        <rdfs:label xml:lang="en">hasCoverageZone</rdfs:label>
    </owl:DatatypeProperty>
    


    <!-- https://purl.org/ffdr-ontology#hasDemography -->


    <owl:DatatypeProperty rdf:about="https://purl.org/ffdr-ontology#hasDemography">
        <rdfs:domain rdf:resource="https://purl.org/ffdr-ontology#IncidentSite"/>
        <rdfs:range rdf:resource="http://www.w3.org/2001/XMLSchema#string"/>
        <rdfs:comment xml:lang="en">The &apos;hasDemography&apos; data property represents the demography of a population at a given location.</rdfs:comment>
        <rdfs:label xml:lang="en">hasDemography</rdfs:label>
    </owl:DatatypeProperty>
    


    <!-- https://purl.org/ffdr-ontology#hasDescription -->


    <owl:DatatypeProperty rdf:about="https://purl.org/ffdr-ontology#hasDescription">
        <rdfs:domain>
            <owl:Class>
                <owl:unionOf rdf:parseType="Collection">
                    <rdf:Description rdf:about="https://purl.org/ffdr-ontology#BuildingOccupancy"/>
                    <rdf:Description rdf:about="https://purl.org/ffdr-ontology#ConcealedSpace"/>
                    <rdf:Description rdf:about="https://purl.org/ffdr-ontology#ConstructionType"/>
                    <rdf:Description rdf:about="https://purl.org/ffdr-ontology#ControlPanel"/>
                    <rdf:Description rdf:about="https://purl.org/ffdr-ontology#HazardousMaterial"/>
                    <rdf:Description rdf:about="https://purl.org/ffdr-ontology#HazardousSubstance"/>
                    <rdf:Description rdf:about="https://purl.org/ffdr-ontology#Obstruction"/>
                    <rdf:Description rdf:about="https://purl.org/ffdr-ontology#RoofTopElement"/>
                    <rdf:Description rdf:about="https://purl.org/ffdr-ontology#VerticalOpening"/>
                </owl:unionOf>
            </owl:Class>
        </rdfs:domain>
        <rdfs:range rdf:resource="http://www.w3.org/2001/XMLSchema#string"/>
        <rdfs:comment xml:lang="en">The &apos;hasDescription&apos; data property represents a description.</rdfs:comment>
        <rdfs:label xml:lang="en">hasDescription</rdfs:label>
    </owl:DatatypeProperty>
    


    <!-- https://purl.org/ffdr-ontology#hasDirectionToExit -->


    <owl:DatatypeProperty rdf:about="https://purl.org/ffdr-ontology#hasDirectionToExit">
        <rdfs:domain>
            <owl:Class>
                <owl:unionOf rdf:parseType="Collection">
                    <rdf:Description rdf:about="https://purl.org/ffdr-ontology#Ramp"/>
                    <rdf:Description rdf:about="https://purl.org/ffdr-ontology#Stairway"/>
                </owl:unionOf>
            </owl:Class>
        </rdfs:domain>
        <rdfs:range rdf:resource="http://www.w3.org/2001/XMLSchema#string"/>
        <rdfs:comment xml:lang="en">The &apos;hasDirectionToExit&apos; data property represents the exit direction of a stairway or ramp.</rdfs:comment>
        <rdfs:label xml:lang="en">hasDirectionToExit</rdfs:label>
    </owl:DatatypeProperty>
    


    <!-- https://purl.org/ffdr-ontology#hasDischargeLevel -->


    <owl:DatatypeProperty rdf:about="https://purl.org/ffdr-ontology#hasDischargeLevel">
        <rdfs:domain>
            <owl:Class>
                <owl:unionOf rdf:parseType="Collection">
                    <rdf:Description rdf:about="https://purl.org/ffdr-ontology#Elevator"/>
                    <rdf:Description rdf:about="https://purl.org/ffdr-ontology#Ramp"/>
                    <rdf:Description rdf:about="https://purl.org/ffdr-ontology#Stairway"/>
                </owl:unionOf>
            </owl:Class>
        </rdfs:domain>
        <rdfs:range rdf:resource="http://www.w3.org/2001/XMLSchema#string"/>
        <rdfs:comment xml:lang="en">The &apos;hasDischargeLevel&apos; data property represents the level where a stairway,  a ramp, or an elevator discharge.</rdfs:comment>
        <rdfs:label xml:lang="en">hasDischargeLevel</rdfs:label>
    </owl:DatatypeProperty>
    


    <!-- https://purl.org/ffdr-ontology#hasDistanceFromFDC -->


    <owl:DatatypeProperty rdf:about="https://purl.org/ffdr-ontology#hasDistanceFromFDC">
        <rdfs:domain>
            <owl:Class>
                <owl:unionOf rdf:parseType="Collection">
                    <rdf:Description rdf:about="https://purl.org/ffdr-ontology#FireHydrant"/>
                    <rdf:Description rdf:about="https://purl.org/ffdr-ontology#StaticWaterSource"/>
                </owl:unionOf>
            </owl:Class>
        </rdfs:domain>
        <rdfs:range rdf:resource="http://www.w3.org/2001/XMLSchema#double"/>
        <rdfs:comment xml:lang="en">The &apos;hasDistanceFromFDC&apos; data property represents the distance between a given element and a fire department connection (FDS).</rdfs:comment>
        <rdfs:label xml:lang="en">hasDistanceFromFDC</rdfs:label>
    </owl:DatatypeProperty>
    


    <!-- https://purl.org/ffdr-ontology#hasDistanceFromIncidentBuilding -->


    <owl:DatatypeProperty rdf:about="https://purl.org/ffdr-ontology#hasDistanceFromIncidentBuilding">
        <rdfs:domain>
            <owl:Class>
                <owl:unionOf rdf:parseType="Collection">
                    <rdf:Description rdf:about="https://purl.org/ffdr-ontology#EmergencyServiceProvider"/>
                    <rdf:Description rdf:about="https://purl.org/ffdr-ontology#StaticWaterSource"/>
                    <rdf:Description rdf:about="https://purl.org/ffdr-ontology#SurroundingStructure"/>
                </owl:unionOf>
            </owl:Class>
        </rdfs:domain>
        <rdfs:range rdf:resource="http://www.w3.org/2001/XMLSchema#double"/>
        <rdfs:comment xml:lang="en">The &apos;hasDistanceFromIncidentBuilding&apos; data property represents the distance between a given element and the incident building.</rdfs:comment>
        <rdfs:label xml:lang="en">hasDistanceFromIncidentBuilding</rdfs:label>
    </owl:DatatypeProperty>
    


    <!-- https://purl.org/ffdr-ontology#hasDistanceFromWaterSource -->


    <owl:DatatypeProperty rdf:about="https://purl.org/ffdr-ontology#hasDistanceFromWaterSource">
        <rdfs:domain rdf:resource="https://purl.org/ffdr-ontology#FireDepartmentConnection"/>
        <rdfs:range rdf:resource="http://www.w3.org/2001/XMLSchema#double"/>
        <rdfs:comment xml:lang="en">The &apos;hasDistanceFromWaterSource&apos; data property represents the distance between a given element and a water source.</rdfs:comment>
        <rdfs:label xml:lang="en">hasDistanceFromWaterSource</rdfs:label>
    </owl:DatatypeProperty>
    


    <!-- https://purl.org/ffdr-ontology#hasEnclosedArea -->


    <owl:DatatypeProperty rdf:about="https://purl.org/ffdr-ontology#hasEnclosedArea">
        <rdfs:domain>
            <owl:Class>
                <owl:unionOf rdf:parseType="Collection">
                    <rdf:Description rdf:about="https://purl.org/ffdr-ontology#FireBarrier"/>
                    <rdf:Description rdf:about="https://purl.org/ffdr-ontology#FirePartition"/>
                    <rdf:Description rdf:about="https://purl.org/ffdr-ontology#Firewall"/>
                    <rdf:Description rdf:about="https://purl.org/ffdr-ontology#SmokeBarrier"/>
                    <rdf:Description rdf:about="https://purl.org/ffdr-ontology#SmokePartition"/>
                </owl:unionOf>
            </owl:Class>
        </rdfs:domain>
        <rdfs:range rdf:resource="http://www.w3.org/2001/XMLSchema#string"/>
        <rdfs:comment xml:lang="en">The &apos;hasEnclosedArea&apos; data property represents an area enclosed and bounded by walls.</rdfs:comment>
        <rdfs:label xml:lang="en">hasEnclosedArea</rdfs:label>
    </owl:DatatypeProperty>
    


    <!-- https://purl.org/ffdr-ontology#hasExitTravelDistances -->


    <owl:DatatypeProperty rdf:about="https://purl.org/ffdr-ontology#hasExitTravelDistances">
        <rdfs:domain>
            <owl:Class>
                <owl:unionOf rdf:parseType="Collection">
                    <rdf:Description rdf:about="https://purl.org/ffdr-ontology#Door"/>
                    <rdf:Description rdf:about="https://purl.org/ffdr-ontology#Elevator"/>
                    <rdf:Description rdf:about="https://purl.org/ffdr-ontology#Ramp"/>
                    <rdf:Description rdf:about="https://purl.org/ffdr-ontology#Stairway"/>
                </owl:unionOf>
            </owl:Class>
        </rdfs:domain>
        <rdfs:range rdf:resource="http://www.w3.org/2001/XMLSchema#double"/>
        <rdfs:comment xml:lang="en">The &apos;hasExitTravelDistances&apos; data property represents the distance between a given element and a building exit.</rdfs:comment>
        <rdfs:label xml:lang="en">hasExitTravelDistances</rdfs:label>
    </owl:DatatypeProperty>
    


    <!-- https://purl.org/ffdr-ontology#hasFillPressure -->


    <owl:DatatypeProperty rdf:about="https://purl.org/ffdr-ontology#hasFillPressure">
        <rdfs:domain rdf:resource="https://purl.org/ffdr-ontology#FarsFillStation"/>
        <rdfs:range rdf:resource="http://www.w3.org/2001/XMLSchema#double"/>
        <rdfs:comment xml:lang="en">The &apos;hasFillPressure&apos; data property represents the pressure required to fill a given system or container.</rdfs:comment>
        <rdfs:label xml:lang="en">hasFillPressure</rdfs:label>
    </owl:DatatypeProperty>
    


    <!-- https://purl.org/ffdr-ontology#hasFillTime -->


    <owl:DatatypeProperty rdf:about="https://purl.org/ffdr-ontology#hasFillTime">
        <rdfs:domain rdf:resource="https://purl.org/ffdr-ontology#FarsFillStation"/>
        <rdfs:range rdf:resource="http://www.w3.org/2001/XMLSchema#double"/>
        <rdfs:comment xml:lang="en">The &apos;hasFillTime&apos; data property represents the time required to fill a given system or container.</rdfs:comment>
        <rdfs:label xml:lang="en">hasFillTime</rdfs:label>
    </owl:DatatypeProperty>
    


    <!-- https://purl.org/ffdr-ontology#hasFireExtinguisherRating -->


    <owl:DatatypeProperty rdf:about="https://purl.org/ffdr-ontology#hasFireExtinguisherRating">
        <rdfs:domain rdf:resource="https://purl.org/ffdr-ontology#PortableFireExtinguisher"/>
        <rdfs:range rdf:resource="http://www.w3.org/2001/XMLSchema#string"/>
        <rdfs:comment xml:lang="en">The &apos;hasFireExtinguisherRating&apos; data property represents the rating of a given portable fire extinguisher.</rdfs:comment>
        <rdfs:label xml:lang="en">hasFireExtinguisherRating</rdfs:label>
    </owl:DatatypeProperty>
    


    <!-- https://purl.org/ffdr-ontology#hasFireFlow -->


    <owl:DatatypeProperty rdf:about="https://purl.org/ffdr-ontology#hasFireFlow">
        <rdfs:domain>
            <owl:Class>
                <owl:unionOf rdf:parseType="Collection">
                    <rdf:Description rdf:about="https://purl.org/ffdr-ontology#FireHydrant"/>
                    <rdf:Description rdf:about="https://purl.org/ffdr-ontology#WaterSource"/>
                </owl:unionOf>
            </owl:Class>
        </rdfs:domain>
        <rdfs:range rdf:resource="http://www.w3.org/2001/XMLSchema#double"/>
        <rdfs:comment xml:lang="en">The &apos;hasFireFlow&apos; data property represents the flow rate available at 20 psi (the minimum desired pressure) available for firefighting.</rdfs:comment>
        <rdfs:label xml:lang="en">hasFireFlow</rdfs:label>
    </owl:DatatypeProperty>
    


    <!-- https://purl.org/ffdr-ontology#hasFireResistanceRating -->


    <owl:DatatypeProperty rdf:about="https://purl.org/ffdr-ontology#hasFireResistanceRating">
        <rdfs:domain>
            <owl:Class>
                <owl:unionOf rdf:parseType="Collection">
                    <rdf:Description rdf:about="https://purl.org/ffdr-ontology#FireandSmokeProtectionElement"/>
                    <rdf:Description rdf:about="https://purl.org/ffdr-ontology#NonStructuralElement"/>
                    <rdf:Description rdf:about="https://purl.org/ffdr-ontology#StructuralElement"/>
                </owl:unionOf>
            </owl:Class>
        </rdfs:domain>
        <rdfs:range rdf:resource="http://www.w3.org/2001/XMLSchema#double"/>
        <rdfs:comment xml:lang="en">The &apos;hasFireResistanceRating&apos; data property represents the fire-resistance rating of a given element.</rdfs:comment>
        <rdfs:label xml:lang="en">hasFireResistanceRating</rdfs:label>
    </owl:DatatypeProperty>
    


    <!-- https://purl.org/ffdr-ontology#hasFlammabilityLevel -->


    <owl:DatatypeProperty rdf:about="https://purl.org/ffdr-ontology#hasFlammabilityLevel">
        <rdfs:subPropertyOf rdf:resource="https://purl.org/ffdr-ontology#hasHazardLevel"/>
        <rdfs:domain>
            <owl:Class>
                <owl:unionOf rdf:parseType="Collection">
                    <rdf:Description rdf:about="https://purl.org/ffdr-ontology#HazardousMaterial"/>
                    <rdf:Description rdf:about="https://purl.org/ffdr-ontology#HazardousSubstance"/>
                    <rdf:Description rdf:about="https://purl.org/ffdr-ontology#Vegetation"/>
                </owl:unionOf>
            </owl:Class>
        </rdfs:domain>
        <rdfs:range rdf:resource="http://www.w3.org/2001/XMLSchema#int"/>
        <rdfs:comment xml:lang="en">The &apos;hasFlammabilityLevel&apos; data property represents flammable hazard level based on NFPA 704&apos;s hazard communication standard. 

Levels from 0 to 4


0 - Materials that will not burn under typical fire conditions, including intrinsically non-combustible materials such as concrete, stone, and sand.

1 - Materials that must be preheated before ignition can occur. 

Materials in this degree require considerable preheating, under all ambient temperature conditions, before ignition and combustion can occur. Materials in this degree also include finely divided suspended solids that do not require heating before ignition can occur.

2 - Materials that must be moderately heated or exposed to relatively high ambient temperatures before ignition can occur. 

Under normal conditions, these materials would not form hazardous atmospheres with air, but under high ambient temperatures or under moderate heating, they could release vapour in sufficient quantities to produce hazardous atmospheres with air. Materials in this degree also include finely divided suspended solids that do not require heating before ignition can occur.

3 - Liquids and solids (including finely divided suspended solids) that can be ignited under almost all ambient temperature conditions. 

Materials in this degree produce hazardous atmospheres with air under almost all ambient temperatures are readily ignited under almost all conditions.

4 - Materials that rapidly or completely vaporize at atmospheric pressure and normal ambient temperature or that are readily dispersed in air and burn readily.


Source: NFPA 704, 2022</rdfs:comment>
        <rdfs:label xml:lang="en">hasFlammabilityLevel</rdfs:label>
    </owl:DatatypeProperty>
    


    <!-- https://purl.org/ffdr-ontology#hasFloorsServed -->


    <owl:DatatypeProperty rdf:about="https://purl.org/ffdr-ontology#hasFloorsServed">
        <rdfs:subPropertyOf rdf:resource="http://www.w3.org/2002/07/owl#topDataProperty"/>
        <rdfs:domain>
            <owl:Class>
                <owl:unionOf rdf:parseType="Collection">
                    <rdf:Description rdf:about="https://purl.org/ffdr-ontology#Elevator"/>
                    <rdf:Description rdf:about="https://purl.org/ffdr-ontology#Ramp"/>
                    <rdf:Description rdf:about="https://purl.org/ffdr-ontology#Stairway"/>
                </owl:unionOf>
            </owl:Class>
        </rdfs:domain>
        <rdfs:range rdf:resource="http://www.w3.org/2001/XMLSchema#string"/>
        <rdfs:comment xml:lang="en">The &apos;hasFloorsServed&apos; data property represents the floors served by a given stairway, ramp, or elevator.</rdfs:comment>
        <rdfs:label xml:lang="en">hasFloorsServed</rdfs:label>
    </owl:DatatypeProperty>
    


    <!-- https://purl.org/ffdr-ontology#hasHazardLevel -->


    <owl:DatatypeProperty rdf:about="https://purl.org/ffdr-ontology#hasHazardLevel">
        <rdfs:domain>
            <owl:Class>
                <owl:unionOf rdf:parseType="Collection">
                    <rdf:Description rdf:about="https://purl.org/ffdr-ontology#HazardousMaterial"/>
                    <rdf:Description rdf:about="https://purl.org/ffdr-ontology#HazardousSubstance"/>
                    <rdf:Description rdf:about="https://purl.org/ffdr-ontology#Vegetation"/>
                </owl:unionOf>
            </owl:Class>
        </rdfs:domain>
        <rdfs:range>
            <rdfs:Datatype>
                <owl:unionOf rdf:parseType="Collection">
                    <rdf:Description rdf:about="http://www.w3.org/2001/XMLSchema#int"/>
                    <rdf:Description rdf:about="http://www.w3.org/2001/XMLSchema#string"/>
                </owl:unionOf>
            </rdfs:Datatype>
        </rdfs:range>
        <rdfs:comment xml:lang="en">The &apos;hasHazardLevel&apos; data property represents a hazard level based on NFPA 704&apos;s hazard communication standard. 

Levels from 0 to 4

0-least hazardous
4-most hazardous</rdfs:comment>
        <rdfs:label xml:lang="en">hasHazardLevel</rdfs:label>
    </owl:DatatypeProperty>
    


    <!-- https://purl.org/ffdr-ontology#hasHealthHazardSeverityLevel -->


    <owl:DatatypeProperty rdf:about="https://purl.org/ffdr-ontology#hasHealthHazardSeverityLevel">
        <rdfs:subPropertyOf rdf:resource="https://purl.org/ffdr-ontology#hasHazardLevel"/>
        <rdfs:domain>
            <owl:Class>
                <owl:unionOf rdf:parseType="Collection">
                    <rdf:Description rdf:about="https://purl.org/ffdr-ontology#HazardousMaterial"/>
                    <rdf:Description rdf:about="https://purl.org/ffdr-ontology#HazardousSubstance"/>
                </owl:unionOf>
            </owl:Class>
        </rdfs:domain>
        <rdfs:range rdf:resource="http://www.w3.org/2001/XMLSchema#int"/>
        <rdfs:comment xml:lang="en">The &apos;hasHealthHazardSeverityLevel&apos; data property represents the severity of a health hazard based on NFPA 704&apos;s hazard communication standard. 

Levels from 0 to 4

0 - Materials that, under emergency conditions, would offer no hazard beyond that of ordinary combustible materials

1 - Materials that, under emergency conditions, can cause significant irritation

2 - Materials that, under emergency conditions, can cause temporary incapacitation or residual injury

3 - Material that, under emergency conditions, can cause serious or permanent injury

4 - Materials that, under emergency conditions, can be lethal


Source: NFPA 704, 2022</rdfs:comment>
        <rdfs:label xml:lang="en">hasHealthHazardSeverityLevel</rdfs:label>
    </owl:DatatypeProperty>
    


    <!-- https://purl.org/ffdr-ontology#hasHeight -->


    <owl:DatatypeProperty rdf:about="https://purl.org/ffdr-ontology#hasHeight">
        <rdfs:domain rdf:resource="https://purl.org/ffdr-ontology#Window"/>
        <rdfs:range rdf:resource="http://www.w3.org/2001/XMLSchema#double"/>
        <rdfs:comment xml:lang="en">The &apos;hasHeight&apos; data property represents the height of a given element.</rdfs:comment>
        <rdfs:label xml:lang="en">hasHeight</rdfs:label>
    </owl:DatatypeProperty>
    


    <!-- https://purl.org/ffdr-ontology#hasID -->


    <owl:DatatypeProperty rdf:about="https://purl.org/ffdr-ontology#hasID">
        <rdfs:domain rdf:resource="https://purl.org/ffdr-ontology#NonStructuralElement"/>
        <rdfs:range rdf:resource="http://www.w3.org/2001/XMLSchema#string"/>
        <rdfs:comment xml:lang="en">The &apos;hasID&apos; data property represents the ID of a given element.</rdfs:comment>
        <rdfs:label xml:lang="en">hasID</rdfs:label>
    </owl:DatatypeProperty>
    


    <!-- https://purl.org/ffdr-ontology#hasInstabilityLevel -->


    <owl:DatatypeProperty rdf:about="https://purl.org/ffdr-ontology#hasInstabilityLevel">
        <rdfs:subPropertyOf rdf:resource="https://purl.org/ffdr-ontology#hasHazardLevel"/>
        <rdfs:domain>
            <owl:Class>
                <owl:unionOf rdf:parseType="Collection">
                    <rdf:Description rdf:about="https://purl.org/ffdr-ontology#HazardousMaterial"/>
                    <rdf:Description rdf:about="https://purl.org/ffdr-ontology#HazardousSubstance"/>
                </owl:unionOf>
            </owl:Class>
        </rdfs:domain>
        <rdfs:range rdf:resource="http://www.w3.org/2001/XMLSchema#int"/>
        <rdfs:comment xml:lang="en">The &apos;hasInstabilityLevel&apos; data property represents the instability level of a hazard based on NFPA 704&apos;s hazard communication standard. 

Levels from 0 to 4

0 - Materials that in themselves are normally stable, even under fire conditions

1 - Materials that in themselves are normally stable but that can become unstable at elevated temperatures and pressures

2 - Materials that readily undergo a violent chemical change at elevated temperatures and pressures

3 -Materials that in themselves are capable of detonation or explosive decomposition or explosive reaction but that require a strong initiating source or must be heated under confinement before initiation

4 - Materials that in themselves are readily capable of detonation or explosive decomposition or explosive reaction at normal temperatures and pressures.

Source: NFPA 704, 2022</rdfs:comment>
        <rdfs:label xml:lang="en">hasInstabilityLevel</rdfs:label>
    </owl:DatatypeProperty>
    


    <!-- https://purl.org/ffdr-ontology#hasIsolationValveLocation -->


    <owl:DatatypeProperty rdf:about="https://purl.org/ffdr-ontology#hasIsolationValveLocation">
        <rdfs:domain rdf:resource="https://purl.org/ffdr-ontology#StandpipeSystem"/>
        <rdfs:range rdf:resource="http://www.w3.org/2001/XMLSchema#string"/>
        <rdfs:comment xml:lang="en">The &apos;hasIsolationValveLocation&apos; data property represents the location of isolation valves on a standpipe system.</rdfs:comment>
        <rdfs:label xml:lang="en">hasIsolationValveLocation</rdfs:label>
    </owl:DatatypeProperty>
    


    <!-- https://purl.org/ffdr-ontology#hasKey -->


    <owl:DatatypeProperty rdf:about="https://purl.org/ffdr-ontology#hasKey">
        <rdfs:domain rdf:resource="https://purl.org/ffdr-ontology#KeyBox"/>
        <rdfs:range rdf:resource="http://www.w3.org/2001/XMLSchema#string"/>
        <rdfs:comment xml:lang="en">The &apos;hasKey&apos; data property represents the keys found inside a given element.</rdfs:comment>
        <rdfs:label xml:lang="en">hasKey</rdfs:label>
    </owl:DatatypeProperty>
    


    <!-- https://purl.org/ffdr-ontology#hasKeyLocated -->


    <owl:DatatypeProperty rdf:about="https://purl.org/ffdr-ontology#hasKeyLocated">
        <rdfs:domain rdf:resource="https://purl.org/ffdr-ontology#FireCommandCenter"/>
        <rdfs:range rdf:resource="http://www.w3.org/2001/XMLSchema#string"/>
        <rdfs:comment xml:lang="en">The &apos;hasKeyLocated&apos; data property represents the location of the keys to a given room.</rdfs:comment>
        <rdfs:label xml:lang="en">hasKeyLocated</rdfs:label>
    </owl:DatatypeProperty>
    


    <!-- https://purl.org/ffdr-ontology#hasLocation -->


    <owl:DatatypeProperty rdf:about="https://purl.org/ffdr-ontology#hasLocation">
        <rdfs:domain>
            <owl:Class>
                <owl:unionOf rdf:parseType="Collection">
                    <rdf:Description rdf:about="https://purl.org/ffdr-ontology#AirSupply"/>
                    <rdf:Description rdf:about="https://purl.org/ffdr-ontology#AreaOfRefuge"/>
                    <rdf:Description rdf:about="https://purl.org/ffdr-ontology#BuildingPlan"/>
                    <rdf:Description rdf:about="https://purl.org/ffdr-ontology#ConcealedSpace"/>
                    <rdf:Description rdf:about="https://purl.org/ffdr-ontology#ControlPanel"/>
                    <rdf:Description rdf:about="https://purl.org/ffdr-ontology#EmergencyPowerOutlet"/>
                    <rdf:Description rdf:about="https://purl.org/ffdr-ontology#EmergencyServiceProvider"/>
                    <rdf:Description rdf:about="https://purl.org/ffdr-ontology#ExtremelyValuableMaterial"/>
                    <rdf:Description rdf:about="https://purl.org/ffdr-ontology#FarsFillStation"/>
                    <rdf:Description rdf:about="https://purl.org/ffdr-ontology#FireCommandCenter"/>
                    <rdf:Description rdf:about="https://purl.org/ffdr-ontology#FireDepartmentConnection"/>
                    <rdf:Description rdf:about="https://purl.org/ffdr-ontology#FireHoseConnection"/>
                    <rdf:Description rdf:about="https://purl.org/ffdr-ontology#FirePump"/>
                    <rdf:Description rdf:about="https://purl.org/ffdr-ontology#FireandSmokeProtectionElement"/>
                    <rdf:Description rdf:about="https://purl.org/ffdr-ontology#HazardousSubstance"/>
                    <rdf:Description rdf:about="https://purl.org/ffdr-ontology#Helipad"/>
                    <rdf:Description rdf:about="https://purl.org/ffdr-ontology#KeyBox"/>
                    <rdf:Description rdf:about="https://purl.org/ffdr-ontology#NonStructuralElement"/>
                    <rdf:Description rdf:about="https://purl.org/ffdr-ontology#PortableFireExtinguisher"/>
                    <rdf:Description rdf:about="https://purl.org/ffdr-ontology#RoofTopElement"/>
                    <rdf:Description rdf:about="https://purl.org/ffdr-ontology#SmokeandHeatRemovalSystem"/>
                    <rdf:Description rdf:about="https://purl.org/ffdr-ontology#StaticWaterSource"/>
                    <rdf:Description rdf:about="https://purl.org/ffdr-ontology#StructuralElement"/>
                    <rdf:Description rdf:about="https://purl.org/ffdr-ontology#SurroundingStructure"/>
                    <rdf:Description rdf:about="https://purl.org/ffdr-ontology#VerticalOpening"/>
                </owl:unionOf>
            </owl:Class>
        </rdfs:domain>
        <rdfs:range rdf:resource="http://www.w3.org/2001/XMLSchema#string"/>
        <rdfs:comment xml:lang="en">The &apos;hasLocation&apos; data property represents the location of a given element or area.</rdfs:comment>
        <rdfs:label xml:lang="en">hasLocation</rdfs:label>
    </owl:DatatypeProperty>
    


    <!-- https://purl.org/ffdr-ontology#hasLocationOfControlValve -->


    <owl:DatatypeProperty rdf:about="https://purl.org/ffdr-ontology#hasLocationOfControlValve">
        <rdfs:domain rdf:resource="https://purl.org/ffdr-ontology#AutomaticFireExtinguishingSystem"/>
        <rdfs:range rdf:resource="http://www.w3.org/2001/XMLSchema#string"/>
        <rdfs:comment xml:lang="en">The &apos;hasLocationOfControlValve&apos; data property represents the location of the control valves of a given system.</rdfs:comment>
        <rdfs:label xml:lang="en">hasLocationOfControlValve</rdfs:label>
    </owl:DatatypeProperty>
    


    <!-- https://purl.org/ffdr-ontology#hasMachineRoomLocation -->


    <owl:DatatypeProperty rdf:about="https://purl.org/ffdr-ontology#hasMachineRoomLocation">
        <rdfs:domain rdf:resource="https://purl.org/ffdr-ontology#Elevator"/>
        <rdfs:range rdf:resource="http://www.w3.org/2001/XMLSchema#string"/>
        <rdfs:comment xml:lang="en">The &apos;hasMachineRoomLocation&apos; data property represents the location of the machine room of a given elevator system.</rdfs:comment>
        <rdfs:label xml:lang="en">hasMachineRoomLocation</rdfs:label>
    </owl:DatatypeProperty>
    


    <!-- https://purl.org/ffdr-ontology#hasNumberOfExit -->


    <owl:DatatypeProperty rdf:about="https://purl.org/ffdr-ontology#hasNumberOfExit">
        <rdfs:domain rdf:resource="https://purl.org/ffdr-ontology#IncidentBuilding"/>
        <rdfs:range rdf:resource="http://www.w3.org/2001/XMLSchema#int"/>
        <rdfs:comment xml:lang="en">The &apos;hasNumberOfExit&apos; data property represents the number of exits a given building has.</rdfs:comment>
        <rdfs:label xml:lang="en">hasNumberOfExit</rdfs:label>
    </owl:DatatypeProperty>
    


    <!-- https://purl.org/ffdr-ontology#hasNumberOfInlet -->


    <owl:DatatypeProperty rdf:about="https://purl.org/ffdr-ontology#hasNumberOfInlet">
        <rdfs:domain rdf:resource="https://purl.org/ffdr-ontology#FireDepartmentConnection"/>
        <rdfs:range rdf:resource="http://www.w3.org/2001/XMLSchema#int"/>
        <rdfs:comment xml:lang="en">The &apos;hasNumberOfInlet&apos; data property represents the number of inlets a given connection has.</rdfs:comment>
        <rdfs:label xml:lang="en">hasNumberOfInlet</rdfs:label>
    </owl:DatatypeProperty>
    


    <!-- https://purl.org/ffdr-ontology#hasNumberOfOutlet -->


    <owl:DatatypeProperty rdf:about="https://purl.org/ffdr-ontology#hasNumberOfOutlet">
        <rdfs:domain rdf:resource="https://purl.org/ffdr-ontology#FireHydrant"/>
        <rdfs:range rdf:resource="http://www.w3.org/2001/XMLSchema#int"/>
        <rdfs:comment xml:lang="en">The &apos;hasNumberOfOutlet&apos; data property represents the number of outlets a given connection has.</rdfs:comment>
        <rdfs:label xml:lang="en">hasNumberOfOutlet</rdfs:label>
    </owl:DatatypeProperty>
    


    <!-- https://purl.org/ffdr-ontology#hasNumberOfSimultaneousFill -->


    <owl:DatatypeProperty rdf:about="https://purl.org/ffdr-ontology#hasNumberOfSimultaneousFill">
        <rdfs:domain rdf:resource="https://purl.org/ffdr-ontology#FarsFillStation"/>
        <rdfs:range rdf:resource="http://www.w3.org/2001/XMLSchema#int"/>
        <rdfs:comment xml:lang="en">The &apos;hasNumberOfSimultaneousFill&apos; data property represents the number of simultaneous fills provided by a given fill station or panel.</rdfs:comment>
        <rdfs:label xml:lang="en">hasNumberOfSimultaneousFill</rdfs:label>
    </owl:DatatypeProperty>
    


    <!-- https://purl.org/ffdr-ontology#hasNumberOfStory -->


    <owl:DatatypeProperty rdf:about="https://purl.org/ffdr-ontology#hasNumberOfStory">
        <rdfs:domain rdf:resource="https://purl.org/ffdr-ontology#IncidentBuilding"/>
        <rdfs:range rdf:resource="http://www.w3.org/2001/XMLSchema#int"/>
        <rdfs:comment xml:lang="en">The &apos;hasNumberOfStory&apos; data property represents the number of stories in a building.</rdfs:comment>
        <rdfs:label xml:lang="en">hasNumberOfStory</rdfs:label>
    </owl:DatatypeProperty>
    


    <!-- https://purl.org/ffdr-ontology#hasNumberOfSublevel -->


    <owl:DatatypeProperty rdf:about="https://purl.org/ffdr-ontology#hasNumberOfSublevel">
        <rdfs:domain rdf:resource="https://purl.org/ffdr-ontology#IncidentBuilding"/>
        <rdfs:range rdf:resource="http://www.w3.org/2001/XMLSchema#int"/>
        <rdfs:comment xml:lang="en">The &apos;hasNumberOfSublevel&apos; data property represents the number of sublevels in a building.</rdfs:comment>
        <rdfs:label xml:lang="en">hasNumberOfSublevel</rdfs:label>
    </owl:DatatypeProperty>
    


    <!-- https://purl.org/ffdr-ontology#hasOccupantLoad -->


    <owl:DatatypeProperty rdf:about="https://purl.org/ffdr-ontology#hasOccupantLoad">
        <rdfs:domain rdf:resource="https://purl.org/ffdr-ontology#IncidentBuilding"/>
        <rdfs:range rdf:resource="http://www.w3.org/2001/XMLSchema#int"/>
        <rdfs:comment xml:lang="en">The &apos;hasOccupantLoad&apos; data property represents the occupant load of a building.</rdfs:comment>
        <rdfs:label xml:lang="en">hasOccupantLoad</rdfs:label>
    </owl:DatatypeProperty>
    


    <!-- https://purl.org/ffdr-ontology#hasOpeningDirection -->


    <owl:DatatypeProperty rdf:about="https://purl.org/ffdr-ontology#hasOpeningDirection">
        <rdfs:domain>
            <owl:Class>
                <owl:unionOf rdf:parseType="Collection">
                    <rdf:Description rdf:about="https://purl.org/ffdr-ontology#Door"/>
                    <rdf:Description rdf:about="https://purl.org/ffdr-ontology#Window"/>
                </owl:unionOf>
            </owl:Class>
        </rdfs:domain>
        <rdfs:range rdf:resource="http://www.w3.org/2001/XMLSchema#string"/>
        <rdfs:comment xml:lang="en">The &apos;hasOpeningDirection&apos; data property represents the opening direction of a given door or window.</rdfs:comment>
        <rdfs:label xml:lang="en">hasOpeningDirection</rdfs:label>
    </owl:DatatypeProperty>
    


    <!-- https://purl.org/ffdr-ontology#hasPrecipitationValue -->


    <owl:DatatypeProperty rdf:about="https://purl.org/ffdr-ontology#hasPrecipitationValue">
        <rdfs:domain rdf:resource="https://purl.org/ffdr-ontology#WeatherCondition"/>
        <rdfs:range rdf:resource="http://www.w3.org/2001/XMLSchema#double"/>
        <rdfs:comment xml:lang="en">The &apos;hasPrecipitationValue&apos; data property represents precipitation value (drizzling, rain, sleet, snow, ice pellets, graupel, or hail) at a given time.</rdfs:comment>
        <rdfs:label xml:lang="en">hasPrecipitationValue</rdfs:label>
    </owl:DatatypeProperty>
    


    <!-- https://purl.org/ffdr-ontology#hasPressure -->


    <owl:DatatypeProperty rdf:about="https://purl.org/ffdr-ontology#hasPressure">
        <rdfs:domain rdf:resource="https://purl.org/ffdr-ontology#MunicipalDistributionSystem"/>
        <rdfs:range rdf:resource="http://www.w3.org/2001/XMLSchema#double"/>
        <rdfs:comment xml:lang="en">The &apos;hasPressure&apos; data property represents the pressure of a given system.</rdfs:comment>
        <rdfs:label xml:lang="en">hasPressure</rdfs:label>
    </owl:DatatypeProperty>
    


    <!-- https://purl.org/ffdr-ontology#hasRelativeHumidity -->


    <owl:DatatypeProperty rdf:about="https://purl.org/ffdr-ontology#hasRelativeHumidity">
        <rdfs:domain rdf:resource="https://purl.org/ffdr-ontology#WeatherCondition"/>
        <rdfs:range rdf:resource="http://www.w3.org/2001/XMLSchema#double"/>
        <rdfs:comment xml:lang="en">The &apos;hasRelativeHumidity&apos; data property represents the relative humidity at a given time.</rdfs:comment>
        <rdfs:label xml:lang="en">hasRelativeHumidity</rdfs:label>
    </owl:DatatypeProperty>
    


    <!-- https://purl.org/ffdr-ontology#hasRequiredMaximumPressure -->


    <owl:DatatypeProperty rdf:about="https://purl.org/ffdr-ontology#hasRequiredMaximumPressure">
        <rdfs:domain>
            <owl:Class>
                <owl:unionOf rdf:parseType="Collection">
                    <rdf:Description rdf:about="https://purl.org/ffdr-ontology#AutomaticSprinklerSystem"/>
                    <rdf:Description rdf:about="https://purl.org/ffdr-ontology#StandpipeSystem"/>
                </owl:unionOf>
            </owl:Class>
        </rdfs:domain>
        <rdfs:range rdf:resource="http://www.w3.org/2001/XMLSchema#double"/>
        <rdfs:comment xml:lang="en">The &apos;hasRequiredMaximumPressure&apos; data property represents the maximum pressure required by a given system.</rdfs:comment>
        <rdfs:label xml:lang="en">hasRequiredMaximumPressure</rdfs:label>
    </owl:DatatypeProperty>
    


    <!-- https://purl.org/ffdr-ontology#hasRequiredMinimumPressure -->


    <owl:DatatypeProperty rdf:about="https://purl.org/ffdr-ontology#hasRequiredMinimumPressure">
        <rdfs:domain>
            <owl:Class>
                <owl:unionOf rdf:parseType="Collection">
                    <rdf:Description rdf:about="https://purl.org/ffdr-ontology#AutomaticSprinklerSystem"/>
                    <rdf:Description rdf:about="https://purl.org/ffdr-ontology#StandpipeSystem"/>
                </owl:unionOf>
            </owl:Class>
        </rdfs:domain>
        <rdfs:range rdf:resource="http://www.w3.org/2001/XMLSchema#double"/>
        <rdfs:comment xml:lang="en">The &apos;hasRequiredMinimumPressure&apos; data property represents the minimum pressure required by a given system.</rdfs:comment>
        <rdfs:label xml:lang="en">hasRequiredMinimumPressure</rdfs:label>
    </owl:DatatypeProperty>
    


    <!-- https://purl.org/ffdr-ontology#hasSize -->


    <owl:DatatypeProperty rdf:about="https://purl.org/ffdr-ontology#hasSize">
        <rdfs:domain rdf:resource="https://purl.org/ffdr-ontology#HoseConnection"/>
        <rdfs:range rdf:resource="http://www.w3.org/2001/XMLSchema#double"/>
        <rdfs:comment xml:lang="en">The &apos;hasSize&apos; data property represents the size of a given element.</rdfs:comment>
        <rdfs:label xml:lang="en">hasSize</rdfs:label>
    </owl:DatatypeProperty>
    


    <!-- https://purl.org/ffdr-ontology#hasSlope -->


    <owl:DatatypeProperty rdf:about="https://purl.org/ffdr-ontology#hasSlope">
        <rdfs:domain>
            <owl:Class>
                <owl:unionOf rdf:parseType="Collection">
                    <rdf:Description rdf:about="https://purl.org/ffdr-ontology#Road"/>
                    <rdf:Description rdf:about="https://purl.org/ffdr-ontology#SurroundingTerrain"/>
                </owl:unionOf>
            </owl:Class>
        </rdfs:domain>
        <rdfs:range rdf:resource="http://www.w3.org/2001/XMLSchema#double"/>
        <rdfs:comment xml:lang="en">The &apos;hasSlope&apos; data property represents the slope of a given terrain.</rdfs:comment>
        <rdfs:label xml:lang="en">hasSlope</rdfs:label>
    </owl:DatatypeProperty>
    


    <!-- https://purl.org/ffdr-ontology#hasSpecialHazard -->


    <owl:DatatypeProperty rdf:about="https://purl.org/ffdr-ontology#hasSpecialHazard">
        <rdfs:subPropertyOf rdf:resource="http://www.w3.org/2002/07/owl#topDataProperty"/>
        <rdfs:domain>
            <owl:Class>
                <owl:unionOf rdf:parseType="Collection">
                    <rdf:Description rdf:about="https://purl.org/ffdr-ontology#HazardousMaterial"/>
                    <rdf:Description rdf:about="https://purl.org/ffdr-ontology#HazardousSubstance"/>
                </owl:unionOf>
            </owl:Class>
        </rdfs:domain>
        <rdfs:range rdf:resource="http://www.w3.org/2001/XMLSchema#string"/>
        <rdfs:comment xml:lang="en">The &apos;hasSpecialHazard&apos; data property represents a special type of hazard based on NFPA 704&apos;s hazard communication standard.</rdfs:comment>
        <rdfs:label xml:lang="en">hasSpecialHazard</rdfs:label>
    </owl:DatatypeProperty>
    


    <!-- https://purl.org/ffdr-ontology#hasSpecies -->


    <owl:DatatypeProperty rdf:about="https://purl.org/ffdr-ontology#hasSpecies">
        <rdfs:domain rdf:resource="https://purl.org/ffdr-ontology#Vegetation"/>
        <rdfs:range rdf:resource="http://www.w3.org/2001/XMLSchema#string"/>
        <rdfs:comment xml:lang="en">The &apos;hasSpecies&apos; data property represents the species of given vegetation.</rdfs:comment>
        <rdfs:label xml:lang="en">hasSpecies</rdfs:label>
    </owl:DatatypeProperty>
    


    <!-- https://purl.org/ffdr-ontology#hasStatus -->


    <owl:DatatypeProperty rdf:about="https://purl.org/ffdr-ontology#hasStatus">
        <rdfs:domain rdf:resource="https://purl.org/ffdr-ontology#Road"/>
        <rdfs:range rdf:resource="http://www.w3.org/2001/XMLSchema#string"/>
        <rdfs:comment xml:lang="en">The &apos;hasStatus&apos; data property represents the status of a given structure.</rdfs:comment>
        <rdfs:label xml:lang="en">hasStatus</rdfs:label>
    </owl:DatatypeProperty>
    


    <!-- https://purl.org/ffdr-ontology#hasTemperature -->


    <owl:DatatypeProperty rdf:about="https://purl.org/ffdr-ontology#hasTemperature">
        <rdfs:domain rdf:resource="https://purl.org/ffdr-ontology#WeatherCondition"/>
        <rdfs:range rdf:resource="http://www.w3.org/2001/XMLSchema#double"/>
        <rdfs:comment xml:lang="en">The &apos;hasTemperature&apos; data property represents the temperature at a given time.</rdfs:comment>
        <rdfs:label xml:lang="en">hasTemperature</rdfs:label>
    </owl:DatatypeProperty>
    


    <!-- https://purl.org/ffdr-ontology#hasThickness -->


    <owl:DatatypeProperty rdf:about="https://purl.org/ffdr-ontology#hasThickness">
        <rdfs:domain rdf:resource="https://purl.org/ffdr-ontology#Wall"/>
        <rdfs:range rdf:resource="http://www.w3.org/2001/XMLSchema#double"/>
        <rdfs:comment xml:lang="en">The &apos;hasThickness&apos; data property represents the thickness of a given element.</rdfs:comment>
        <rdfs:label xml:lang="en">hasThickness</rdfs:label>
    </owl:DatatypeProperty>
    


    <!-- https://purl.org/ffdr-ontology#hasTimeMark -->


    <owl:DatatypeProperty rdf:about="https://purl.org/ffdr-ontology#hasTimeMark">
        <rdfs:domain rdf:resource="https://purl.org/ffdr-ontology#WeatherCondition"/>
        <rdfs:range rdf:resource="http://www.w3.org/2001/XMLSchema#dateTimeStamp"/>
        <rdfs:comment xml:lang="en">The &apos;hasTimeMark&apos; data property represents a specific time.</rdfs:comment>
        <rdfs:label xml:lang="en">hasTimeMark</rdfs:label>
    </owl:DatatypeProperty>
    


    <!-- https://purl.org/ffdr-ontology#hasTrafficLevel -->


    <owl:DatatypeProperty rdf:about="https://purl.org/ffdr-ontology#hasTrafficLevel">
        <rdfs:domain rdf:resource="https://purl.org/ffdr-ontology#RoadToIncident"/>
        <rdfs:range rdf:resource="http://www.w3.org/2001/XMLSchema#string"/>
        <rdfs:comment xml:lang="en">The &apos;hasTrafficLevel&apos; data property represents the traffic level on a given road</rdfs:comment>
        <rdfs:label xml:lang="en">hasTrafficLevel</rdfs:label>
    </owl:DatatypeProperty>
    


    <!-- https://purl.org/ffdr-ontology#hasTurningRadius -->


    <owl:DatatypeProperty rdf:about="https://purl.org/ffdr-ontology#hasTurningRadius">
        <rdfs:domain rdf:resource="https://purl.org/ffdr-ontology#FireLane"/>
        <rdfs:range rdf:resource="http://www.w3.org/2001/XMLSchema#double"/>
        <rdfs:comment xml:lang="en">The &apos;hasTurningRadius&apos; data property represents the inside or outside turning radius of a given road.</rdfs:comment>
        <rdfs:label xml:lang="en">hasTurningRadius</rdfs:label>
    </owl:DatatypeProperty>
    


    <!-- https://purl.org/ffdr-ontology#hasType -->


    <owl:DatatypeProperty rdf:about="https://purl.org/ffdr-ontology#hasType">
        <rdfs:domain>
            <owl:Class>
                <owl:unionOf rdf:parseType="Collection">
                    <rdf:Description rdf:about="https://purl.org/ffdr-ontology#AirSupply"/>
                    <rdf:Description rdf:about="https://purl.org/ffdr-ontology#BuildingPlan"/>
                    <rdf:Description rdf:about="https://purl.org/ffdr-ontology#ConstructionType"/>
                    <rdf:Description rdf:about="https://purl.org/ffdr-ontology#EmergencyPowerOutlet"/>
                    <rdf:Description rdf:about="https://purl.org/ffdr-ontology#FireHydrant"/>
                    <rdf:Description rdf:about="https://purl.org/ffdr-ontology#HoseConnection"/>
                    <rdf:Description rdf:about="https://purl.org/ffdr-ontology#MassNotificationSystem"/>
                    <rdf:Description rdf:about="https://purl.org/ffdr-ontology#Obstruction"/>
                    <rdf:Description rdf:about="https://purl.org/ffdr-ontology#PortableFireExtinguisher"/>
                    <rdf:Description rdf:about="https://purl.org/ffdr-ontology#Road"/>
                    <rdf:Description rdf:about="https://purl.org/ffdr-ontology#RoofTopElement"/>
                    <rdf:Description rdf:about="https://purl.org/ffdr-ontology#SmokeControlSystem"/>
                    <rdf:Description rdf:about="https://purl.org/ffdr-ontology#SmokeandHeatRemovalSystem"/>
                    <rdf:Description rdf:about="https://purl.org/ffdr-ontology#StandpipeSystem"/>
                    <rdf:Description rdf:about="https://purl.org/ffdr-ontology#StaticWaterSource"/>
                </owl:unionOf>
            </owl:Class>
        </rdfs:domain>
        <rdfs:range rdf:resource="http://www.w3.org/2001/XMLSchema#string"/>
        <rdfs:comment xml:lang="en">The &apos;hasType&apos; data property represents a type.</rdfs:comment>
        <rdfs:label xml:lang="en">hasType</rdfs:label>
    </owl:DatatypeProperty>
    


    <!-- https://purl.org/ffdr-ontology#hasTypeOfSignalInitiator -->


    <owl:DatatypeProperty rdf:about="https://purl.org/ffdr-ontology#hasTypeOfSignalInitiator">
        <rdfs:domain rdf:resource="https://purl.org/ffdr-ontology#FireAlarmSystem"/>
        <rdfs:range rdf:resource="http://www.w3.org/2001/XMLSchema#string"/>
        <rdfs:comment xml:lang="en">Possible types of alarm signal initiator:

- Manual pull stations,
- Sprinkler flow detectors,
- Smoke detector
- Heat detectors
- Flame detectors
- Optical detectors</rdfs:comment>
        <rdfs:comment xml:lang="en">The &apos;hasTypeOfSignalInitiator&apos; data property represents the type of alarm signal initiator.</rdfs:comment>
        <rdfs:label xml:lang="en">hasTypeOfSignalInitiator</rdfs:label>
    </owl:DatatypeProperty>
    


    <!-- https://purl.org/ffdr-ontology#hasVerticalClearance -->


    <owl:DatatypeProperty rdf:about="https://purl.org/ffdr-ontology#hasVerticalClearance">
        <rdfs:domain rdf:resource="https://purl.org/ffdr-ontology#FireLane"/>
        <rdfs:range rdf:resource="http://www.w3.org/2001/XMLSchema#double"/>
        <rdfs:comment xml:lang="en">The &apos;hasVerticalClearance&apos; data property represents the vertical clearance of a given road.</rdfs:comment>
        <rdfs:label xml:lang="en">hasVerticalClearance</rdfs:label>
    </owl:DatatypeProperty>
    


    <!-- https://purl.org/ffdr-ontology#hasWidth -->


    <owl:DatatypeProperty rdf:about="https://purl.org/ffdr-ontology#hasWidth">
        <rdfs:domain>
            <owl:Class>
                <owl:unionOf rdf:parseType="Collection">
                    <rdf:Description rdf:about="https://purl.org/ffdr-ontology#Balcony"/>
                    <rdf:Description rdf:about="https://purl.org/ffdr-ontology#Door"/>
                    <rdf:Description rdf:about="https://purl.org/ffdr-ontology#Hallway"/>
                    <rdf:Description rdf:about="https://purl.org/ffdr-ontology#Ramp"/>
                    <rdf:Description rdf:about="https://purl.org/ffdr-ontology#Road"/>
                    <rdf:Description rdf:about="https://purl.org/ffdr-ontology#Stairway"/>
                    <rdf:Description rdf:about="https://purl.org/ffdr-ontology#Window"/>
                </owl:unionOf>
            </owl:Class>
        </rdfs:domain>
        <rdfs:range rdf:resource="http://www.w3.org/2001/XMLSchema#double"/>
        <rdfs:comment xml:lang="en">The &apos;hasWidth&apos; data property represents width.</rdfs:comment>
        <rdfs:label xml:lang="en">hasWidth</rdfs:label>
    </owl:DatatypeProperty>
    


    <!-- https://purl.org/ffdr-ontology#hasWindDirection -->


    <owl:DatatypeProperty rdf:about="https://purl.org/ffdr-ontology#hasWindDirection">
        <rdfs:domain rdf:resource="https://purl.org/ffdr-ontology#WeatherCondition"/>
        <rdfs:range rdf:resource="http://www.w3.org/2001/XMLSchema#string"/>
        <rdfs:comment xml:lang="en">The &apos;hasWindDirection&apos; data property represents wind direction at a given time.</rdfs:comment>
        <rdfs:label xml:lang="en">hasWindDirection</rdfs:label>
    </owl:DatatypeProperty>
    


    <!-- https://purl.org/ffdr-ontology#hasWindSpeed -->


    <owl:DatatypeProperty rdf:about="https://purl.org/ffdr-ontology#hasWindSpeed">
        <rdfs:domain rdf:resource="https://purl.org/ffdr-ontology#WeatherCondition"/>
        <rdfs:range rdf:resource="http://www.w3.org/2001/XMLSchema#double"/>
        <rdfs:comment xml:lang="en">The &apos;hasWindSpeed&apos; data property represents wind speed at a given time.</rdfs:comment>
        <rdfs:label xml:lang="en">hasWindSpeed</rdfs:label>
    </owl:DatatypeProperty>
    


    <!-- https://purl.org/ffdr-ontology#includeHazardousOperation -->


    <owl:DatatypeProperty rdf:about="https://purl.org/ffdr-ontology#includeHazardousOperation">
        <rdfs:domain rdf:resource="https://purl.org/ffdr-ontology#IncidentBuilding"/>
        <rdfs:range rdf:resource="http://www.w3.org/2001/XMLSchema#boolean"/>
        <rdfs:comment xml:lang="en">The &apos;includeHazardousOperation&apos; data property represents hazardous operations taking place in a given building.</rdfs:comment>
        <rdfs:label xml:lang="en">includeHazardousOperation</rdfs:label>
    </owl:DatatypeProperty>
    


    <!-- https://purl.org/ffdr-ontology#isAbandoned -->


    <owl:DatatypeProperty rdf:about="https://purl.org/ffdr-ontology#isAbandoned">
        <rdfs:domain rdf:resource="https://purl.org/ffdr-ontology#BuildingOccupancy"/>
        <rdfs:range rdf:resource="http://www.w3.org/2001/XMLSchema#boolean"/>
        <rdfs:comment xml:lang="en">The &apos;isAbandoned&apos; data property checks whether a given building is abandoned or not.</rdfs:comment>
        <rdfs:label xml:lang="en">isAbandoned</rdfs:label>
    </owl:DatatypeProperty>
    


    <!-- https://purl.org/ffdr-ontology#isAccessible -->


    <owl:DatatypeProperty rdf:about="https://purl.org/ffdr-ontology#isAccessible">
        <rdfs:domain rdf:resource="https://purl.org/ffdr-ontology#RoofAssembly"/>
        <rdfs:range rdf:resource="http://www.w3.org/2001/XMLSchema#boolean"/>
        <rdfs:comment xml:lang="en">The &apos;isAccessible&apos; data property checks whether a given area is accessible or not.</rdfs:comment>
        <rdfs:label xml:lang="en">isAccessible</rdfs:label>
    </owl:DatatypeProperty>
    


    <!-- https://purl.org/ffdr-ontology#isControlValveOn -->


    <owl:DatatypeProperty rdf:about="https://purl.org/ffdr-ontology#isControlValveOn">
        <rdfs:domain rdf:resource="https://purl.org/ffdr-ontology#AutomaticSprinklerSystem"/>
        <rdfs:range rdf:resource="http://www.w3.org/2001/XMLSchema#boolean"/>
        <rdfs:comment xml:lang="en">The &apos;isControlValveOn&apos; data property checks whether the control valve of a given system is turned on or not.</rdfs:comment>
        <rdfs:label xml:lang="en">isControlValveOn</rdfs:label>
    </owl:DatatypeProperty>
    


    <!-- https://purl.org/ffdr-ontology#isDecontaminationRequired -->


    <owl:DatatypeProperty rdf:about="https://purl.org/ffdr-ontology#isDecontaminationRequired">
        <rdfs:domain rdf:resource="https://purl.org/ffdr-ontology#HazardousSubstance"/>
        <rdfs:range rdf:resource="http://www.w3.org/2001/XMLSchema#boolean"/>
        <rdfs:comment xml:lang="en">The &apos;isDecontaminationRequired&apos; data property checks whether decontamination is required or not.</rdfs:comment>
        <rdfs:label xml:lang="en">isDecontaminationRequired</rdfs:label>
    </owl:DatatypeProperty>
    


    <!-- https://purl.org/ffdr-ontology#isExit -->


    <owl:DatatypeProperty rdf:about="https://purl.org/ffdr-ontology#isExit">
        <rdfs:domain>
            <owl:Class>
                <owl:unionOf rdf:parseType="Collection">
                    <rdf:Description rdf:about="https://purl.org/ffdr-ontology#Door"/>
                    <rdf:Description rdf:about="https://purl.org/ffdr-ontology#Ramp"/>
                    <rdf:Description rdf:about="https://purl.org/ffdr-ontology#Stairway"/>
                </owl:unionOf>
            </owl:Class>
        </rdfs:domain>
        <rdfs:range rdf:resource="http://www.w3.org/2001/XMLSchema#boolean"/>
        <rdfs:comment xml:lang="en">The &apos;isExit&apos; data property checks whether a given element is an exit or not.</rdfs:comment>
        <rdfs:label xml:lang="en">isExit</rdfs:label>
    </owl:DatatypeProperty>
    


    <!-- https://purl.org/ffdr-ontology#isFunctional -->


    <owl:DatatypeProperty rdf:about="https://purl.org/ffdr-ontology#isFunctional">
        <rdfs:domain>
            <owl:Class>
                <owl:unionOf rdf:parseType="Collection">
                    <rdf:Description rdf:about="https://purl.org/ffdr-ontology#Door"/>
                    <rdf:Description rdf:about="https://purl.org/ffdr-ontology#Elevator"/>
                    <rdf:Description rdf:about="https://purl.org/ffdr-ontology#FireHydrant"/>
                    <rdf:Description rdf:about="https://purl.org/ffdr-ontology#WaterSource"/>
                    <rdf:Description rdf:about="https://purl.org/ffdr-ontology#Window"/>
                </owl:unionOf>
            </owl:Class>
        </rdfs:domain>
        <rdfs:range rdf:resource="http://www.w3.org/2001/XMLSchema#boolean"/>
        <rdfs:comment xml:lang="en">The &apos;isFunctional&apos; data property checks whether a given element or system is functional or not.</rdfs:comment>
        <rdfs:label xml:lang="en">isFunctional</rdfs:label>
    </owl:DatatypeProperty>
    


    <!-- https://purl.org/ffdr-ontology#isInAlarm -->


    <owl:DatatypeProperty rdf:about="https://purl.org/ffdr-ontology#isInAlarm">
        <rdfs:domain rdf:resource="https://purl.org/ffdr-ontology#SensorDetector"/>
        <rdfs:range rdf:resource="http://www.w3.org/2001/XMLSchema#boolean"/>
        <rdfs:comment xml:lang="en">The &apos;isInAlarm&apos; data property checks whether a given element&apos;s or system&apos;s alarm is activated or not.</rdfs:comment>
        <rdfs:label xml:lang="en">isInAlarm</rdfs:label>
    </owl:DatatypeProperty>
    


    <!-- https://purl.org/ffdr-ontology#isIsolationValveOpen -->


    <owl:DatatypeProperty rdf:about="https://purl.org/ffdr-ontology#isIsolationValveOpen">
        <rdfs:domain rdf:resource="https://purl.org/ffdr-ontology#StandpipeSystem"/>
        <rdfs:range rdf:resource="http://www.w3.org/2001/XMLSchema#boolean"/>
        <rdfs:comment xml:lang="en">The &apos;isIsolationValveOpen&apos; data property checks whether the isolation valve of a given element or system is open or not.</rdfs:comment>
        <rdfs:label xml:lang="en">isIsolationValveOpen</rdfs:label>
    </owl:DatatypeProperty>
    


    <!-- https://purl.org/ffdr-ontology#isLightweightConstruction -->


    <owl:DatatypeProperty rdf:about="https://purl.org/ffdr-ontology#isLightweightConstruction">
        <rdfs:domain>
            <owl:Class>
                <owl:unionOf rdf:parseType="Collection">
                    <rdf:Description rdf:about="https://purl.org/ffdr-ontology#FloorAssembly"/>
                    <rdf:Description rdf:about="https://purl.org/ffdr-ontology#RoofAssembly"/>
                </owl:unionOf>
            </owl:Class>
        </rdfs:domain>
        <rdfs:range rdf:resource="http://www.w3.org/2001/XMLSchema#boolean"/>
        <rdfs:comment xml:lang="en">The &apos;isLightweightConstruction&apos; data property checks whether a given assembly is made of lightweight construction or not.</rdfs:comment>
        <rdfs:label xml:lang="en">isLightweightConstruction</rdfs:label>
    </owl:DatatypeProperty>
    


    <!-- https://purl.org/ffdr-ontology#isOnExterior -->


    <owl:DatatypeProperty rdf:about="https://purl.org/ffdr-ontology#isOnExterior">
        <rdfs:domain>
            <owl:Class>
                <owl:unionOf rdf:parseType="Collection">
                    <rdf:Description rdf:about="https://purl.org/ffdr-ontology#ExteriorWall"/>
                    <rdf:Description rdf:about="https://purl.org/ffdr-ontology#ExteriorWindow"/>
                    <rdf:Description rdf:about="https://purl.org/ffdr-ontology#Window"/>
                </owl:unionOf>
            </owl:Class>
        </rdfs:domain>
        <rdfs:range rdf:resource="http://www.w3.org/2001/XMLSchema#boolean"/>
        <rdfs:comment xml:lang="en">The &apos;isOnExterior&apos; data property checks whether a given element is on the exterior of a building or not.</rdfs:comment>
        <rdfs:label xml:lang="en">isOnExterior</rdfs:label>
    </owl:DatatypeProperty>
    


    <!-- https://purl.org/ffdr-ontology#isPrimaryFireServiceEntryPoint -->


    <owl:DatatypeProperty rdf:about="https://purl.org/ffdr-ontology#isPrimaryFireServiceEntryPoint">
        <rdfs:domain rdf:resource="https://purl.org/ffdr-ontology#Door"/>
        <rdfs:range rdf:resource="http://www.w3.org/2001/XMLSchema#boolean"/>
        <rdfs:comment xml:lang="en">The &apos;isPrimaryFireServiceEntryPoint&apos; data property checks whether a given entry is the primary fire service entry point or not.</rdfs:comment>
        <rdfs:label xml:lang="en">isPrimaryFireServiceEntryPoint</rdfs:label>
    </owl:DatatypeProperty>
    


    <!-- https://purl.org/ffdr-ontology#isQualifiedForEvacuation -->


    <owl:DatatypeProperty rdf:about="https://purl.org/ffdr-ontology#isQualifiedForEvacuation">
        <rdfs:domain rdf:resource="https://purl.org/ffdr-ontology#Elevator"/>
        <rdfs:range rdf:resource="http://www.w3.org/2001/XMLSchema#boolean"/>
        <rdfs:comment xml:lang="en">The &apos;isQualifiedForEvacuation&apos; data property checks whether an element or system can be used for evacuation or not.</rdfs:comment>
        <rdfs:label xml:lang="en">isQualifiedForEvacuation</rdfs:label>
    </owl:DatatypeProperty>
    


    <!-- https://purl.org/ffdr-ontology#isRoofAccess -->


    <owl:DatatypeProperty rdf:about="https://purl.org/ffdr-ontology#isRoofAccess">
        <rdfs:domain>
            <owl:Class>
                <owl:unionOf rdf:parseType="Collection">
                    <rdf:Description rdf:about="https://purl.org/ffdr-ontology#Ramp"/>
                    <rdf:Description rdf:about="https://purl.org/ffdr-ontology#Stairway"/>
                </owl:unionOf>
            </owl:Class>
        </rdfs:domain>
        <rdfs:range rdf:resource="http://www.w3.org/2001/XMLSchema#boolean"/>
        <rdfs:comment xml:lang="en">The &apos;isRoofAccess&apos; data property checks whether a given element or system can provide access to a roof or not.</rdfs:comment>
        <rdfs:label xml:lang="en">isRoofAccess</rdfs:label>
    </owl:DatatypeProperty>
    


    <!-- https://purl.org/ffdr-ontology#isShaftway -->


    <owl:DatatypeProperty rdf:about="https://purl.org/ffdr-ontology#isShaftway">
        <rdfs:domain>
            <owl:Class>
                <owl:unionOf rdf:parseType="Collection">
                    <rdf:Description rdf:about="https://purl.org/ffdr-ontology#Door"/>
                    <rdf:Description rdf:about="https://purl.org/ffdr-ontology#Window"/>
                </owl:unionOf>
            </owl:Class>
        </rdfs:domain>
        <rdfs:range rdf:resource="http://www.w3.org/2001/XMLSchema#boolean"/>
        <rdfs:comment xml:lang="en">The &apos;isShaftway&apos; data property checks whether a given element has a shaft (vertical opening) behind it or not.</rdfs:comment>
        <rdfs:label xml:lang="en">isShaftway</rdfs:label>
    </owl:DatatypeProperty>
    


    <!-- https://purl.org/ffdr-ontology#isSystemActivated -->


    <owl:DatatypeProperty rdf:about="https://purl.org/ffdr-ontology#isSystemActivated">
        <rdfs:domain>
            <owl:Class>
                <owl:unionOf rdf:parseType="Collection">
                    <rdf:Description rdf:about="https://purl.org/ffdr-ontology#AutomaticFireExtinguishingSystem"/>
                    <rdf:Description rdf:about="https://purl.org/ffdr-ontology#FireAlarmSystem"/>
                    <rdf:Description rdf:about="https://purl.org/ffdr-ontology#SmokeControlSystem"/>
                    <rdf:Description rdf:about="https://purl.org/ffdr-ontology#SmokeandHeatRemovalSystem"/>
                </owl:unionOf>
            </owl:Class>
        </rdfs:domain>
        <rdfs:range rdf:resource="http://www.w3.org/2001/XMLSchema#boolean"/>
        <rdfs:comment xml:lang="en">The &apos;isSystemActivated&apos; data property checks whether a given system is activated or not.</rdfs:comment>
        <rdfs:label xml:lang="en">isSystemActivated</rdfs:label>
    </owl:DatatypeProperty>
    


    <!-- https://purl.org/ffdr-ontology#isUtilityRunning -->


    <owl:DatatypeProperty rdf:about="https://purl.org/ffdr-ontology#isUtilityRunning">
        <rdfs:domain rdf:resource="https://purl.org/ffdr-ontology#BuildingUtilitySystem"/>
        <rdfs:range rdf:resource="http://www.w3.org/2001/XMLSchema#boolean"/>
        <rdfs:comment xml:lang="en">The &apos;isUtilityRunning&apos; data property checks whether a given utility is running or not.</rdfs:comment>
        <rdfs:label xml:lang="en">isUtilityRunning</rdfs:label>
    </owl:DatatypeProperty>
    


    <!-- 
    ///////////////////////////////////////////////////////////////////////////////////////
    //
    // Classes
    //
    ///////////////////////////////////////////////////////////////////////////////////////
     -->


    


    <!-- https://purl.org/ffdr-ontology#Address -->


    <owl:Class rdf:about="https://purl.org/ffdr-ontology#Address">
        <rdfs:comment xml:lang="en">The &apos;Address&apos; class represents different types of addresses needed during a building fire emergency.</rdfs:comment>
        <rdfs:label xml:lang="en">Address</rdfs:label>
    </owl:Class>
    


    <!-- https://purl.org/ffdr-ontology#AirSupply -->


    <owl:Class rdf:about="https://purl.org/ffdr-ontology#AirSupply">
        <rdfs:subClassOf>
            <owl:Restriction>
                <owl:onProperty rdf:resource="https://purl.org/ffdr-ontology#hasLocation"/>
                <owl:someValuesFrom rdf:resource="http://www.w3.org/2001/XMLSchema#string"/>
            </owl:Restriction>
        </rdfs:subClassOf>
        <rdfs:subClassOf>
            <owl:Restriction>
                <owl:onProperty rdf:resource="https://purl.org/ffdr-ontology#hasType"/>
                <owl:someValuesFrom rdf:resource="http://www.w3.org/2001/XMLSchema#string"/>
            </owl:Restriction>
        </rdfs:subClassOf>
        <rdfs:comment xml:lang="en">Air supply type: Fire department connection panel (FDCP) or fixed air storage system</rdfs:comment>
        <rdfs:comment xml:lang="en">The &apos;AirSupply&apos; class represents an air supply system used to fill firefighters&apos; breathing apparatus cylinders.</rdfs:comment>
        <rdfs:label xml:lang="en">AirSupply</rdfs:label>
    </owl:Class>
    


    <!-- https://purl.org/ffdr-ontology#AlarmSystemAnnunciatorPanel -->


    <owl:Class rdf:about="https://purl.org/ffdr-ontology#AlarmSystemAnnunciatorPanel">
        <rdfs:subClassOf rdf:resource="https://purl.org/ffdr-ontology#ControlPanel"/>
        <rdfs:comment xml:lang="en">The &apos;AlarmSystemAnnunciatorPanel&apos; class represents annunciator panels that display information about the type and location of an active alarm.</rdfs:comment>
        <rdfs:label xml:lang="en">AlarmSystemAnnunciatorPanel</rdfs:label>
    </owl:Class>
    


    <!-- https://purl.org/ffdr-ontology#AlternativeAutomaticFireExtinguishingSystem -->


    <owl:Class rdf:about="https://purl.org/ffdr-ontology#AlternativeAutomaticFireExtinguishingSystem">
        <rdfs:subClassOf rdf:resource="https://purl.org/ffdr-ontology#AutomaticFireExtinguishingSystem"/>
        <owl:disjointWith rdf:resource="https://purl.org/ffdr-ontology#AutomaticSprinklerSystem"/>
        <rdfs:comment xml:lang="en">The &apos;AlternativeAutomaticFireExtinguishingSystem&apos; class represents an automatic fire extinguishing system installed in a building instead of a sprinkler system.</rdfs:comment>
        <rdfs:label xml:lang="en">AlternativeAutomaticFireExtinguishingSystem</rdfs:label>
    </owl:Class>
    


    <!-- https://purl.org/ffdr-ontology#AreaOfRefuge -->


    <owl:Class rdf:about="https://purl.org/ffdr-ontology#AreaOfRefuge">
        <rdfs:subClassOf rdf:resource="https://purl.org/ffdr-ontology#BuildingComponent"/>
        <rdfs:subClassOf>
            <owl:Restriction>
                <owl:onProperty rdf:resource="https://purl.org/ffdr-ontology#hasCapacity"/>
                <owl:someValuesFrom rdf:resource="http://www.w3.org/2001/XMLSchema#int"/>
            </owl:Restriction>
        </rdfs:subClassOf>
        <rdfs:subClassOf>
            <owl:Restriction>
                <owl:onProperty rdf:resource="https://purl.org/ffdr-ontology#hasLocation"/>
                <owl:someValuesFrom rdf:resource="http://www.w3.org/2001/XMLSchema#string"/>
            </owl:Restriction>
        </rdfs:subClassOf>
        <rdfs:comment xml:lang="en">The &apos;AreaOfRefuge&apos; class represents an area of refuge, which is a protected area in a building where occupants can take refuge during an emergency (NFPA 101).</rdfs:comment>
        <rdfs:label xml:lang="en">AreaOfRefuge</rdfs:label>
    </owl:Class>
    


    <!-- https://purl.org/ffdr-ontology#AutomaticFireExtinguishingSystem -->


    <owl:Class rdf:about="https://purl.org/ffdr-ontology#AutomaticFireExtinguishingSystem">
        <rdfs:subClassOf rdf:resource="https://purl.org/ffdr-ontology#BuildingSafetySystem"/>
        <rdfs:subClassOf>
            <owl:Restriction>
                <owl:onProperty rdf:resource="https://purl.org/ffdr-ontology#hasConnectionWith"/>
                <owl:someValuesFrom rdf:resource="https://purl.org/ffdr-ontology#FireAlarmSystem"/>
            </owl:Restriction>
        </rdfs:subClassOf>
        <rdfs:subClassOf>
            <owl:Restriction>
                <owl:onProperty rdf:resource="https://purl.org/ffdr-ontology#hasCoverageZone"/>
                <owl:someValuesFrom rdf:resource="http://www.w3.org/2001/XMLSchema#string"/>
            </owl:Restriction>
        </rdfs:subClassOf>
        <rdfs:subClassOf>
            <owl:Restriction>
                <owl:onProperty rdf:resource="https://purl.org/ffdr-ontology#hasLocationOfControlValve"/>
                <owl:someValuesFrom rdf:resource="http://www.w3.org/2001/XMLSchema#string"/>
            </owl:Restriction>
        </rdfs:subClassOf>
        <rdfs:subClassOf>
            <owl:Restriction>
                <owl:onProperty rdf:resource="https://purl.org/ffdr-ontology#isSystemActivated"/>
                <owl:someValuesFrom rdf:resource="http://www.w3.org/2001/XMLSchema#boolean"/>
            </owl:Restriction>
        </rdfs:subClassOf>
        <rdfs:comment xml:lang="en">The &apos;AutomaticFireExtinguishingSystem&apos; class represents an automatic fire extinguishing system installed in a building.</rdfs:comment>
        <rdfs:label xml:lang="en">AutomaticFireExtinguishingSystem</rdfs:label>
    </owl:Class>
    


    <!-- https://purl.org/ffdr-ontology#AutomaticSprinklerSystem -->


    <owl:Class rdf:about="https://purl.org/ffdr-ontology#AutomaticSprinklerSystem">
        <rdfs:subClassOf rdf:resource="https://purl.org/ffdr-ontology#AutomaticFireExtinguishingSystem"/>
        <rdfs:subClassOf>
            <owl:Restriction>
                <owl:onProperty rdf:resource="https://purl.org/ffdr-ontology#hasWaterSource"/>
                <owl:someValuesFrom>
                    <owl:Class>
                        <owl:unionOf rdf:parseType="Collection">
                            <rdf:Description rdf:about="https://purl.org/ffdr-ontology#FireDepartmentConnection"/>
                            <rdf:Description rdf:about="https://purl.org/ffdr-ontology#WaterSource"/>
                        </owl:unionOf>
                    </owl:Class>
                </owl:someValuesFrom>
            </owl:Restriction>
        </rdfs:subClassOf>
        <rdfs:subClassOf>
            <owl:Restriction>
                <owl:onProperty rdf:resource="https://purl.org/ffdr-ontology#hasRequiredMaximumPressure"/>
                <owl:someValuesFrom rdf:resource="http://www.w3.org/2001/XMLSchema#double"/>
            </owl:Restriction>
        </rdfs:subClassOf>
        <rdfs:subClassOf>
            <owl:Restriction>
                <owl:onProperty rdf:resource="https://purl.org/ffdr-ontology#hasRequiredMinimumPressure"/>
                <owl:someValuesFrom rdf:resource="http://www.w3.org/2001/XMLSchema#double"/>
            </owl:Restriction>
        </rdfs:subClassOf>
        <rdfs:subClassOf>
            <owl:Restriction>
                <owl:onProperty rdf:resource="https://purl.org/ffdr-ontology#isControlValveOn"/>
                <owl:someValuesFrom rdf:resource="http://www.w3.org/2001/XMLSchema#boolean"/>
            </owl:Restriction>
        </rdfs:subClassOf>
        <rdfs:comment xml:lang="en">The &apos;AutomaticSprinklerSystem&apos; class represents a sprinkler system installed in a building.</rdfs:comment>
        <rdfs:label xml:lang="en">AutomaticSprinklerSystem</rdfs:label>
    </owl:Class>
    


    <!-- https://purl.org/ffdr-ontology#BackUpPowerSupplySystem -->


    <owl:Class rdf:about="https://purl.org/ffdr-ontology#BackUpPowerSupplySystem">
        <rdfs:subClassOf rdf:resource="https://purl.org/ffdr-ontology#BuildingUtilitySystem"/>
        <rdfs:comment xml:lang="en">The &apos;BackUpPowerSupplySystem&apos; class represents a building&apos;s backup power supply system.</rdfs:comment>
        <rdfs:label xml:lang="en">BackUpPowerSupplySystem</rdfs:label>
    </owl:Class>
    


    <!-- https://purl.org/ffdr-ontology#Balcony -->


    <owl:Class rdf:about="https://purl.org/ffdr-ontology#Balcony">
        <rdfs:subClassOf rdf:resource="https://purl.org/ffdr-ontology#NonStructuralElement"/>
        <rdfs:subClassOf>
            <owl:Restriction>
                <owl:onProperty rdf:resource="https://purl.org/ffdr-ontology#hasCapacity"/>
                <owl:qualifiedCardinality rdf:datatype="http://www.w3.org/2001/XMLSchema#nonNegativeInteger">1</owl:qualifiedCardinality>
                <owl:onDataRange rdf:resource="http://www.w3.org/2001/XMLSchema#int"/>
            </owl:Restriction>
        </rdfs:subClassOf>
        <rdfs:subClassOf>
            <owl:Restriction>
                <owl:onProperty rdf:resource="https://purl.org/ffdr-ontology#hasWidth"/>
                <owl:qualifiedCardinality rdf:datatype="http://www.w3.org/2001/XMLSchema#nonNegativeInteger">1</owl:qualifiedCardinality>
                <owl:onDataRange rdf:resource="http://www.w3.org/2001/XMLSchema#double"/>
            </owl:Restriction>
        </rdfs:subClassOf>
        <rdfs:comment xml:lang="en">The &apos;Balcony&apos; class represents balconies that may be found in a building.</rdfs:comment>
        <rdfs:label xml:lang="en">Balcony</rdfs:label>
    </owl:Class>
    


    <!-- https://purl.org/ffdr-ontology#Building -->


    <owl:Class rdf:about="https://purl.org/ffdr-ontology#Building">
        <rdfs:subClassOf rdf:resource="https://purl.org/ffdr-ontology#SurroundingStructure"/>
        <rdfs:comment xml:lang="en">The &apos;Building&apos; class represents buildings other than the incident building.</rdfs:comment>
        <rdfs:label xml:lang="en">Building</rdfs:label>
    </owl:Class>
    


    <!-- https://purl.org/ffdr-ontology#BuildingAddress -->


    <owl:Class rdf:about="https://purl.org/ffdr-ontology#BuildingAddress">
        <rdfs:subClassOf rdf:resource="https://purl.org/ffdr-ontology#Address"/>
        <rdfs:comment xml:lang="en">The &apos;BuildingAddress&apos; class represents a building&apos;s address.</rdfs:comment>
        <rdfs:label xml:lang="en">BuildingAddress</rdfs:label>
    </owl:Class>
    


    <!-- https://purl.org/ffdr-ontology#BuildingComponent -->


    <owl:Class rdf:about="https://purl.org/ffdr-ontology#BuildingComponent">
        <rdfs:comment xml:lang="en">The &apos;BuildingComponent&apos; class represents different building components that firefighters may interact with during a building fire emergency.</rdfs:comment>
        <rdfs:label xml:lang="en">BuildingComponent</rdfs:label>
    </owl:Class>
    


    <!-- https://purl.org/ffdr-ontology#BuildingEngineerContactAddress -->


    <owl:Class rdf:about="https://purl.org/ffdr-ontology#BuildingEngineerContactAddress">
        <rdfs:subClassOf rdf:resource="https://purl.org/ffdr-ontology#Address"/>
        <rdfs:comment xml:lang="en">The &apos;BuildingEngineerContactAddress&apos; class represents a building engineer&apos;s contact address.</rdfs:comment>
        <rdfs:label xml:lang="en">BuildingEngineerContactAddress</rdfs:label>
    </owl:Class>
    


    <!-- https://purl.org/ffdr-ontology#BuildingManagerContactAddress -->


    <owl:Class rdf:about="https://purl.org/ffdr-ontology#BuildingManagerContactAddress">
        <rdfs:subClassOf rdf:resource="https://purl.org/ffdr-ontology#Address"/>
        <rdfs:comment xml:lang="en">The &apos;BuildingManagerContactAddress&apos; class represents a building manager&apos;s contact address.</rdfs:comment>
        <rdfs:label xml:lang="en">BuildingManagerContactAddress</rdfs:label>
    </owl:Class>
    


    <!-- https://purl.org/ffdr-ontology#BuildingOccupancy -->


    <owl:Class rdf:about="https://purl.org/ffdr-ontology#BuildingOccupancy">
        <owl:equivalentClass>
            <owl:Class>
                <owl:oneOf rdf:parseType="Collection">
                    <rdf:Description rdf:about="https://purl.org/ffdr-ontology#Assembly"/>
                    <rdf:Description rdf:about="https://purl.org/ffdr-ontology#Business"/>
                    <rdf:Description rdf:about="https://purl.org/ffdr-ontology#Educational"/>
                    <rdf:Description rdf:about="https://purl.org/ffdr-ontology#FactoryAndIndustrial"/>
                    <rdf:Description rdf:about="https://purl.org/ffdr-ontology#HighHazard"/>
                    <rdf:Description rdf:about="https://purl.org/ffdr-ontology#Institutional"/>
                    <rdf:Description rdf:about="https://purl.org/ffdr-ontology#Mercantile"/>
                    <rdf:Description rdf:about="https://purl.org/ffdr-ontology#Residential"/>
                    <rdf:Description rdf:about="https://purl.org/ffdr-ontology#Storage"/>
                    <rdf:Description rdf:about="https://purl.org/ffdr-ontology#UtilityAndMiscellaneous"/>
                </owl:oneOf>
            </owl:Class>
        </owl:equivalentClass>
        <rdfs:subClassOf>
            <owl:Restriction>
                <owl:onProperty rdf:resource="https://purl.org/ffdr-ontology#hasDescription"/>
                <owl:someValuesFrom rdf:resource="http://www.w3.org/2001/XMLSchema#string"/>
            </owl:Restriction>
        </rdfs:subClassOf>
        <rdfs:subClassOf>
            <owl:Restriction>
                <owl:onProperty rdf:resource="https://purl.org/ffdr-ontology#isAbandoned"/>
                <owl:someValuesFrom rdf:resource="http://www.w3.org/2001/XMLSchema#boolean"/>
            </owl:Restriction>
        </rdfs:subClassOf>
        <rdfs:comment xml:lang="en">The &apos;BuildingOccupancy&apos; class represents the purpose of a building based on the classification given in the International Building Code (2018).</rdfs:comment>
        <rdfs:label xml:lang="en">BuildingOccupancy</rdfs:label>
    </owl:Class>
    


    <!-- https://purl.org/ffdr-ontology#BuildingPlan -->


    <owl:Class rdf:about="https://purl.org/ffdr-ontology#BuildingPlan">
        <rdfs:subClassOf>
            <owl:Restriction>
                <owl:onProperty rdf:resource="https://purl.org/ffdr-ontology#hasLocation"/>
                <owl:someValuesFrom rdf:resource="http://www.w3.org/2001/XMLSchema#string"/>
            </owl:Restriction>
        </rdfs:subClassOf>
        <rdfs:subClassOf>
            <owl:Restriction>
                <owl:onProperty rdf:resource="https://purl.org/ffdr-ontology#hasType"/>
                <owl:someValuesFrom rdf:resource="http://www.w3.org/2001/XMLSchema#string"/>
            </owl:Restriction>
        </rdfs:subClassOf>
        <rdfs:comment xml:lang="en">The &apos;BuildingPlan&apos; class represents building plans such as schematic plans of the building and a fire emergency evacuation plan.</rdfs:comment>
        <rdfs:label xml:lang="en">BuildingPlan</rdfs:label>
    </owl:Class>
    


    <!-- https://purl.org/ffdr-ontology#BuildingSafetySystem -->


    <owl:Class rdf:about="https://purl.org/ffdr-ontology#BuildingSafetySystem">
        <rdfs:subClassOf rdf:resource="https://purl.org/ffdr-ontology#BuildingComponent"/>
        <rdfs:comment xml:lang="en">The &apos;BuildingSafetySystem&apos; class represents components of a building geared towards building safety.</rdfs:comment>
        <rdfs:label xml:lang="en">BuildingSafetySystem</rdfs:label>
    </owl:Class>
    


    <!-- https://purl.org/ffdr-ontology#BuildingUtilitySystem -->


    <owl:Class rdf:about="https://purl.org/ffdr-ontology#BuildingUtilitySystem">
        <rdfs:subClassOf rdf:resource="https://purl.org/ffdr-ontology#BuildingComponent"/>
        <rdfs:subClassOf>
            <owl:Restriction>
                <owl:onProperty rdf:resource="https://purl.org/ffdr-ontology#hasAddress"/>
                <owl:someValuesFrom rdf:resource="https://purl.org/ffdr-ontology#UtilityContactAddress"/>
            </owl:Restriction>
        </rdfs:subClassOf>
        <rdfs:subClassOf>
            <owl:Restriction>
                <owl:onProperty rdf:resource="https://purl.org/ffdr-ontology#hasControlPanel"/>
                <owl:someValuesFrom rdf:resource="https://purl.org/ffdr-ontology#UtilityControlPanel"/>
            </owl:Restriction>
        </rdfs:subClassOf>
        <rdfs:subClassOf>
            <owl:Restriction>
                <owl:onProperty rdf:resource="https://purl.org/ffdr-ontology#isUtilityRunning"/>
                <owl:someValuesFrom rdf:resource="http://www.w3.org/2001/XMLSchema#boolean"/>
            </owl:Restriction>
        </rdfs:subClassOf>
        <rdfs:comment xml:lang="en">The &apos;BuildingUtilitySystem&apos; class represents utilities found in a building.</rdfs:comment>
        <rdfs:label xml:lang="en">BuildingUtilitySystem</rdfs:label>
    </owl:Class>
    


    <!-- https://purl.org/ffdr-ontology#CarbonMonoxideDetector -->


    <owl:Class rdf:about="https://purl.org/ffdr-ontology#CarbonMonoxideDetector">
        <rdfs:subClassOf rdf:resource="https://purl.org/ffdr-ontology#SensorDetector"/>
        <rdfs:comment xml:lang="en">The &apos;CarbonMonoxideDetector&apos; class represents Carbon Monoxide detectors installed in a building.</rdfs:comment>
        <rdfs:label xml:lang="en">CarbonMonoxideDetector</rdfs:label>
    </owl:Class>
    


    <!-- https://purl.org/ffdr-ontology#CbrSensor -->


    <owl:Class rdf:about="https://purl.org/ffdr-ontology#CbrSensor">
        <rdfs:subClassOf rdf:resource="https://purl.org/ffdr-ontology#SensorDetector"/>
        <rdfs:comment xml:lang="en">The &apos;CbrSensor&apos; class represents Chemical/Biological/Radiation (CBR) sensors installed in a building.</rdfs:comment>
        <rdfs:label xml:lang="en">CbrSensor</rdfs:label>
    </owl:Class>
    


    <!-- https://purl.org/ffdr-ontology#ConcealedSpace -->


    <owl:Class rdf:about="https://purl.org/ffdr-ontology#ConcealedSpace">
        <rdfs:subClassOf rdf:resource="https://purl.org/ffdr-ontology#BuildingComponent"/>
        <rdfs:subClassOf>
            <owl:Restriction>
                <owl:onProperty rdf:resource="https://purl.org/ffdr-ontology#hasFireExtinguishingSystem"/>
                <owl:someValuesFrom rdf:resource="https://purl.org/ffdr-ontology#AutomaticFireExtinguishingSystem"/>
            </owl:Restriction>
        </rdfs:subClassOf>
        <rdfs:subClassOf>
            <owl:Restriction>
                <owl:onProperty rdf:resource="https://purl.org/ffdr-ontology#hasDescription"/>
                <owl:someValuesFrom rdf:resource="http://www.w3.org/2001/XMLSchema#string"/>
            </owl:Restriction>
        </rdfs:subClassOf>
        <rdfs:subClassOf>
            <owl:Restriction>
                <owl:onProperty rdf:resource="https://purl.org/ffdr-ontology#hasLocation"/>
                <owl:someValuesFrom rdf:resource="http://www.w3.org/2001/XMLSchema#string"/>
            </owl:Restriction>
        </rdfs:subClassOf>
        <rdfs:comment xml:lang="en">The &apos;ConcealedSpace&apos; class represents concealed spaces that may be found in a building.</rdfs:comment>
        <rdfs:label xml:lang="en">ConcealedSpace</rdfs:label>
    </owl:Class>
    


    <!-- https://purl.org/ffdr-ontology#ConstructionType -->


    <owl:Class rdf:about="https://purl.org/ffdr-ontology#ConstructionType">
        <owl:equivalentClass>
            <owl:Class>
                <owl:oneOf rdf:parseType="Collection">
                    <rdf:Description rdf:about="https://purl.org/ffdr-ontology#TypeI"/>
                    <rdf:Description rdf:about="https://purl.org/ffdr-ontology#TypeII"/>
                    <rdf:Description rdf:about="https://purl.org/ffdr-ontology#TypeIII"/>
                    <rdf:Description rdf:about="https://purl.org/ffdr-ontology#TypeIV"/>
                    <rdf:Description rdf:about="https://purl.org/ffdr-ontology#TypeV"/>
                </owl:oneOf>
            </owl:Class>
        </owl:equivalentClass>
        <rdfs:subClassOf>
            <owl:Restriction>
                <owl:onProperty rdf:resource="https://purl.org/ffdr-ontology#hasDescription"/>
                <owl:someValuesFrom rdf:resource="http://www.w3.org/2001/XMLSchema#string"/>
            </owl:Restriction>
        </rdfs:subClassOf>
        <rdfs:subClassOf>
            <owl:Restriction>
                <owl:onProperty rdf:resource="https://purl.org/ffdr-ontology#hasType"/>
                <owl:someValuesFrom rdf:resource="http://www.w3.org/2001/XMLSchema#string"/>
            </owl:Restriction>
        </rdfs:subClassOf>
        <rdfs:comment xml:lang="en">The &apos;ConstructionType&apos; class represents the construction type of a building. The classification is based on the materials used in a building (whether they are combustible or noncombustible) and the fire resistance of a building&apos;s elements (IBC, 2018)</rdfs:comment>
        <rdfs:label xml:lang="en">ConstructionType</rdfs:label>
    </owl:Class>
    


    <!-- https://purl.org/ffdr-ontology#ControlPanel -->


    <owl:Class rdf:about="https://purl.org/ffdr-ontology#ControlPanel">
        <rdfs:subClassOf>
            <owl:Restriction>
                <owl:onProperty rdf:resource="https://purl.org/ffdr-ontology#hasDescription"/>
                <owl:someValuesFrom rdf:resource="http://www.w3.org/2001/XMLSchema#string"/>
            </owl:Restriction>
        </rdfs:subClassOf>
        <rdfs:subClassOf>
            <owl:Restriction>
                <owl:onProperty rdf:resource="https://purl.org/ffdr-ontology#hasLocation"/>
                <owl:someValuesFrom rdf:resource="http://www.w3.org/2001/XMLSchema#string"/>
            </owl:Restriction>
        </rdfs:subClassOf>
        <rdfs:comment xml:lang="en">The &apos;ControlPanel&apos; class represents different control panels used to control several building systems and utilities.</rdfs:comment>
        <rdfs:label xml:lang="en">ControlPanel</rdfs:label>
    </owl:Class>
    


    <!-- https://purl.org/ffdr-ontology#Door -->


    <owl:Class rdf:about="https://purl.org/ffdr-ontology#Door">
        <rdfs:subClassOf rdf:resource="https://purl.org/ffdr-ontology#NonStructuralElement"/>
        <rdfs:subClassOf>
            <owl:Restriction>
                <owl:onProperty rdf:resource="https://purl.org/ffdr-ontology#hasControlPanel"/>
                <owl:someValuesFrom rdf:resource="https://purl.org/ffdr-ontology#DoorUnlockingSystemControlPanel"/>
            </owl:Restriction>
        </rdfs:subClassOf>
        <rdfs:subClassOf>
            <owl:Restriction>
                <owl:onProperty rdf:resource="https://purl.org/ffdr-ontology#hasOpeningDirection"/>
                <owl:someValuesFrom rdf:resource="http://www.w3.org/2001/XMLSchema#string"/>
            </owl:Restriction>
        </rdfs:subClassOf>
        <rdfs:subClassOf>
            <owl:Restriction>
                <owl:onProperty rdf:resource="https://purl.org/ffdr-ontology#isFunctional"/>
                <owl:someValuesFrom rdf:resource="http://www.w3.org/2001/XMLSchema#boolean"/>
            </owl:Restriction>
        </rdfs:subClassOf>
        <rdfs:subClassOf>
            <owl:Restriction>
                <owl:onProperty rdf:resource="https://purl.org/ffdr-ontology#isPrimaryFireServiceEntryPoint"/>
                <owl:someValuesFrom rdf:resource="http://www.w3.org/2001/XMLSchema#boolean"/>
            </owl:Restriction>
        </rdfs:subClassOf>
        <rdfs:subClassOf>
            <owl:Restriction>
                <owl:onProperty rdf:resource="https://purl.org/ffdr-ontology#isShaftway"/>
                <owl:someValuesFrom rdf:resource="http://www.w3.org/2001/XMLSchema#boolean"/>
            </owl:Restriction>
        </rdfs:subClassOf>
        <rdfs:subClassOf>
            <owl:Restriction>
                <owl:onProperty rdf:resource="https://purl.org/ffdr-ontology#hasExitTravelDistances"/>
                <owl:qualifiedCardinality rdf:datatype="http://www.w3.org/2001/XMLSchema#nonNegativeInteger">1</owl:qualifiedCardinality>
                <owl:onDataRange rdf:resource="http://www.w3.org/2001/XMLSchema#double"/>
            </owl:Restriction>
        </rdfs:subClassOf>
        <rdfs:subClassOf>
            <owl:Restriction>
                <owl:onProperty rdf:resource="https://purl.org/ffdr-ontology#hasWidth"/>
                <owl:qualifiedCardinality rdf:datatype="http://www.w3.org/2001/XMLSchema#nonNegativeInteger">1</owl:qualifiedCardinality>
                <owl:onDataRange rdf:resource="http://www.w3.org/2001/XMLSchema#double"/>
            </owl:Restriction>
        </rdfs:subClassOf>
        <rdfs:subClassOf>
            <owl:Restriction>
                <owl:onProperty rdf:resource="https://purl.org/ffdr-ontology#isExit"/>
                <owl:qualifiedCardinality rdf:datatype="http://www.w3.org/2001/XMLSchema#nonNegativeInteger">1</owl:qualifiedCardinality>
                <owl:onDataRange rdf:resource="http://www.w3.org/2001/XMLSchema#boolean"/>
            </owl:Restriction>
        </rdfs:subClassOf>
        <rdfs:comment xml:lang="en">The &apos;Door&apos; class represents doors in a building.</rdfs:comment>
        <rdfs:label xml:lang="en">Door</rdfs:label>
    </owl:Class>
    


    <!-- https://purl.org/ffdr-ontology#DoorUnlockingSystemControlPanel -->


    <owl:Class rdf:about="https://purl.org/ffdr-ontology#DoorUnlockingSystemControlPanel">
        <rdfs:subClassOf rdf:resource="https://purl.org/ffdr-ontology#ControlPanel"/>
        <rdfs:comment xml:lang="en">The &apos;DoorUnlockingSystemControlPanel&apos; class represents a control panel used to unlock some or all doors in a building.</rdfs:comment>
        <rdfs:label xml:lang="en">DoorUnlockingSystemControlPanel</rdfs:label>
    </owl:Class>
    


    <!-- https://purl.org/ffdr-ontology#Elevator -->


    <owl:Class rdf:about="https://purl.org/ffdr-ontology#Elevator">
        <rdfs:subClassOf rdf:resource="https://purl.org/ffdr-ontology#NonStructuralElement"/>
        <rdfs:subClassOf>
            <owl:Restriction>
                <owl:onProperty rdf:resource="https://purl.org/ffdr-ontology#hasControlPanel"/>
                <owl:someValuesFrom rdf:resource="https://purl.org/ffdr-ontology#ElevatorOverrideControlPanel"/>
            </owl:Restriction>
        </rdfs:subClassOf>
        <rdfs:subClassOf>
            <owl:Restriction>
                <owl:onProperty rdf:resource="https://purl.org/ffdr-ontology#hasFireExtinguishingSystem"/>
                <owl:someValuesFrom rdf:resource="https://purl.org/ffdr-ontology#AutomaticFireExtinguishingSystem"/>
            </owl:Restriction>
        </rdfs:subClassOf>
        <rdfs:subClassOf>
            <owl:Restriction>
                <owl:onProperty rdf:resource="https://purl.org/ffdr-ontology#hasCapacity"/>
                <owl:someValuesFrom rdf:resource="http://www.w3.org/2001/XMLSchema#int"/>
            </owl:Restriction>
        </rdfs:subClassOf>
        <rdfs:subClassOf>
            <owl:Restriction>
                <owl:onProperty rdf:resource="https://purl.org/ffdr-ontology#hasDischargeLevel"/>
                <owl:someValuesFrom rdf:resource="http://www.w3.org/2001/XMLSchema#string"/>
            </owl:Restriction>
        </rdfs:subClassOf>
        <rdfs:subClassOf>
            <owl:Restriction>
                <owl:onProperty rdf:resource="https://purl.org/ffdr-ontology#hasFloorsServed"/>
                <owl:someValuesFrom rdf:resource="http://www.w3.org/2001/XMLSchema#string"/>
            </owl:Restriction>
        </rdfs:subClassOf>
        <rdfs:subClassOf>
            <owl:Restriction>
                <owl:onProperty rdf:resource="https://purl.org/ffdr-ontology#hasMachineRoomLocation"/>
                <owl:someValuesFrom rdf:resource="http://www.w3.org/2001/XMLSchema#string"/>
            </owl:Restriction>
        </rdfs:subClassOf>
        <rdfs:subClassOf>
            <owl:Restriction>
                <owl:onProperty rdf:resource="https://purl.org/ffdr-ontology#isFunctional"/>
                <owl:someValuesFrom rdf:resource="http://www.w3.org/2001/XMLSchema#boolean"/>
            </owl:Restriction>
        </rdfs:subClassOf>
        <rdfs:subClassOf>
            <owl:Restriction>
                <owl:onProperty rdf:resource="https://purl.org/ffdr-ontology#isQualifiedForEvacuation"/>
                <owl:someValuesFrom rdf:resource="http://www.w3.org/2001/XMLSchema#boolean"/>
            </owl:Restriction>
        </rdfs:subClassOf>
        <rdfs:subClassOf>
            <owl:Restriction>
                <owl:onProperty rdf:resource="https://purl.org/ffdr-ontology#hasExitTravelDistances"/>
                <owl:qualifiedCardinality rdf:datatype="http://www.w3.org/2001/XMLSchema#nonNegativeInteger">1</owl:qualifiedCardinality>
                <owl:onDataRange rdf:resource="http://www.w3.org/2001/XMLSchema#double"/>
            </owl:Restriction>
        </rdfs:subClassOf>
        <rdfs:comment xml:lang="en">The &apos;Elevator&apos; class represents elevators that may be found in a building.</rdfs:comment>
        <rdfs:label xml:lang="en">Elevator</rdfs:label>
    </owl:Class>
    


    <!-- https://purl.org/ffdr-ontology#ElevatorOverrideControlPanel -->


    <owl:Class rdf:about="https://purl.org/ffdr-ontology#ElevatorOverrideControlPanel">
        <rdfs:subClassOf rdf:resource="https://purl.org/ffdr-ontology#ControlPanel"/>
        <rdfs:comment xml:lang="en">The &apos;ElevatorOverrideControlPanel&apos; class represents a control panel used to override elevators in a building.</rdfs:comment>
        <rdfs:label xml:lang="en">ElevatorOverrideControlPanel</rdfs:label>
    </owl:Class>
    


    <!-- https://purl.org/ffdr-ontology#EmergencyPowerOutlet -->


    <owl:Class rdf:about="https://purl.org/ffdr-ontology#EmergencyPowerOutlet">
        <rdfs:subClassOf rdf:resource="https://purl.org/ffdr-ontology#BuildingSafetySystem"/>
        <rdfs:subClassOf>
            <owl:Restriction>
                <owl:onProperty rdf:resource="https://purl.org/ffdr-ontology#hasLocation"/>
                <owl:someValuesFrom rdf:resource="http://www.w3.org/2001/XMLSchema#string"/>
            </owl:Restriction>
        </rdfs:subClassOf>
        <rdfs:subClassOf>
            <owl:Restriction>
                <owl:onProperty rdf:resource="https://purl.org/ffdr-ontology#hasType"/>
                <owl:someValuesFrom rdf:resource="http://www.w3.org/2001/XMLSchema#string"/>
            </owl:Restriction>
        </rdfs:subClassOf>
        <rdfs:comment xml:lang="en">The &apos;EmergencyPowerOutlet&apos; class represents emergency power outlets built into a building that can provide power to electric-operated firefighting equipment (OSHA, 2015).</rdfs:comment>
        <rdfs:label xml:lang="en">EmergencyPowerOutlet</rdfs:label>
    </owl:Class>
    


    <!-- https://purl.org/ffdr-ontology#EmergencyServiceProvider -->


    <owl:Class rdf:about="https://purl.org/ffdr-ontology#EmergencyServiceProvider">
        <rdfs:subClassOf>
            <owl:Restriction>
                <owl:onProperty rdf:resource="https://purl.org/ffdr-ontology#hasAddress"/>
                <owl:someValuesFrom rdf:resource="https://purl.org/ffdr-ontology#EmergencyServiceProviderContactAddress"/>
            </owl:Restriction>
        </rdfs:subClassOf>
        <rdfs:subClassOf>
            <owl:Restriction>
                <owl:onProperty rdf:resource="https://purl.org/ffdr-ontology#hasDistanceFromIncidentBuilding"/>
                <owl:someValuesFrom rdf:resource="http://www.w3.org/2001/XMLSchema#double"/>
            </owl:Restriction>
        </rdfs:subClassOf>
        <rdfs:subClassOf>
            <owl:Restriction>
                <owl:onProperty rdf:resource="https://purl.org/ffdr-ontology#hasLocation"/>
                <owl:someValuesFrom rdf:resource="http://www.w3.org/2001/XMLSchema#string"/>
            </owl:Restriction>
        </rdfs:subClassOf>
        <rdfs:comment xml:lang="en">The &apos;EmergencyServiceProvider&apos; class represents emergency service providers involved in a building fire emergency response.</rdfs:comment>
        <rdfs:label xml:lang="en">EmergencyServiceProvider</rdfs:label>
    </owl:Class>
    


    <!-- https://purl.org/ffdr-ontology#EmergencyServiceProviderContactAddress -->


    <owl:Class rdf:about="https://purl.org/ffdr-ontology#EmergencyServiceProviderContactAddress">
        <rdfs:subClassOf rdf:resource="https://purl.org/ffdr-ontology#Address"/>
        <rdfs:comment xml:lang="en">The &apos;EmergencyServiceProviderContactAddress&apos; class represents different emergency service provider&apos;s contact address.</rdfs:comment>
        <rdfs:label xml:lang="en">EmergencyServiceProviderContactAddress</rdfs:label>
    </owl:Class>
    


    <!-- https://purl.org/ffdr-ontology#ExteriorDoor -->


    <owl:Class rdf:about="https://purl.org/ffdr-ontology#ExteriorDoor">
        <owl:equivalentClass>
            <owl:Class>
                <owl:intersectionOf rdf:parseType="Collection">
                    <rdf:Description rdf:about="https://purl.org/ffdr-ontology#Door"/>
                    <owl:Restriction>
                        <owl:onProperty rdf:resource="https://purl.org/ffdr-ontology#isExit"/>
                        <owl:hasValue rdf:datatype="http://www.w3.org/2001/XMLSchema#boolean">true</owl:hasValue>
                    </owl:Restriction>
                </owl:intersectionOf>
            </owl:Class>
        </owl:equivalentClass>
        <rdfs:subClassOf rdf:resource="https://purl.org/ffdr-ontology#Facade"/>
        <rdfs:comment xml:lang="en">The &apos;ExteriorDoor&apos; class represents doors found on the exterior of a building.</rdfs:comment>
        <rdfs:label xml:lang="en">ExteriorDoor</rdfs:label>
    </owl:Class>
    


    <!-- https://purl.org/ffdr-ontology#ExteriorWall -->


    <owl:Class rdf:about="https://purl.org/ffdr-ontology#ExteriorWall">
        <owl:equivalentClass>
            <owl:Class>
                <owl:intersectionOf rdf:parseType="Collection">
                    <rdf:Description rdf:about="https://purl.org/ffdr-ontology#Wall"/>
                    <owl:Restriction>
                        <owl:onProperty rdf:resource="https://purl.org/ffdr-ontology#isOnExterior"/>
                        <owl:hasValue rdf:datatype="http://www.w3.org/2001/XMLSchema#boolean">true</owl:hasValue>
                    </owl:Restriction>
                </owl:intersectionOf>
            </owl:Class>
        </owl:equivalentClass>
        <rdfs:subClassOf rdf:resource="https://purl.org/ffdr-ontology#Facade"/>
        <rdfs:comment xml:lang="en">The &apos;ExteriorWall&apos; class represents walls found on the exterior of a building.</rdfs:comment>
        <rdfs:label xml:lang="en">ExteriorWall</rdfs:label>
    </owl:Class>
    


    <!-- https://purl.org/ffdr-ontology#ExteriorWindow -->


    <owl:Class rdf:about="https://purl.org/ffdr-ontology#ExteriorWindow">
        <owl:equivalentClass>
            <owl:Class>
                <owl:intersectionOf rdf:parseType="Collection">
                    <rdf:Description rdf:about="https://purl.org/ffdr-ontology#Window"/>
                    <owl:Restriction>
                        <owl:onProperty rdf:resource="https://purl.org/ffdr-ontology#isOnExterior"/>
                        <owl:hasValue rdf:datatype="http://www.w3.org/2001/XMLSchema#boolean">true</owl:hasValue>
                    </owl:Restriction>
                </owl:intersectionOf>
            </owl:Class>
        </owl:equivalentClass>
        <rdfs:subClassOf rdf:resource="https://purl.org/ffdr-ontology#Facade"/>
        <rdfs:comment xml:lang="en">The &apos;ExteriorWindow&apos; class represents windows found on the exterior of a building.</rdfs:comment>
        <rdfs:label xml:lang="en">ExteriorWindow</rdfs:label>
    </owl:Class>
    


    <!-- https://purl.org/ffdr-ontology#ExtremelyValuableMaterial -->


    <owl:Class rdf:about="https://purl.org/ffdr-ontology#ExtremelyValuableMaterial">
        <rdfs:subClassOf rdf:resource="https://purl.org/ffdr-ontology#BuildingComponent"/>
        <rdfs:subClassOf>
            <owl:Restriction>
                <owl:onProperty rdf:resource="https://purl.org/ffdr-ontology#hasLocation"/>
                <owl:someValuesFrom rdf:resource="http://www.w3.org/2001/XMLSchema#string"/>
            </owl:Restriction>
        </rdfs:subClassOf>
        <rdfs:comment xml:lang="en">The &apos;ExtremelyValuableMaterial&apos; class represents extremely valuable materials that may be found in a building.</rdfs:comment>
        <rdfs:label xml:lang="en">ExtremelyValuableMaterial</rdfs:label>
    </owl:Class>
    


    <!-- https://purl.org/ffdr-ontology#Facade -->


    <owl:Class rdf:about="https://purl.org/ffdr-ontology#Facade">
        <rdfs:subClassOf rdf:resource="https://purl.org/ffdr-ontology#BuildingComponent"/>
        <rdfs:comment xml:lang="en">The &apos;Facade&apos; class represents the facade of a building.</rdfs:comment>
        <rdfs:label xml:lang="en">Facade</rdfs:label>
    </owl:Class>
    


    <!-- https://purl.org/ffdr-ontology#FarsControlPanel -->


    <owl:Class rdf:about="https://purl.org/ffdr-ontology#FarsControlPanel">
        <rdfs:subClassOf rdf:resource="https://purl.org/ffdr-ontology#ControlPanel"/>
        <rdfs:comment xml:lang="en">The &apos;FarsControlPanel&apos; class represents a control panel used to control a firefighter&apos;s air replenishment system (FARS)  that may be found in a building.</rdfs:comment>
        <rdfs:label xml:lang="en">FarsControlPanel</rdfs:label>
    </owl:Class>
    


    <!-- https://purl.org/ffdr-ontology#FarsFillStation -->


    <owl:Class rdf:about="https://purl.org/ffdr-ontology#FarsFillStation">
        <rdfs:subClassOf rdf:resource="https://purl.org/ffdr-ontology#BuildingSafetySystem"/>
        <rdfs:subClassOf>
            <owl:Restriction>
                <owl:onProperty rdf:resource="https://purl.org/ffdr-ontology#hasControlPanel"/>
                <owl:someValuesFrom rdf:resource="https://purl.org/ffdr-ontology#FarsControlPanel"/>
            </owl:Restriction>
        </rdfs:subClassOf>
        <rdfs:subClassOf>
            <owl:Restriction>
                <owl:onProperty rdf:resource="https://purl.org/ffdr-ontology#hasFillPressure"/>
                <owl:someValuesFrom rdf:resource="http://www.w3.org/2001/XMLSchema#double"/>
            </owl:Restriction>
        </rdfs:subClassOf>
        <rdfs:subClassOf>
            <owl:Restriction>
                <owl:onProperty rdf:resource="https://purl.org/ffdr-ontology#hasFillTime"/>
                <owl:someValuesFrom rdf:resource="http://www.w3.org/2001/XMLSchema#double"/>
            </owl:Restriction>
        </rdfs:subClassOf>
        <rdfs:subClassOf>
            <owl:Restriction>
                <owl:onProperty rdf:resource="https://purl.org/ffdr-ontology#hasLocation"/>
                <owl:someValuesFrom rdf:resource="http://www.w3.org/2001/XMLSchema#string"/>
            </owl:Restriction>
        </rdfs:subClassOf>
        <rdfs:subClassOf>
            <owl:Restriction>
                <owl:onProperty rdf:resource="https://purl.org/ffdr-ontology#hasNumberOfSimultaneousFill"/>
                <owl:someValuesFrom rdf:resource="http://www.w3.org/2001/XMLSchema#int"/>
            </owl:Restriction>
        </rdfs:subClassOf>
        <rdfs:comment xml:lang="en">The &apos;FarsFillStation&apos; class represents firefighter air replenishment system (FARS) filling stations or panels that allow firefighters to replenish their breathing apparatus cylinders (OSHA, 2015).</rdfs:comment>
        <rdfs:label xml:lang="en">FarsFillStation</rdfs:label>
    </owl:Class>
    


    <!-- https://purl.org/ffdr-ontology#FireAlarmSystem -->


    <owl:Class rdf:about="https://purl.org/ffdr-ontology#FireAlarmSystem">
        <rdfs:subClassOf rdf:resource="https://purl.org/ffdr-ontology#BuildingSafetySystem"/>
        <rdfs:subClassOf>
            <owl:Restriction>
                <owl:onProperty rdf:resource="https://purl.org/ffdr-ontology#hasControlPanel"/>
                <owl:someValuesFrom rdf:resource="https://purl.org/ffdr-ontology#AlarmSystemAnnunciatorPanel"/>
            </owl:Restriction>
        </rdfs:subClassOf>
        <rdfs:subClassOf>
            <owl:Restriction>
                <owl:onProperty rdf:resource="https://purl.org/ffdr-ontology#hasCoverageZone"/>
                <owl:someValuesFrom rdf:resource="http://www.w3.org/2001/XMLSchema#string"/>
            </owl:Restriction>
        </rdfs:subClassOf>
        <rdfs:subClassOf>
            <owl:Restriction>
                <owl:onProperty rdf:resource="https://purl.org/ffdr-ontology#hasTypeOfSignalInitiator"/>
                <owl:someValuesFrom rdf:resource="http://www.w3.org/2001/XMLSchema#string"/>
            </owl:Restriction>
        </rdfs:subClassOf>
        <rdfs:subClassOf>
            <owl:Restriction>
                <owl:onProperty rdf:resource="https://purl.org/ffdr-ontology#isSystemActivated"/>
                <owl:someValuesFrom rdf:resource="http://www.w3.org/2001/XMLSchema#boolean"/>
            </owl:Restriction>
        </rdfs:subClassOf>
        <rdfs:comment xml:lang="en">The &apos;FireAlarmSystem&apos; class represents a fire alarm system installed in a building.</rdfs:comment>
        <rdfs:label xml:lang="en">FireAlarmSystem</rdfs:label>
    </owl:Class>
    


    <!-- https://purl.org/ffdr-ontology#FireBarrier -->


    <owl:Class rdf:about="https://purl.org/ffdr-ontology#FireBarrier">
        <rdfs:subClassOf rdf:resource="https://purl.org/ffdr-ontology#FireandSmokeProtectionElement"/>
        <rdfs:subClassOf>
            <owl:Restriction>
                <owl:onProperty rdf:resource="https://purl.org/ffdr-ontology#hasEnclosedArea"/>
                <owl:someValuesFrom rdf:resource="http://www.w3.org/2001/XMLSchema#string"/>
            </owl:Restriction>
        </rdfs:subClassOf>
        <rdfs:comment xml:lang="en">The &apos;FireBarrier&apos; class represents a fire barrier, which is a fire-resistance-rated wall assembly of materials designed to restrict the spread of fire in which continuity of the wall is maintained (IFC, 2018).</rdfs:comment>
        <rdfs:label xml:lang="en">FireBarrier</rdfs:label>
    </owl:Class>
    


    <!-- https://purl.org/ffdr-ontology#FireCommandCenter -->


    <owl:Class rdf:about="https://purl.org/ffdr-ontology#FireCommandCenter">
        <rdfs:subClassOf>
            <owl:Restriction>
                <owl:onProperty rdf:resource="https://purl.org/ffdr-ontology#contains"/>
                <owl:someValuesFrom rdf:resource="https://purl.org/ffdr-ontology#ControlPanel"/>
            </owl:Restriction>
        </rdfs:subClassOf>
        <rdfs:subClassOf>
            <owl:Restriction>
                <owl:onProperty rdf:resource="https://purl.org/ffdr-ontology#hasKeyLocated"/>
                <owl:someValuesFrom rdf:resource="http://www.w3.org/2001/XMLSchema#string"/>
            </owl:Restriction>
        </rdfs:subClassOf>
        <rdfs:subClassOf>
            <owl:Restriction>
                <owl:onProperty rdf:resource="https://purl.org/ffdr-ontology#hasLocation"/>
                <owl:someValuesFrom rdf:resource="http://www.w3.org/2001/XMLSchema#string"/>
            </owl:Restriction>
        </rdfs:subClassOf>
        <rdfs:comment xml:lang="en">The &apos;FireCommandCenter&apos; class represents A fire command center, which is a dedicated room or area where fire protection systems, alarms, and other emergency systems are monitored and controlled (NFPA 72).</rdfs:comment>
        <rdfs:label xml:lang="en">FireCommandCenter</rdfs:label>
    </owl:Class>
    


    <!-- https://purl.org/ffdr-ontology#FireDepartmentCommunicationSystemPanel -->


    <owl:Class rdf:about="https://purl.org/ffdr-ontology#FireDepartmentCommunicationSystemPanel">
        <rdfs:subClassOf rdf:resource="https://purl.org/ffdr-ontology#ControlPanel"/>
        <rdfs:comment xml:lang="en">The &apos;FireDepartmentCommunicationSystemPanel&apos; class represents a control panel used to control a fire department communication system that may be found in a building.</rdfs:comment>
        <rdfs:label xml:lang="en">FireDepartmentCommunicationSystemPanel</rdfs:label>
    </owl:Class>
    


    <!-- https://purl.org/ffdr-ontology#FireDepartmentConnection -->


    <owl:Class rdf:about="https://purl.org/ffdr-ontology#FireDepartmentConnection">
        <rdfs:subClassOf rdf:resource="https://purl.org/ffdr-ontology#BuildingSafetySystem"/>
        <rdfs:subClassOf>
            <owl:Restriction>
                <owl:onProperty rdf:resource="https://purl.org/ffdr-ontology#hasHoseConnection"/>
                <owl:someValuesFrom rdf:resource="https://purl.org/ffdr-ontology#HoseConnection"/>
            </owl:Restriction>
        </rdfs:subClassOf>
        <rdfs:subClassOf>
            <owl:Restriction>
                <owl:onProperty rdf:resource="https://purl.org/ffdr-ontology#hasWaterSource"/>
                <owl:someValuesFrom rdf:resource="https://purl.org/ffdr-ontology#WaterSource"/>
            </owl:Restriction>
        </rdfs:subClassOf>
        <rdfs:subClassOf>
            <owl:Restriction>
                <owl:onProperty rdf:resource="https://purl.org/ffdr-ontology#hasCoverageZone"/>
                <owl:someValuesFrom rdf:resource="http://www.w3.org/2001/XMLSchema#string"/>
            </owl:Restriction>
        </rdfs:subClassOf>
        <rdfs:subClassOf>
            <owl:Restriction>
                <owl:onProperty rdf:resource="https://purl.org/ffdr-ontology#hasDistanceFromWaterSource"/>
                <owl:someValuesFrom rdf:resource="http://www.w3.org/2001/XMLSchema#double"/>
            </owl:Restriction>
        </rdfs:subClassOf>
        <rdfs:subClassOf>
            <owl:Restriction>
                <owl:onProperty rdf:resource="https://purl.org/ffdr-ontology#hasLocation"/>
                <owl:someValuesFrom rdf:resource="http://www.w3.org/2001/XMLSchema#string"/>
            </owl:Restriction>
        </rdfs:subClassOf>
        <rdfs:subClassOf>
            <owl:Restriction>
                <owl:onProperty rdf:resource="https://purl.org/ffdr-ontology#hasNumberOfInlet"/>
                <owl:someValuesFrom rdf:resource="http://www.w3.org/2001/XMLSchema#int"/>
            </owl:Restriction>
        </rdfs:subClassOf>
        <rdfs:comment xml:lang="en">The &apos;FireDepartmentConnection&apos; class represents fire department connections (FDC) through which firefighters pump water into a standpipe system (NFPA 14).</rdfs:comment>
        <rdfs:label xml:lang="en">FireDepartmentConnection</rdfs:label>
    </owl:Class>
    


    <!-- https://purl.org/ffdr-ontology#FireHoseConnection -->


    <owl:Class rdf:about="https://purl.org/ffdr-ontology#FireHoseConnection">
        <rdfs:subClassOf rdf:resource="https://purl.org/ffdr-ontology#BuildingSafetySystem"/>
        <rdfs:subClassOf>
            <owl:Restriction>
                <owl:onProperty rdf:resource="https://purl.org/ffdr-ontology#hasHoseConnection"/>
                <owl:someValuesFrom rdf:resource="https://purl.org/ffdr-ontology#HoseConnection"/>
            </owl:Restriction>
        </rdfs:subClassOf>
        <rdfs:subClassOf>
            <owl:Restriction>
                <owl:onProperty rdf:resource="https://purl.org/ffdr-ontology#hasWaterSource"/>
                <owl:someValuesFrom rdf:resource="https://purl.org/ffdr-ontology#StandpipeSystem"/>
            </owl:Restriction>
        </rdfs:subClassOf>
        <rdfs:subClassOf>
            <owl:Restriction>
                <owl:onProperty rdf:resource="https://purl.org/ffdr-ontology#hasLocation"/>
                <owl:someValuesFrom rdf:resource="http://www.w3.org/2001/XMLSchema#string"/>
            </owl:Restriction>
        </rdfs:subClassOf>
        <rdfs:comment xml:lang="en">The &apos;FireHoseConnection&apos; class represents fire hose connections which are outlets of a standpipe system where firefighters connect their fire hose (NFPA 14).</rdfs:comment>
        <rdfs:label xml:lang="en">FireHoseConnection</rdfs:label>
    </owl:Class>
    


    <!-- https://purl.org/ffdr-ontology#FireHydrant -->


    <owl:Class rdf:about="https://purl.org/ffdr-ontology#FireHydrant">
        <rdfs:subClassOf rdf:resource="https://purl.org/ffdr-ontology#SurroundingStructure"/>
        <rdfs:subClassOf>
            <owl:Restriction>
                <owl:onProperty rdf:resource="https://purl.org/ffdr-ontology#hasHoseConnection"/>
                <owl:someValuesFrom rdf:resource="https://purl.org/ffdr-ontology#HoseConnection"/>
            </owl:Restriction>
        </rdfs:subClassOf>
        <rdfs:subClassOf>
            <owl:Restriction>
                <owl:onProperty rdf:resource="https://purl.org/ffdr-ontology#hasWaterSource"/>
                <owl:someValuesFrom rdf:resource="https://purl.org/ffdr-ontology#WaterSource"/>
            </owl:Restriction>
        </rdfs:subClassOf>
        <rdfs:subClassOf>
            <owl:Restriction>
                <owl:onProperty rdf:resource="https://purl.org/ffdr-ontology#hasDistanceFromFDC"/>
                <owl:someValuesFrom rdf:resource="http://www.w3.org/2001/XMLSchema#double"/>
            </owl:Restriction>
        </rdfs:subClassOf>
        <rdfs:subClassOf>
            <owl:Restriction>
                <owl:onProperty rdf:resource="https://purl.org/ffdr-ontology#hasFireFlow"/>
                <owl:someValuesFrom rdf:resource="http://www.w3.org/2001/XMLSchema#double"/>
            </owl:Restriction>
        </rdfs:subClassOf>
        <rdfs:subClassOf>
            <owl:Restriction>
                <owl:onProperty rdf:resource="https://purl.org/ffdr-ontology#hasNumberOfOutlet"/>
                <owl:someValuesFrom rdf:resource="http://www.w3.org/2001/XMLSchema#int"/>
            </owl:Restriction>
        </rdfs:subClassOf>
        <rdfs:subClassOf>
            <owl:Restriction>
                <owl:onProperty rdf:resource="https://purl.org/ffdr-ontology#hasType"/>
                <owl:someValuesFrom rdf:resource="http://www.w3.org/2001/XMLSchema#string"/>
            </owl:Restriction>
        </rdfs:subClassOf>
        <rdfs:subClassOf>
            <owl:Restriction>
                <owl:onProperty rdf:resource="https://purl.org/ffdr-ontology#isFunctional"/>
                <owl:someValuesFrom rdf:resource="http://www.w3.org/2001/XMLSchema#boolean"/>
            </owl:Restriction>
        </rdfs:subClassOf>
        <rdfs:comment xml:lang="en">The &apos;FireHydrant&apos; class represents fire hydrants, which are an important part of a fire suppression operation that provides firefighters with a hose connection to a water supply system (NFPA 24).</rdfs:comment>
        <rdfs:comment xml:lang="en">Type: Wet barrel hydrants (on pressurized water distribution systems), Dry barrel hydrants (used on static water supply sources)</rdfs:comment>
        <rdfs:label xml:lang="en">FireHydrant</rdfs:label>
    </owl:Class>
    


    <!-- https://purl.org/ffdr-ontology#FireLane -->


    <owl:Class rdf:about="https://purl.org/ffdr-ontology#FireLane">
        <rdfs:subClassOf rdf:resource="https://purl.org/ffdr-ontology#Road"/>
        <rdfs:subClassOf rdf:resource="https://purl.org/ffdr-ontology#SurroundingStructure"/>
        <rdfs:subClassOf>
            <owl:Restriction>
                <owl:onProperty rdf:resource="https://purl.org/ffdr-ontology#hasAccessBarrierType"/>
                <owl:someValuesFrom rdf:resource="http://www.w3.org/2001/XMLSchema#string"/>
            </owl:Restriction>
        </rdfs:subClassOf>
        <rdfs:subClassOf>
            <owl:Restriction>
                <owl:onProperty rdf:resource="https://purl.org/ffdr-ontology#hasAnglesOfApproach"/>
                <owl:someValuesFrom rdf:resource="http://www.w3.org/2001/XMLSchema#double"/>
            </owl:Restriction>
        </rdfs:subClassOf>
        <rdfs:subClassOf>
            <owl:Restriction>
                <owl:onProperty rdf:resource="https://purl.org/ffdr-ontology#hasTurningRadius"/>
                <owl:someValuesFrom rdf:resource="http://www.w3.org/2001/XMLSchema#double"/>
            </owl:Restriction>
        </rdfs:subClassOf>
        <rdfs:subClassOf>
            <owl:Restriction>
                <owl:onProperty rdf:resource="https://purl.org/ffdr-ontology#hasVerticalClearance"/>
                <owl:someValuesFrom rdf:resource="http://www.w3.org/2001/XMLSchema#double"/>
            </owl:Restriction>
        </rdfs:subClassOf>
        <owl:disjointWith rdf:resource="https://purl.org/ffdr-ontology#RoadToIncident"/>
        <rdfs:comment xml:lang="en">The &apos;FireLane&apos; class represents a fire lane, which is an access road designated for fire apparatus (NFPA 1).</rdfs:comment>
        <rdfs:label xml:lang="en">FireLane</rdfs:label>
    </owl:Class>
    


    <!-- https://purl.org/ffdr-ontology#FirePartition -->


    <owl:Class rdf:about="https://purl.org/ffdr-ontology#FirePartition">
        <rdfs:subClassOf rdf:resource="https://purl.org/ffdr-ontology#FireandSmokeProtectionElement"/>
        <rdfs:subClassOf>
            <owl:Restriction>
                <owl:onProperty rdf:resource="https://purl.org/ffdr-ontology#hasEnclosedArea"/>
                <owl:someValuesFrom rdf:resource="http://www.w3.org/2001/XMLSchema#string"/>
            </owl:Restriction>
        </rdfs:subClassOf>
        <rdfs:comment xml:lang="en">The &apos;FirePartition&apos; class represents a fire partition, which is a vertical assembly of materials designed to restrict the spread of fire while protecting openings (IFC, 2018).</rdfs:comment>
        <rdfs:label xml:lang="en">FirePartition</rdfs:label>
    </owl:Class>
    


    <!-- https://purl.org/ffdr-ontology#FirePump -->


    <owl:Class rdf:about="https://purl.org/ffdr-ontology#FirePump">
        <rdfs:subClassOf rdf:resource="https://purl.org/ffdr-ontology#BuildingSafetySystem"/>
        <rdfs:subClassOf>
            <owl:Restriction>
                <owl:onProperty rdf:resource="https://purl.org/ffdr-ontology#hasLocation"/>
                <owl:someValuesFrom rdf:resource="http://www.w3.org/2001/XMLSchema#string"/>
            </owl:Restriction>
        </rdfs:subClassOf>
        <rdfs:comment xml:lang="en">The &apos;FirePump&apos; class represents fire pumps which are used to boost the water pressure to standpipes and sprinkler systems (OSHA, 2015).</rdfs:comment>
        <rdfs:label xml:lang="en">FirePump</rdfs:label>
    </owl:Class>
    


    <!-- https://purl.org/ffdr-ontology#FireServiceOrganization -->


    <owl:Class rdf:about="https://purl.org/ffdr-ontology#FireServiceOrganization">
        <rdfs:subClassOf rdf:resource="https://purl.org/ffdr-ontology#EmergencyServiceProvider"/>
        <rdfs:comment xml:lang="en">The &apos;FireServiceOrganization&apos; class represents fire service organizations involved in a building fire emergency response.</rdfs:comment>
        <rdfs:label xml:lang="en">FireServiceOrganization</rdfs:label>
    </owl:Class>
    


    <!-- https://purl.org/ffdr-ontology#FireandSmokeProtectionElement -->


    <owl:Class rdf:about="https://purl.org/ffdr-ontology#FireandSmokeProtectionElement">
        <rdfs:subClassOf rdf:resource="https://purl.org/ffdr-ontology#BuildingSafetySystem"/>
        <rdfs:subClassOf>
            <owl:Restriction>
                <owl:onProperty rdf:resource="https://purl.org/ffdr-ontology#hasMaterial"/>
                <owl:someValuesFrom rdf:resource="https://purl.org/ffdr-ontology#Material"/>
            </owl:Restriction>
        </rdfs:subClassOf>
        <rdfs:subClassOf>
            <owl:Restriction>
                <owl:onProperty rdf:resource="https://purl.org/ffdr-ontology#hasLocation"/>
                <owl:someValuesFrom rdf:resource="http://www.w3.org/2001/XMLSchema#string"/>
            </owl:Restriction>
        </rdfs:subClassOf>
        <rdfs:subClassOf>
            <owl:Restriction>
                <owl:onProperty rdf:resource="https://purl.org/ffdr-ontology#hasFireResistanceRating"/>
                <owl:qualifiedCardinality rdf:datatype="http://www.w3.org/2001/XMLSchema#nonNegativeInteger">1</owl:qualifiedCardinality>
                <owl:onDataRange rdf:resource="http://www.w3.org/2001/XMLSchema#double"/>
            </owl:Restriction>
        </rdfs:subClassOf>
        <rdfs:comment xml:lang="en">The &apos;FireandSmokeProtectionElement&apos; class represents fire and smoke protection elements that can protect firefighters and building occupants (OSHA, 2015).</rdfs:comment>
        <rdfs:label xml:lang="en">FireandSmokeProtectionElement</rdfs:label>
    </owl:Class>
    


    <!-- https://purl.org/ffdr-ontology#Firewall -->


    <owl:Class rdf:about="https://purl.org/ffdr-ontology#Firewall">
        <rdfs:subClassOf rdf:resource="https://purl.org/ffdr-ontology#Facade"/>
        <rdfs:subClassOf rdf:resource="https://purl.org/ffdr-ontology#FireandSmokeProtectionElement"/>
        <rdfs:subClassOf>
            <owl:Restriction>
                <owl:onProperty rdf:resource="https://purl.org/ffdr-ontology#hasEnclosedArea"/>
                <owl:someValuesFrom rdf:resource="http://www.w3.org/2001/XMLSchema#string"/>
            </owl:Restriction>
        </rdfs:subClassOf>
        <rdfs:comment xml:lang="en">The &apos;Firewall&apos; class represents a firewall, which is a fire-resistance-rated wall that restricts the spread of fire while protecting openings and extending continuously from the foundation to or through the roof. It has sufficient structural stability under fire conditions to allow the structure to collapse without the collapse of the wall (IFC, 2018).</rdfs:comment>
        <rdfs:label xml:lang="en">Firewall</rdfs:label>
    </owl:Class>
    


    <!-- https://purl.org/ffdr-ontology#FloorAssembly -->


    <owl:Class rdf:about="https://purl.org/ffdr-ontology#FloorAssembly">
        <rdfs:subClassOf rdf:resource="https://purl.org/ffdr-ontology#NonStructuralElement"/>
        <rdfs:subClassOf>
            <owl:Restriction>
                <owl:onProperty rdf:resource="https://purl.org/ffdr-ontology#isLightweightConstruction"/>
                <owl:someValuesFrom rdf:resource="http://www.w3.org/2001/XMLSchema#boolean"/>
            </owl:Restriction>
        </rdfs:subClassOf>
        <rdfs:comment xml:lang="en">The &apos;FloorAssembly&apos; class represents the floor assembly in a building.</rdfs:comment>
        <rdfs:label xml:lang="en">FloorAssembly</rdfs:label>
    </owl:Class>
    


    <!-- https://purl.org/ffdr-ontology#GasDetector -->


    <owl:Class rdf:about="https://purl.org/ffdr-ontology#GasDetector">
        <rdfs:subClassOf rdf:resource="https://purl.org/ffdr-ontology#SensorDetector"/>
        <rdfs:comment xml:lang="en">The &apos;GasDetector&apos; class represents different gas detectors installed in a building.</rdfs:comment>
        <rdfs:label xml:lang="en">GasDetector</rdfs:label>
    </owl:Class>
    


    <!-- https://purl.org/ffdr-ontology#GasSupplySystem -->


    <owl:Class rdf:about="https://purl.org/ffdr-ontology#GasSupplySystem">
        <rdfs:subClassOf rdf:resource="https://purl.org/ffdr-ontology#BuildingUtilitySystem"/>
        <rdfs:comment xml:lang="en">The &apos;GasSupplySystem&apos; class represents a building&apos;s gas supply system.</rdfs:comment>
        <rdfs:label xml:lang="en">GasSupplySystem</rdfs:label>
    </owl:Class>
    


    <!-- https://purl.org/ffdr-ontology#Hallway -->


    <owl:Class rdf:about="https://purl.org/ffdr-ontology#Hallway">
        <rdfs:subClassOf rdf:resource="https://purl.org/ffdr-ontology#NonStructuralElement"/>
        <rdfs:subClassOf>
            <owl:Restriction>
                <owl:onProperty rdf:resource="https://purl.org/ffdr-ontology#hasCapacity"/>
                <owl:qualifiedCardinality rdf:datatype="http://www.w3.org/2001/XMLSchema#nonNegativeInteger">1</owl:qualifiedCardinality>
                <owl:onDataRange rdf:resource="http://www.w3.org/2001/XMLSchema#int"/>
            </owl:Restriction>
        </rdfs:subClassOf>
        <rdfs:subClassOf>
            <owl:Restriction>
                <owl:onProperty rdf:resource="https://purl.org/ffdr-ontology#hasWidth"/>
                <owl:qualifiedCardinality rdf:datatype="http://www.w3.org/2001/XMLSchema#nonNegativeInteger">1</owl:qualifiedCardinality>
                <owl:onDataRange rdf:resource="http://www.w3.org/2001/XMLSchema#double"/>
            </owl:Restriction>
        </rdfs:subClassOf>
        <rdfs:comment xml:lang="en">The &apos;Hallway&apos; class represents hallways in a building.</rdfs:comment>
        <rdfs:label xml:lang="en">Hallway</rdfs:label>
    </owl:Class>
    


    <!-- https://purl.org/ffdr-ontology#HazardousMaterial -->


    <owl:Class rdf:about="https://purl.org/ffdr-ontology#HazardousMaterial">
        <rdfs:subClassOf rdf:resource="https://purl.org/ffdr-ontology#SurroundingStructure"/>
        <rdfs:subClassOf>
            <owl:Restriction>
                <owl:onProperty rdf:resource="https://purl.org/ffdr-ontology#hasDescription"/>
                <owl:someValuesFrom rdf:resource="http://www.w3.org/2001/XMLSchema#string"/>
            </owl:Restriction>
        </rdfs:subClassOf>
        <rdfs:subClassOf>
            <owl:Restriction>
                <owl:onProperty rdf:resource="https://purl.org/ffdr-ontology#hasHazardLevel"/>
                <owl:someValuesFrom rdf:resource="http://www.w3.org/2001/XMLSchema#int"/>
            </owl:Restriction>
        </rdfs:subClassOf>
        <rdfs:subClassOf>
            <owl:Restriction>
                <owl:onProperty rdf:resource="https://purl.org/ffdr-ontology#hasSpecialHazard"/>
                <owl:someValuesFrom rdf:resource="http://www.w3.org/2001/XMLSchema#string"/>
            </owl:Restriction>
        </rdfs:subClassOf>
        <rdfs:comment xml:lang="en">The &apos;HazardousMaterial&apos; class represents any hazardous materials such as gas tanks and chemical storage.</rdfs:comment>
        <rdfs:label xml:lang="en">HazardousMaterial</rdfs:label>
    </owl:Class>
    


    <!-- https://purl.org/ffdr-ontology#HazardousSubstance -->


    <owl:Class rdf:about="https://purl.org/ffdr-ontology#HazardousSubstance">
        <rdfs:subClassOf rdf:resource="https://purl.org/ffdr-ontology#BuildingComponent"/>
        <rdfs:subClassOf>
            <owl:Restriction>
                <owl:onProperty rdf:resource="https://purl.org/ffdr-ontology#hasDescription"/>
                <owl:someValuesFrom rdf:resource="http://www.w3.org/2001/XMLSchema#string"/>
            </owl:Restriction>
        </rdfs:subClassOf>
        <rdfs:subClassOf>
            <owl:Restriction>
                <owl:onProperty rdf:resource="https://purl.org/ffdr-ontology#hasHazardLevel"/>
                <owl:someValuesFrom rdf:resource="http://www.w3.org/2001/XMLSchema#int"/>
            </owl:Restriction>
        </rdfs:subClassOf>
        <rdfs:subClassOf>
            <owl:Restriction>
                <owl:onProperty rdf:resource="https://purl.org/ffdr-ontology#hasLocation"/>
                <owl:someValuesFrom rdf:resource="http://www.w3.org/2001/XMLSchema#string"/>
            </owl:Restriction>
        </rdfs:subClassOf>
        <rdfs:subClassOf>
            <owl:Restriction>
                <owl:onProperty rdf:resource="https://purl.org/ffdr-ontology#hasSpecialHazard"/>
                <owl:someValuesFrom rdf:resource="http://www.w3.org/2001/XMLSchema#string"/>
            </owl:Restriction>
        </rdfs:subClassOf>
        <rdfs:subClassOf>
            <owl:Restriction>
                <owl:onProperty rdf:resource="https://purl.org/ffdr-ontology#isDecontaminationRequired"/>
                <owl:someValuesFrom rdf:resource="http://www.w3.org/2001/XMLSchema#boolean"/>
            </owl:Restriction>
        </rdfs:subClassOf>
        <rdfs:comment xml:lang="en">The &apos;HazardousSubstance&apos; class represents hazardous substances that may be found in a building.</rdfs:comment>
        <rdfs:label xml:lang="en">HazardousSubstance</rdfs:label>
    </owl:Class>
    


    <!-- https://purl.org/ffdr-ontology#Helipad -->


    <owl:Class rdf:about="https://purl.org/ffdr-ontology#Helipad">
        <rdfs:subClassOf rdf:resource="https://purl.org/ffdr-ontology#BuildingComponent"/>
        <rdfs:subClassOf>
            <owl:Restriction>
                <owl:onProperty rdf:resource="https://purl.org/ffdr-ontology#hasLocation"/>
                <owl:someValuesFrom rdf:resource="http://www.w3.org/2001/XMLSchema#string"/>
            </owl:Restriction>
        </rdfs:subClassOf>
        <rdfs:comment xml:lang="en">The &apos;Helipad&apos; class represents a helipad, which is an area for landing helicopters, that may be available on a building.</rdfs:comment>
        <rdfs:label xml:lang="en">Helipad</rdfs:label>
    </owl:Class>
    


    <!-- https://purl.org/ffdr-ontology#HoseConnection -->


    <owl:Class rdf:about="https://purl.org/ffdr-ontology#HoseConnection">
        <rdfs:subClassOf>
            <owl:Restriction>
                <owl:onProperty rdf:resource="https://purl.org/ffdr-ontology#hasSize"/>
                <owl:someValuesFrom rdf:resource="http://www.w3.org/2001/XMLSchema#double"/>
            </owl:Restriction>
        </rdfs:subClassOf>
        <rdfs:subClassOf>
            <owl:Restriction>
                <owl:onProperty rdf:resource="https://purl.org/ffdr-ontology#hasType"/>
                <owl:someValuesFrom rdf:resource="http://www.w3.org/2001/XMLSchema#string"/>
            </owl:Restriction>
        </rdfs:subClassOf>
        <rdfs:comment xml:lang="en">The &apos;HoseConnection&apos; class represents different hose connections used by firefighters during building fire emergencies.</rdfs:comment>
        <rdfs:comment xml:lang="en">Type could be threaded or quick- connect.</rdfs:comment>
        <rdfs:label xml:lang="en">HoseConnection</rdfs:label>
    </owl:Class>
    


    <!-- https://purl.org/ffdr-ontology#Hospital -->


    <owl:Class rdf:about="https://purl.org/ffdr-ontology#Hospital">
        <rdfs:subClassOf rdf:resource="https://purl.org/ffdr-ontology#EmergencyServiceProvider"/>
        <rdfs:comment xml:lang="en">The &apos;Hospital&apos; class represents hospitals.</rdfs:comment>
        <rdfs:label xml:lang="en">Hospital</rdfs:label>
    </owl:Class>
    


    <!-- https://purl.org/ffdr-ontology#HvacSystem -->


    <owl:Class rdf:about="https://purl.org/ffdr-ontology#HvacSystem">
        <rdfs:subClassOf rdf:resource="https://purl.org/ffdr-ontology#BuildingUtilitySystem"/>
        <rdfs:comment xml:lang="en">The &apos;HvacSystem&apos; class represents a building&apos;s heating, ventilation, and air conditioning (HVAC) system.</rdfs:comment>
        <rdfs:label xml:lang="en">HvacSystem</rdfs:label>
    </owl:Class>
    


    <!-- https://purl.org/ffdr-ontology#IncidentBuilding -->


    <owl:Class rdf:about="https://purl.org/ffdr-ontology#IncidentBuilding">
        <rdfs:subClassOf>
            <owl:Restriction>
                <owl:onProperty rdf:resource="https://purl.org/ffdr-ontology#hasAddress"/>
                <owl:someValuesFrom rdf:resource="https://purl.org/ffdr-ontology#Address"/>
            </owl:Restriction>
        </rdfs:subClassOf>
        <rdfs:subClassOf>
            <owl:Restriction>
                <owl:onProperty rdf:resource="https://purl.org/ffdr-ontology#hasBuildingPlan"/>
                <owl:someValuesFrom rdf:resource="https://purl.org/ffdr-ontology#BuildingPlan"/>
            </owl:Restriction>
        </rdfs:subClassOf>
        <rdfs:subClassOf>
            <owl:Restriction>
                <owl:onProperty rdf:resource="https://purl.org/ffdr-ontology#hasComponent"/>
                <owl:someValuesFrom rdf:resource="https://purl.org/ffdr-ontology#BuildingComponent"/>
            </owl:Restriction>
        </rdfs:subClassOf>
        <rdfs:subClassOf>
            <owl:Restriction>
                <owl:onProperty rdf:resource="https://purl.org/ffdr-ontology#hasOccupancy"/>
                <owl:someValuesFrom rdf:resource="https://purl.org/ffdr-ontology#BuildingOccupancy"/>
            </owl:Restriction>
        </rdfs:subClassOf>
        <rdfs:subClassOf>
            <owl:Restriction>
                <owl:onProperty rdf:resource="https://purl.org/ffdr-ontology#hasConstructionType"/>
                <owl:qualifiedCardinality rdf:datatype="http://www.w3.org/2001/XMLSchema#nonNegativeInteger">1</owl:qualifiedCardinality>
                <owl:onClass rdf:resource="https://purl.org/ffdr-ontology#ConstructionType"/>
            </owl:Restriction>
        </rdfs:subClassOf>
        <rdfs:subClassOf>
            <owl:Restriction>
                <owl:onProperty rdf:resource="https://purl.org/ffdr-ontology#hasBuildingArea"/>
                <owl:someValuesFrom rdf:resource="http://www.w3.org/2001/XMLSchema#double"/>
            </owl:Restriction>
        </rdfs:subClassOf>
        <rdfs:subClassOf>
            <owl:Restriction>
                <owl:onProperty rdf:resource="https://purl.org/ffdr-ontology#hasBuildingHeight"/>
                <owl:someValuesFrom rdf:resource="http://www.w3.org/2001/XMLSchema#double"/>
            </owl:Restriction>
        </rdfs:subClassOf>
        <rdfs:subClassOf>
            <owl:Restriction>
                <owl:onProperty rdf:resource="https://purl.org/ffdr-ontology#hasCondition"/>
                <owl:someValuesFrom rdf:resource="http://www.w3.org/2001/XMLSchema#string"/>
            </owl:Restriction>
        </rdfs:subClassOf>
        <rdfs:subClassOf>
            <owl:Restriction>
                <owl:onProperty rdf:resource="https://purl.org/ffdr-ontology#includeHazardousOperation"/>
                <owl:someValuesFrom rdf:resource="http://www.w3.org/2001/XMLSchema#boolean"/>
            </owl:Restriction>
        </rdfs:subClassOf>
        <rdfs:subClassOf>
            <owl:Restriction>
                <owl:onProperty rdf:resource="https://purl.org/ffdr-ontology#hasNumberOfExit"/>
                <owl:qualifiedCardinality rdf:datatype="http://www.w3.org/2001/XMLSchema#nonNegativeInteger">1</owl:qualifiedCardinality>
                <owl:onDataRange rdf:resource="http://www.w3.org/2001/XMLSchema#int"/>
            </owl:Restriction>
        </rdfs:subClassOf>
        <rdfs:subClassOf>
            <owl:Restriction>
                <owl:onProperty rdf:resource="https://purl.org/ffdr-ontology#hasNumberOfStory"/>
                <owl:qualifiedCardinality rdf:datatype="http://www.w3.org/2001/XMLSchema#nonNegativeInteger">1</owl:qualifiedCardinality>
                <owl:onDataRange rdf:resource="http://www.w3.org/2001/XMLSchema#int"/>
            </owl:Restriction>
        </rdfs:subClassOf>
        <rdfs:subClassOf>
            <owl:Restriction>
                <owl:onProperty rdf:resource="https://purl.org/ffdr-ontology#hasNumberOfSublevel"/>
                <owl:qualifiedCardinality rdf:datatype="http://www.w3.org/2001/XMLSchema#nonNegativeInteger">1</owl:qualifiedCardinality>
                <owl:onDataRange rdf:resource="http://www.w3.org/2001/XMLSchema#int"/>
            </owl:Restriction>
        </rdfs:subClassOf>
        <rdfs:subClassOf>
            <owl:Restriction>
                <owl:onProperty rdf:resource="https://purl.org/ffdr-ontology#hasOccupantLoad"/>
                <owl:qualifiedCardinality rdf:datatype="http://www.w3.org/2001/XMLSchema#nonNegativeInteger">1</owl:qualifiedCardinality>
                <owl:onDataRange rdf:resource="http://www.w3.org/2001/XMLSchema#int"/>
            </owl:Restriction>
        </rdfs:subClassOf>
        <rdfs:comment xml:lang="en">The &apos;Incidentbuilding&apos; class represents a building with a fire emergency.</rdfs:comment>
        <rdfs:label xml:lang="en">IncidentBuilding</rdfs:label>
    </owl:Class>
    


    <!-- https://purl.org/ffdr-ontology#IncidentSite -->


    <owl:Class rdf:about="https://purl.org/ffdr-ontology#IncidentSite">
        <rdfs:subClassOf>
            <owl:Restriction>
                <owl:onProperty rdf:resource="https://purl.org/ffdr-ontology#contains"/>
                <owl:someValuesFrom rdf:resource="https://purl.org/ffdr-ontology#FireCommandCenter"/>
            </owl:Restriction>
        </rdfs:subClassOf>
        <rdfs:subClassOf>
            <owl:Restriction>
                <owl:onProperty rdf:resource="https://purl.org/ffdr-ontology#contains"/>
                <owl:someValuesFrom rdf:resource="https://purl.org/ffdr-ontology#IncidentBuilding"/>
            </owl:Restriction>
        </rdfs:subClassOf>
        <rdfs:subClassOf>
            <owl:Restriction>
                <owl:onProperty rdf:resource="https://purl.org/ffdr-ontology#contains"/>
                <owl:someValuesFrom rdf:resource="https://purl.org/ffdr-ontology#SurroundingStructure"/>
            </owl:Restriction>
        </rdfs:subClassOf>
        <rdfs:subClassOf>
            <owl:Restriction>
                <owl:onProperty rdf:resource="https://purl.org/ffdr-ontology#contains"/>
                <owl:someValuesFrom rdf:resource="https://purl.org/ffdr-ontology#SurroundingTerrain"/>
            </owl:Restriction>
        </rdfs:subClassOf>
        <rdfs:subClassOf>
            <owl:Restriction>
                <owl:onProperty rdf:resource="https://purl.org/ffdr-ontology#hasAddress"/>
                <owl:someValuesFrom rdf:resource="https://purl.org/ffdr-ontology#PublicSafetyAgencyContactAddress"/>
            </owl:Restriction>
        </rdfs:subClassOf>
        <rdfs:subClassOf>
            <owl:Restriction>
                <owl:onProperty rdf:resource="https://purl.org/ffdr-ontology#hasWeatherCondition"/>
                <owl:someValuesFrom rdf:resource="https://purl.org/ffdr-ontology#WeatherCondition"/>
            </owl:Restriction>
        </rdfs:subClassOf>
        <rdfs:subClassOf>
            <owl:Restriction>
                <owl:onProperty rdf:resource="https://purl.org/ffdr-ontology#hasDemography"/>
                <owl:someValuesFrom rdf:resource="http://www.w3.org/2001/XMLSchema#string"/>
            </owl:Restriction>
        </rdfs:subClassOf>
        <rdfs:comment xml:lang="en">The &apos;IncidentSite&apos; class represents a site where a building fire emergency has occurred.</rdfs:comment>
        <rdfs:label xml:lang="en">IncidentSite</rdfs:label>
    </owl:Class>
    


    <!-- https://purl.org/ffdr-ontology#KeyBox -->


    <owl:Class rdf:about="https://purl.org/ffdr-ontology#KeyBox">
        <rdfs:subClassOf rdf:resource="https://purl.org/ffdr-ontology#BuildingComponent"/>
        <rdfs:subClassOf>
            <owl:Restriction>
                <owl:onProperty rdf:resource="https://purl.org/ffdr-ontology#hasKey"/>
                <owl:someValuesFrom rdf:resource="http://www.w3.org/2001/XMLSchema#string"/>
            </owl:Restriction>
        </rdfs:subClassOf>
        <rdfs:subClassOf>
            <owl:Restriction>
                <owl:onProperty rdf:resource="https://purl.org/ffdr-ontology#hasLocation"/>
                <owl:someValuesFrom rdf:resource="http://www.w3.org/2001/XMLSchema#string"/>
            </owl:Restriction>
        </rdfs:subClassOf>
        <rdfs:comment xml:lang="en">The &apos;KeyBox&apos; class represents key boxes,  which are small vaults placed in a building or nearby that contain keys to a building&apos;s doors, elevators, and other rooms (OSHA, 2015).</rdfs:comment>
        <rdfs:label xml:lang="en">KeyBox</rdfs:label>
    </owl:Class>
    


    <!-- https://purl.org/ffdr-ontology#MassNotificationSystem -->


    <owl:Class rdf:about="https://purl.org/ffdr-ontology#MassNotificationSystem">
        <rdfs:subClassOf rdf:resource="https://purl.org/ffdr-ontology#BuildingSafetySystem"/>
        <rdfs:subClassOf>
            <owl:Restriction>
                <owl:onProperty rdf:resource="https://purl.org/ffdr-ontology#hasControlPanel"/>
                <owl:someValuesFrom rdf:resource="https://purl.org/ffdr-ontology#MassNotificationSystemControlPanel"/>
            </owl:Restriction>
        </rdfs:subClassOf>
        <rdfs:subClassOf>
            <owl:Restriction>
                <owl:onProperty rdf:resource="https://purl.org/ffdr-ontology#hasCoverageZone"/>
                <owl:someValuesFrom rdf:resource="http://www.w3.org/2001/XMLSchema#string"/>
            </owl:Restriction>
        </rdfs:subClassOf>
        <rdfs:subClassOf>
            <owl:Restriction>
                <owl:onProperty rdf:resource="https://purl.org/ffdr-ontology#hasType"/>
                <owl:someValuesFrom rdf:resource="http://www.w3.org/2001/XMLSchema#string"/>
            </owl:Restriction>
        </rdfs:subClassOf>
        <rdfs:comment xml:lang="en">Notification type could be auditory or visual or both.</rdfs:comment>
        <rdfs:comment xml:lang="en">The &apos;MassNotificationSystem&apos; class represents a mass notification system that is used by firefighters to provide clear instruction to building occupants (OSHA, 2015).</rdfs:comment>
        <rdfs:label xml:lang="en">MassNotificationSystem</rdfs:label>
    </owl:Class>
    


    <!-- https://purl.org/ffdr-ontology#MassNotificationSystemControlPanel -->


    <owl:Class rdf:about="https://purl.org/ffdr-ontology#MassNotificationSystemControlPanel">
        <rdfs:subClassOf rdf:resource="https://purl.org/ffdr-ontology#ControlPanel"/>
        <rdfs:comment xml:lang="en">The &apos;MassNotificationSystemControlPanel&apos; class represents a control panel used to control a mass notification system that may be found in a building.</rdfs:comment>
        <rdfs:label xml:lang="en">MassNotificationSystemControlPanel</rdfs:label>
    </owl:Class>
    


    <!-- https://purl.org/ffdr-ontology#Material -->


    <owl:Class rdf:about="https://purl.org/ffdr-ontology#Material">
        <rdfs:comment xml:lang="en">The &apos;Material&apos; class represents the constituting materials of different elements.</rdfs:comment>
        <rdfs:label xml:lang="en">Material</rdfs:label>
    </owl:Class>
    


    <!-- https://purl.org/ffdr-ontology#MunicipalDistributionSystem -->


    <owl:Class rdf:about="https://purl.org/ffdr-ontology#MunicipalDistributionSystem">
        <rdfs:subClassOf rdf:resource="https://purl.org/ffdr-ontology#WaterSource"/>
        <rdfs:subClassOf>
            <owl:Restriction>
                <owl:onProperty rdf:resource="https://purl.org/ffdr-ontology#hasPressure"/>
                <owl:someValuesFrom rdf:resource="http://www.w3.org/2001/XMLSchema#double"/>
            </owl:Restriction>
        </rdfs:subClassOf>
        <owl:disjointWith rdf:resource="https://purl.org/ffdr-ontology#StaticWaterSource"/>
        <rdfs:comment xml:lang="en">The &apos;MunicipalDistributionSystem&apos; class represents a water distribution system provided and maintained by municipalities or similar entities.</rdfs:comment>
        <rdfs:label xml:lang="en">MunicipalDistributionSystem</rdfs:label>
    </owl:Class>
    


    <!-- https://purl.org/ffdr-ontology#NonStructuralElement -->


    <owl:Class rdf:about="https://purl.org/ffdr-ontology#NonStructuralElement">
        <rdfs:subClassOf rdf:resource="https://purl.org/ffdr-ontology#BuildingComponent"/>
        <rdfs:subClassOf>
            <owl:Restriction>
                <owl:onProperty rdf:resource="https://purl.org/ffdr-ontology#hasMaterial"/>
                <owl:someValuesFrom rdf:resource="https://purl.org/ffdr-ontology#Material"/>
            </owl:Restriction>
        </rdfs:subClassOf>
        <rdfs:subClassOf>
            <owl:Restriction>
                <owl:onProperty rdf:resource="https://purl.org/ffdr-ontology#hasID"/>
                <owl:someValuesFrom rdf:resource="http://www.w3.org/2001/XMLSchema#string"/>
            </owl:Restriction>
        </rdfs:subClassOf>
        <rdfs:subClassOf>
            <owl:Restriction>
                <owl:onProperty rdf:resource="https://purl.org/ffdr-ontology#hasLocation"/>
                <owl:someValuesFrom rdf:resource="http://www.w3.org/2001/XMLSchema#string"/>
            </owl:Restriction>
        </rdfs:subClassOf>
        <rdfs:subClassOf>
            <owl:Restriction>
                <owl:onProperty rdf:resource="https://purl.org/ffdr-ontology#hasFireResistanceRating"/>
                <owl:maxQualifiedCardinality rdf:datatype="http://www.w3.org/2001/XMLSchema#nonNegativeInteger">1</owl:maxQualifiedCardinality>
                <owl:onDataRange rdf:resource="http://www.w3.org/2001/XMLSchema#double"/>
            </owl:Restriction>
        </rdfs:subClassOf>
        <rdfs:comment xml:lang="en">The &apos;NonStructuralElement&apos; class represents the non-structural elements of a building.</rdfs:comment>
        <rdfs:label xml:lang="en">NonStructuralElement</rdfs:label>
    </owl:Class>
    


    <!-- https://purl.org/ffdr-ontology#Obstruction -->


    <owl:Class rdf:about="https://purl.org/ffdr-ontology#Obstruction">
        <rdfs:subClassOf rdf:resource="https://purl.org/ffdr-ontology#SurroundingStructure"/>
        <rdfs:subClassOf>
            <owl:Restriction>
                <owl:onProperty rdf:resource="https://purl.org/ffdr-ontology#hasDescription"/>
                <owl:someValuesFrom rdf:resource="http://www.w3.org/2001/XMLSchema#string"/>
            </owl:Restriction>
        </rdfs:subClassOf>
        <rdfs:subClassOf>
            <owl:Restriction>
                <owl:onProperty rdf:resource="https://purl.org/ffdr-ontology#hasType"/>
                <owl:someValuesFrom rdf:resource="http://www.w3.org/2001/XMLSchema#string"/>
            </owl:Restriction>
        </rdfs:subClassOf>
        <rdfs:comment xml:lang="en">The &apos;Obstruction&apos; class represents structures nearby the building, such as fences that can obstruct firefighters&apos; and fire trucks&apos; movement.</rdfs:comment>
        <rdfs:label xml:lang="en">Obstruction</rdfs:label>
    </owl:Class>
    


    <!-- https://purl.org/ffdr-ontology#OwnerContactAddress -->


    <owl:Class rdf:about="https://purl.org/ffdr-ontology#OwnerContactAddress">
        <rdfs:subClassOf rdf:resource="https://purl.org/ffdr-ontology#Address"/>
        <rdfs:comment xml:lang="en">The &apos;OwnerContactAddress&apos; class represents a building owner&apos;s contact address.</rdfs:comment>
        <rdfs:label xml:lang="en">OwnerContactAddress</rdfs:label>
    </owl:Class>
    


    <!-- https://purl.org/ffdr-ontology#ParkingLot -->


    <owl:Class rdf:about="https://purl.org/ffdr-ontology#ParkingLot">
        <rdfs:subClassOf rdf:resource="https://purl.org/ffdr-ontology#SurroundingStructure"/>
        <rdfs:subClassOf>
            <owl:Restriction>
                <owl:onProperty rdf:resource="https://purl.org/ffdr-ontology#hasArea"/>
                <owl:someValuesFrom rdf:resource="http://www.w3.org/2001/XMLSchema#double"/>
            </owl:Restriction>
        </rdfs:subClassOf>
        <rdfs:comment xml:lang="en">The &apos;ParkingLot&apos; class represents parking lots.</rdfs:comment>
        <rdfs:label xml:lang="en">ParkingLot</rdfs:label>
    </owl:Class>
    


    <!-- https://purl.org/ffdr-ontology#Pipeline -->


    <owl:Class rdf:about="https://purl.org/ffdr-ontology#Pipeline">
        <rdfs:subClassOf rdf:resource="https://purl.org/ffdr-ontology#SurroundingStructure"/>
        <rdfs:comment xml:lang="en">The &apos;Pipeline&apos; class represents pipelines located near an incident building.</rdfs:comment>
        <rdfs:label xml:lang="en">Pipeline</rdfs:label>
    </owl:Class>
    


    <!-- https://purl.org/ffdr-ontology#PoliceDepartment -->


    <owl:Class rdf:about="https://purl.org/ffdr-ontology#PoliceDepartment">
        <rdfs:subClassOf rdf:resource="https://purl.org/ffdr-ontology#EmergencyServiceProvider"/>
        <rdfs:comment xml:lang="en">The &apos;PoliceDepartment&apos; class represents police departments.</rdfs:comment>
        <rdfs:label xml:lang="en">PoliceDepartment</rdfs:label>
    </owl:Class>
    


    <!-- https://purl.org/ffdr-ontology#PortableFireExtinguisher -->


    <owl:Class rdf:about="https://purl.org/ffdr-ontology#PortableFireExtinguisher">
        <rdfs:subClassOf rdf:resource="https://purl.org/ffdr-ontology#BuildingSafetySystem"/>
        <rdfs:subClassOf>
            <owl:Restriction>
                <owl:onProperty rdf:resource="https://purl.org/ffdr-ontology#hasFireExtinguisherRating"/>
                <owl:someValuesFrom rdf:resource="http://www.w3.org/2001/XMLSchema#string"/>
            </owl:Restriction>
        </rdfs:subClassOf>
        <rdfs:subClassOf>
            <owl:Restriction>
                <owl:onProperty rdf:resource="https://purl.org/ffdr-ontology#hasLocation"/>
                <owl:someValuesFrom rdf:resource="http://www.w3.org/2001/XMLSchema#string"/>
            </owl:Restriction>
        </rdfs:subClassOf>
        <rdfs:subClassOf>
            <owl:Restriction>
                <owl:onProperty rdf:resource="https://purl.org/ffdr-ontology#hasType"/>
                <owl:someValuesFrom rdf:resource="http://www.w3.org/2001/XMLSchema#string"/>
            </owl:Restriction>
        </rdfs:subClassOf>
        <rdfs:comment xml:lang="en">Has different type such as:   Air-Water;  Air-Foam;  Wet Chemical;  Dry Chemical Powder; Carbon Dioxide and Vaporising Liquid.</rdfs:comment>
        <rdfs:comment xml:lang="en">The &apos;PortableFireExtinguisher&apos; class represents portable fire extinguishers placed throughout a building.</rdfs:comment>
        <rdfs:label xml:lang="en">PortableFireExtinguisher</rdfs:label>
    </owl:Class>
    


    <!-- https://purl.org/ffdr-ontology#PowerLine -->


    <owl:Class rdf:about="https://purl.org/ffdr-ontology#PowerLine">
        <rdfs:subClassOf rdf:resource="https://purl.org/ffdr-ontology#SurroundingStructure"/>
        <rdfs:comment xml:lang="en">The &apos;PowerLine&apos; class represents power lines located near an incident building.</rdfs:comment>
        <rdfs:label xml:lang="en">PowerLine</rdfs:label>
    </owl:Class>
    


    <!-- https://purl.org/ffdr-ontology#PrimaryPowerSupplySystem -->


    <owl:Class rdf:about="https://purl.org/ffdr-ontology#PrimaryPowerSupplySystem">
        <rdfs:subClassOf rdf:resource="https://purl.org/ffdr-ontology#BuildingUtilitySystem"/>
        <rdfs:comment xml:lang="en">The &apos;PrimaryPowerSupplySystem&apos; class represents a building&apos;s primary power supply system.</rdfs:comment>
        <rdfs:label xml:lang="en">PrimaryPowerSupplySystem</rdfs:label>
    </owl:Class>
    


    <!-- https://purl.org/ffdr-ontology#PublicSafetyAgencyContactAddress -->


    <owl:Class rdf:about="https://purl.org/ffdr-ontology#PublicSafetyAgencyContactAddress">
        <rdfs:subClassOf rdf:resource="https://purl.org/ffdr-ontology#Address"/>
        <rdfs:comment xml:lang="en">The &apos;PublicSafetyAgencyContactAddress&apos; class represents public safety agencies&apos;s contact address.</rdfs:comment>
        <rdfs:label xml:lang="en">PublicSafetyAgencyContactAddress</rdfs:label>
    </owl:Class>
    


    <!-- https://purl.org/ffdr-ontology#Ramp -->


    <owl:Class rdf:about="https://purl.org/ffdr-ontology#Ramp">
        <rdfs:subClassOf rdf:resource="https://purl.org/ffdr-ontology#NonStructuralElement"/>
        <rdfs:subClassOf>
            <owl:Restriction>
                <owl:onProperty rdf:resource="https://purl.org/ffdr-ontology#hasFireExtinguishingSystem"/>
                <owl:someValuesFrom rdf:resource="https://purl.org/ffdr-ontology#AutomaticFireExtinguishingSystem"/>
            </owl:Restriction>
        </rdfs:subClassOf>
        <rdfs:subClassOf>
            <owl:Restriction>
                <owl:onProperty rdf:resource="https://purl.org/ffdr-ontology#hasDirectionToExit"/>
                <owl:someValuesFrom rdf:resource="http://www.w3.org/2001/XMLSchema#string"/>
            </owl:Restriction>
        </rdfs:subClassOf>
        <rdfs:subClassOf>
            <owl:Restriction>
                <owl:onProperty rdf:resource="https://purl.org/ffdr-ontology#hasDischargeLevel"/>
                <owl:someValuesFrom rdf:resource="http://www.w3.org/2001/XMLSchema#string"/>
            </owl:Restriction>
        </rdfs:subClassOf>
        <rdfs:subClassOf>
            <owl:Restriction>
                <owl:onProperty rdf:resource="https://purl.org/ffdr-ontology#hasFloorsServed"/>
                <owl:someValuesFrom rdf:resource="http://www.w3.org/2001/XMLSchema#string"/>
            </owl:Restriction>
        </rdfs:subClassOf>
        <rdfs:subClassOf>
            <owl:Restriction>
                <owl:onProperty rdf:resource="https://purl.org/ffdr-ontology#isRoofAccess"/>
                <owl:someValuesFrom rdf:resource="http://www.w3.org/2001/XMLSchema#boolean"/>
            </owl:Restriction>
        </rdfs:subClassOf>
        <rdfs:subClassOf>
            <owl:Restriction>
                <owl:onProperty rdf:resource="https://purl.org/ffdr-ontology#hasCapacity"/>
                <owl:qualifiedCardinality rdf:datatype="http://www.w3.org/2001/XMLSchema#nonNegativeInteger">1</owl:qualifiedCardinality>
                <owl:onDataRange rdf:resource="http://www.w3.org/2001/XMLSchema#int"/>
            </owl:Restriction>
        </rdfs:subClassOf>
        <rdfs:subClassOf>
            <owl:Restriction>
                <owl:onProperty rdf:resource="https://purl.org/ffdr-ontology#hasExitTravelDistances"/>
                <owl:qualifiedCardinality rdf:datatype="http://www.w3.org/2001/XMLSchema#nonNegativeInteger">1</owl:qualifiedCardinality>
                <owl:onDataRange rdf:resource="http://www.w3.org/2001/XMLSchema#double"/>
            </owl:Restriction>
        </rdfs:subClassOf>
        <rdfs:subClassOf>
            <owl:Restriction>
                <owl:onProperty rdf:resource="https://purl.org/ffdr-ontology#hasWidth"/>
                <owl:qualifiedCardinality rdf:datatype="http://www.w3.org/2001/XMLSchema#nonNegativeInteger">1</owl:qualifiedCardinality>
                <owl:onDataRange rdf:resource="http://www.w3.org/2001/XMLSchema#double"/>
            </owl:Restriction>
        </rdfs:subClassOf>
        <rdfs:subClassOf>
            <owl:Restriction>
                <owl:onProperty rdf:resource="https://purl.org/ffdr-ontology#isExit"/>
                <owl:qualifiedCardinality rdf:datatype="http://www.w3.org/2001/XMLSchema#nonNegativeInteger">1</owl:qualifiedCardinality>
                <owl:onDataRange rdf:resource="http://www.w3.org/2001/XMLSchema#boolean"/>
            </owl:Restriction>
        </rdfs:subClassOf>
        <rdfs:comment xml:lang="en">The &apos;Ramp&apos; class represents ramps that may be found in a building.</rdfs:comment>
        <rdfs:label xml:lang="en">Ramp</rdfs:label>
    </owl:Class>
    


    <!-- https://purl.org/ffdr-ontology#Road -->


    <owl:Class rdf:about="https://purl.org/ffdr-ontology#Road">
        <rdfs:subClassOf>
            <owl:Restriction>
                <owl:onProperty rdf:resource="https://purl.org/ffdr-ontology#hasMaterial"/>
                <owl:someValuesFrom rdf:resource="https://purl.org/ffdr-ontology#Material"/>
            </owl:Restriction>
        </rdfs:subClassOf>
        <rdfs:subClassOf>
            <owl:Restriction>
                <owl:onProperty rdf:resource="https://purl.org/ffdr-ontology#hasCondition"/>
                <owl:someValuesFrom rdf:resource="http://www.w3.org/2001/XMLSchema#string"/>
            </owl:Restriction>
        </rdfs:subClassOf>
        <rdfs:subClassOf>
            <owl:Restriction>
                <owl:onProperty rdf:resource="https://purl.org/ffdr-ontology#hasSlope"/>
                <owl:someValuesFrom rdf:resource="http://www.w3.org/2001/XMLSchema#double"/>
            </owl:Restriction>
        </rdfs:subClassOf>
        <rdfs:subClassOf>
            <owl:Restriction>
                <owl:onProperty rdf:resource="https://purl.org/ffdr-ontology#hasType"/>
                <owl:someValuesFrom rdf:resource="http://www.w3.org/2001/XMLSchema#string"/>
            </owl:Restriction>
        </rdfs:subClassOf>
        <rdfs:subClassOf>
            <owl:Restriction>
                <owl:onProperty rdf:resource="https://purl.org/ffdr-ontology#hasWidth"/>
                <owl:someValuesFrom rdf:resource="http://www.w3.org/2001/XMLSchema#double"/>
            </owl:Restriction>
        </rdfs:subClassOf>
        <rdfs:comment xml:lang="en">The &apos;Road&apos; class represents roads.</rdfs:comment>
        <rdfs:label xml:lang="en">Road</rdfs:label>
    </owl:Class>
    


    <!-- https://purl.org/ffdr-ontology#RoadToIncident -->


    <owl:Class rdf:about="https://purl.org/ffdr-ontology#RoadToIncident">
        <rdfs:subClassOf rdf:resource="https://purl.org/ffdr-ontology#Road"/>
        <rdfs:subClassOf>
            <owl:Restriction>
                <owl:onProperty rdf:resource="https://purl.org/ffdr-ontology#hasTrafficLevel"/>
                <owl:someValuesFrom rdf:resource="http://www.w3.org/2001/XMLSchema#string"/>
            </owl:Restriction>
        </rdfs:subClassOf>
        <rdfs:comment xml:lang="en">The &apos;RoadToIncident&apos; class represents a road that leads to an incident site.</rdfs:comment>
        <rdfs:label xml:lang="en">RoadToIncident</rdfs:label>
    </owl:Class>
    


    <!-- https://purl.org/ffdr-ontology#RoofAssembly -->


    <owl:Class rdf:about="https://purl.org/ffdr-ontology#RoofAssembly">
        <rdfs:subClassOf rdf:resource="https://purl.org/ffdr-ontology#NonStructuralElement"/>
        <rdfs:subClassOf>
            <owl:Restriction>
                <owl:onProperty rdf:resource="https://purl.org/ffdr-ontology#isAccessible"/>
                <owl:someValuesFrom rdf:resource="http://www.w3.org/2001/XMLSchema#boolean"/>
            </owl:Restriction>
        </rdfs:subClassOf>
        <rdfs:subClassOf>
            <owl:Restriction>
                <owl:onProperty rdf:resource="https://purl.org/ffdr-ontology#isLightweightConstruction"/>
                <owl:someValuesFrom rdf:resource="http://www.w3.org/2001/XMLSchema#boolean"/>
            </owl:Restriction>
        </rdfs:subClassOf>
        <rdfs:comment xml:lang="en">The &apos;RoofAssembly&apos; class represents the roof assembly in a building.</rdfs:comment>
        <rdfs:label xml:lang="en">RoofAssembly</rdfs:label>
    </owl:Class>
    


    <!-- https://purl.org/ffdr-ontology#RoofTopElement -->


    <owl:Class rdf:about="https://purl.org/ffdr-ontology#RoofTopElement">
        <rdfs:subClassOf rdf:resource="https://purl.org/ffdr-ontology#BuildingComponent"/>
        <rdfs:subClassOf>
            <owl:Restriction>
                <owl:onProperty rdf:resource="https://purl.org/ffdr-ontology#hasDescription"/>
                <owl:someValuesFrom rdf:resource="http://www.w3.org/2001/XMLSchema#string"/>
            </owl:Restriction>
        </rdfs:subClassOf>
        <rdfs:subClassOf>
            <owl:Restriction>
                <owl:onProperty rdf:resource="https://purl.org/ffdr-ontology#hasLocation"/>
                <owl:someValuesFrom rdf:resource="http://www.w3.org/2001/XMLSchema#string"/>
            </owl:Restriction>
        </rdfs:subClassOf>
        <rdfs:subClassOf>
            <owl:Restriction>
                <owl:onProperty rdf:resource="https://purl.org/ffdr-ontology#hasType"/>
                <owl:someValuesFrom rdf:resource="http://www.w3.org/2001/XMLSchema#string"/>
            </owl:Restriction>
        </rdfs:subClassOf>
        <rdfs:comment xml:lang="en">The &apos;RoofTopElement&apos; class represents roof-top elements, such as skylights, photovoltaic panels, vegetation, and Other Obstructions (cables, wires, ropes).</rdfs:comment>
        <rdfs:label xml:lang="en">RoofTopElement</rdfs:label>
    </owl:Class>
    


    <!-- https://purl.org/ffdr-ontology#SensorDetector -->


    <owl:Class rdf:about="https://purl.org/ffdr-ontology#SensorDetector">
        <rdfs:subClassOf rdf:resource="https://purl.org/ffdr-ontology#BuildingSafetySystem"/>
        <rdfs:subClassOf>
            <owl:Restriction>
                <owl:onProperty rdf:resource="https://purl.org/ffdr-ontology#hasCoverageZone"/>
                <owl:someValuesFrom rdf:resource="http://www.w3.org/2001/XMLSchema#string"/>
            </owl:Restriction>
        </rdfs:subClassOf>
        <rdfs:subClassOf>
            <owl:Restriction>
                <owl:onProperty rdf:resource="https://purl.org/ffdr-ontology#isInAlarm"/>
                <owl:someValuesFrom rdf:resource="http://www.w3.org/2001/XMLSchema#boolean"/>
            </owl:Restriction>
        </rdfs:subClassOf>
        <rdfs:comment xml:lang="en">The &apos;SensorDetector&apos; class represents different sensors and detectors installed in a building.</rdfs:comment>
        <rdfs:label xml:lang="en">SensorDetector</rdfs:label>
    </owl:Class>
    


    <!-- https://purl.org/ffdr-ontology#ShaftEnclosure -->


    <owl:Class rdf:about="https://purl.org/ffdr-ontology#ShaftEnclosure">
        <rdfs:subClassOf rdf:resource="https://purl.org/ffdr-ontology#FireandSmokeProtectionElement"/>
        <rdfs:comment xml:lang="en">The &apos;ShaftEnclosure&apos; class represents a shaft enclosure that protects vertical openings.</rdfs:comment>
        <rdfs:label xml:lang="en">ShaftEnclosure</rdfs:label>
    </owl:Class>
    


    <!-- https://purl.org/ffdr-ontology#SmokeBarrier -->


    <owl:Class rdf:about="https://purl.org/ffdr-ontology#SmokeBarrier">
        <rdfs:subClassOf rdf:resource="https://purl.org/ffdr-ontology#FireandSmokeProtectionElement"/>
        <rdfs:subClassOf>
            <owl:Restriction>
                <owl:onProperty rdf:resource="https://purl.org/ffdr-ontology#hasEnclosedArea"/>
                <owl:someValuesFrom rdf:resource="http://www.w3.org/2001/XMLSchema#string"/>
            </owl:Restriction>
        </rdfs:subClassOf>
        <rdfs:comment xml:lang="en">The &apos;SmokeBarrier&apos; class represents a smoke barrier, which is a continuous vertical or horizontal membrane (such as a wall, floor, or ceiling assembly) that restricts the movement of smoke (IFC 2018).</rdfs:comment>
        <rdfs:label xml:lang="en">SmokeBarrier</rdfs:label>
    </owl:Class>
    


    <!-- https://purl.org/ffdr-ontology#SmokeControlSystem -->


    <owl:Class rdf:about="https://purl.org/ffdr-ontology#SmokeControlSystem">
        <rdfs:subClassOf rdf:resource="https://purl.org/ffdr-ontology#BuildingSafetySystem"/>
        <rdfs:subClassOf>
            <owl:Restriction>
                <owl:onProperty rdf:resource="https://purl.org/ffdr-ontology#hasControlPanel"/>
                <owl:someValuesFrom rdf:resource="https://purl.org/ffdr-ontology#SmokeControlSystemControlPanel"/>
            </owl:Restriction>
        </rdfs:subClassOf>
        <rdfs:subClassOf>
            <owl:Restriction>
                <owl:onProperty rdf:resource="https://purl.org/ffdr-ontology#hasCoverageZone"/>
                <owl:someValuesFrom rdf:resource="http://www.w3.org/2001/XMLSchema#string"/>
            </owl:Restriction>
        </rdfs:subClassOf>
        <rdfs:subClassOf>
            <owl:Restriction>
                <owl:onProperty rdf:resource="https://purl.org/ffdr-ontology#hasType"/>
                <owl:someValuesFrom rdf:resource="http://www.w3.org/2001/XMLSchema#string"/>
            </owl:Restriction>
        </rdfs:subClassOf>
        <rdfs:subClassOf>
            <owl:Restriction>
                <owl:onProperty rdf:resource="https://purl.org/ffdr-ontology#isSystemActivated"/>
                <owl:someValuesFrom rdf:resource="http://www.w3.org/2001/XMLSchema#boolean"/>
            </owl:Restriction>
        </rdfs:subClassOf>
        <rdfs:comment xml:lang="en">System type could be: smoke exhaust systems and stair pressurization systems</rdfs:comment>
        <rdfs:comment xml:lang="en">The &apos;SmokeControlSystem&apos; class represents a smoke control system that supports the protection of building occupants while they evacuate the building (OSHA, 2015).</rdfs:comment>
        <rdfs:label xml:lang="en">SmokeControlSystem</rdfs:label>
    </owl:Class>
    


    <!-- https://purl.org/ffdr-ontology#SmokeControlSystemControlPanel -->


    <owl:Class rdf:about="https://purl.org/ffdr-ontology#SmokeControlSystemControlPanel">
        <rdfs:subClassOf rdf:resource="https://purl.org/ffdr-ontology#ControlPanel"/>
        <rdfs:comment xml:lang="en">The &apos;SmokeControlSystemControlPanel&apos; class represents a control panel used to control a smoke control system that may be found in a building.</rdfs:comment>
        <rdfs:label xml:lang="en">SmokeControlSystemControlPanel</rdfs:label>
    </owl:Class>
    


    <!-- https://purl.org/ffdr-ontology#SmokePartition -->


    <owl:Class rdf:about="https://purl.org/ffdr-ontology#SmokePartition">
        <rdfs:subClassOf rdf:resource="https://purl.org/ffdr-ontology#FireandSmokeProtectionElement"/>
        <rdfs:subClassOf>
            <owl:Restriction>
                <owl:onProperty rdf:resource="https://purl.org/ffdr-ontology#hasEnclosedArea"/>
                <owl:someValuesFrom rdf:resource="http://www.w3.org/2001/XMLSchema#string"/>
            </owl:Restriction>
        </rdfs:subClassOf>
        <rdfs:comment xml:lang="en">The &apos;SmokePartition&apos; class represents a smoke partition, which is a wall assembly that limits the transfer of smoke (IFC, 2018).</rdfs:comment>
        <rdfs:label xml:lang="en">SmokePartition</rdfs:label>
    </owl:Class>
    


    <!-- https://purl.org/ffdr-ontology#SmokeandHeatRemovalSystem -->


    <owl:Class rdf:about="https://purl.org/ffdr-ontology#SmokeandHeatRemovalSystem">
        <rdfs:subClassOf rdf:resource="https://purl.org/ffdr-ontology#BuildingSafetySystem"/>
        <rdfs:subClassOf>
            <owl:Restriction>
                <owl:onProperty rdf:resource="https://purl.org/ffdr-ontology#hasLocation"/>
                <owl:someValuesFrom rdf:resource="http://www.w3.org/2001/XMLSchema#string"/>
            </owl:Restriction>
        </rdfs:subClassOf>
        <rdfs:subClassOf>
            <owl:Restriction>
                <owl:onProperty rdf:resource="https://purl.org/ffdr-ontology#hasType"/>
                <owl:someValuesFrom rdf:resource="http://www.w3.org/2001/XMLSchema#string"/>
            </owl:Restriction>
        </rdfs:subClassOf>
        <rdfs:subClassOf>
            <owl:Restriction>
                <owl:onProperty rdf:resource="https://purl.org/ffdr-ontology#isSystemActivated"/>
                <owl:someValuesFrom rdf:resource="http://www.w3.org/2001/XMLSchema#boolean"/>
            </owl:Restriction>
        </rdfs:subClassOf>
        <rdfs:comment xml:lang="en">The &apos;SmokeandHeatRemovalSystem&apos; class represents a smoke and heat removal system that assists firefighters in removing smoke after a fire is extinguished (OSHA, 2015).</rdfs:comment>
        <rdfs:label xml:lang="en">SmokeandHeatRemovalSystem</rdfs:label>
    </owl:Class>
    


    <!-- https://purl.org/ffdr-ontology#Stairway -->


    <owl:Class rdf:about="https://purl.org/ffdr-ontology#Stairway">
        <rdfs:subClassOf rdf:resource="https://purl.org/ffdr-ontology#NonStructuralElement"/>
        <rdfs:subClassOf>
            <owl:Restriction>
                <owl:onProperty rdf:resource="https://purl.org/ffdr-ontology#hasFireExtinguishingSystem"/>
                <owl:someValuesFrom rdf:resource="https://purl.org/ffdr-ontology#AutomaticFireExtinguishingSystem"/>
            </owl:Restriction>
        </rdfs:subClassOf>
        <rdfs:subClassOf>
            <owl:Restriction>
                <owl:onProperty rdf:resource="https://purl.org/ffdr-ontology#hasDirectionToExit"/>
                <owl:someValuesFrom rdf:resource="http://www.w3.org/2001/XMLSchema#string"/>
            </owl:Restriction>
        </rdfs:subClassOf>
        <rdfs:subClassOf>
            <owl:Restriction>
                <owl:onProperty rdf:resource="https://purl.org/ffdr-ontology#hasDischargeLevel"/>
                <owl:someValuesFrom rdf:resource="http://www.w3.org/2001/XMLSchema#string"/>
            </owl:Restriction>
        </rdfs:subClassOf>
        <rdfs:subClassOf>
            <owl:Restriction>
                <owl:onProperty rdf:resource="https://purl.org/ffdr-ontology#hasFloorsServed"/>
                <owl:someValuesFrom rdf:resource="http://www.w3.org/2001/XMLSchema#string"/>
            </owl:Restriction>
        </rdfs:subClassOf>
        <rdfs:subClassOf>
            <owl:Restriction>
                <owl:onProperty rdf:resource="https://purl.org/ffdr-ontology#isRoofAccess"/>
                <owl:someValuesFrom rdf:resource="http://www.w3.org/2001/XMLSchema#boolean"/>
            </owl:Restriction>
        </rdfs:subClassOf>
        <rdfs:subClassOf>
            <owl:Restriction>
                <owl:onProperty rdf:resource="https://purl.org/ffdr-ontology#hasCapacity"/>
                <owl:qualifiedCardinality rdf:datatype="http://www.w3.org/2001/XMLSchema#nonNegativeInteger">1</owl:qualifiedCardinality>
                <owl:onDataRange rdf:resource="http://www.w3.org/2001/XMLSchema#int"/>
            </owl:Restriction>
        </rdfs:subClassOf>
        <rdfs:subClassOf>
            <owl:Restriction>
                <owl:onProperty rdf:resource="https://purl.org/ffdr-ontology#hasExitTravelDistances"/>
                <owl:qualifiedCardinality rdf:datatype="http://www.w3.org/2001/XMLSchema#nonNegativeInteger">1</owl:qualifiedCardinality>
                <owl:onDataRange rdf:resource="http://www.w3.org/2001/XMLSchema#double"/>
            </owl:Restriction>
        </rdfs:subClassOf>
        <rdfs:subClassOf>
            <owl:Restriction>
                <owl:onProperty rdf:resource="https://purl.org/ffdr-ontology#hasWidth"/>
                <owl:qualifiedCardinality rdf:datatype="http://www.w3.org/2001/XMLSchema#nonNegativeInteger">1</owl:qualifiedCardinality>
                <owl:onDataRange rdf:resource="http://www.w3.org/2001/XMLSchema#double"/>
            </owl:Restriction>
        </rdfs:subClassOf>
        <rdfs:subClassOf>
            <owl:Restriction>
                <owl:onProperty rdf:resource="https://purl.org/ffdr-ontology#isExit"/>
                <owl:qualifiedCardinality rdf:datatype="http://www.w3.org/2001/XMLSchema#nonNegativeInteger">1</owl:qualifiedCardinality>
                <owl:onDataRange rdf:resource="http://www.w3.org/2001/XMLSchema#boolean"/>
            </owl:Restriction>
        </rdfs:subClassOf>
        <rdfs:comment xml:lang="en">The &apos;Stairway&apos; class represents stairways that may be found in a building.</rdfs:comment>
        <rdfs:label xml:lang="en">Stairway</rdfs:label>
    </owl:Class>
    


    <!-- https://purl.org/ffdr-ontology#StandpipeSystem -->


    <owl:Class rdf:about="https://purl.org/ffdr-ontology#StandpipeSystem">
        <rdfs:subClassOf rdf:resource="https://purl.org/ffdr-ontology#BuildingSafetySystem"/>
        <rdfs:subClassOf>
            <owl:Restriction>
                <owl:onProperty rdf:resource="https://purl.org/ffdr-ontology#hasWaterSource"/>
                <owl:someValuesFrom>
                    <owl:Class>
                        <owl:unionOf rdf:parseType="Collection">
                            <rdf:Description rdf:about="https://purl.org/ffdr-ontology#FireDepartmentConnection"/>
                            <rdf:Description rdf:about="https://purl.org/ffdr-ontology#WaterSource"/>
                        </owl:unionOf>
                    </owl:Class>
                </owl:someValuesFrom>
            </owl:Restriction>
        </rdfs:subClassOf>
        <rdfs:subClassOf>
            <owl:Restriction>
                <owl:onProperty rdf:resource="https://purl.org/ffdr-ontology#hasClass"/>
                <owl:someValuesFrom rdf:resource="http://www.w3.org/2001/XMLSchema#string"/>
            </owl:Restriction>
        </rdfs:subClassOf>
        <rdfs:subClassOf>
            <owl:Restriction>
                <owl:onProperty rdf:resource="https://purl.org/ffdr-ontology#hasCoverageZone"/>
                <owl:someValuesFrom rdf:resource="http://www.w3.org/2001/XMLSchema#string"/>
            </owl:Restriction>
        </rdfs:subClassOf>
        <rdfs:subClassOf>
            <owl:Restriction>
                <owl:onProperty rdf:resource="https://purl.org/ffdr-ontology#hasIsolationValveLocation"/>
                <owl:someValuesFrom rdf:resource="http://www.w3.org/2001/XMLSchema#string"/>
            </owl:Restriction>
        </rdfs:subClassOf>
        <rdfs:subClassOf>
            <owl:Restriction>
                <owl:onProperty rdf:resource="https://purl.org/ffdr-ontology#hasRequiredMaximumPressure"/>
                <owl:someValuesFrom rdf:resource="http://www.w3.org/2001/XMLSchema#double"/>
            </owl:Restriction>
        </rdfs:subClassOf>
        <rdfs:subClassOf>
            <owl:Restriction>
                <owl:onProperty rdf:resource="https://purl.org/ffdr-ontology#hasRequiredMinimumPressure"/>
                <owl:someValuesFrom rdf:resource="http://www.w3.org/2001/XMLSchema#double"/>
            </owl:Restriction>
        </rdfs:subClassOf>
        <rdfs:subClassOf>
            <owl:Restriction>
                <owl:onProperty rdf:resource="https://purl.org/ffdr-ontology#hasType"/>
                <owl:someValuesFrom rdf:resource="http://www.w3.org/2001/XMLSchema#string"/>
            </owl:Restriction>
        </rdfs:subClassOf>
        <rdfs:subClassOf>
            <owl:Restriction>
                <owl:onProperty rdf:resource="https://purl.org/ffdr-ontology#isIsolationValveOpen"/>
                <owl:someValuesFrom rdf:resource="http://www.w3.org/2001/XMLSchema#boolean"/>
            </owl:Restriction>
        </rdfs:subClassOf>
        <rdfs:comment xml:lang="en">Properties:

has water source: Automatic water supply, manual supply through FDC, Or both

has Class: fire service use (Class I), occupant use (Class II), or combined fire service and occupant use (Class III)

has type: Wet (automatic or manual) and Dry</rdfs:comment>
        <rdfs:comment xml:lang="en">The &apos;StandpipeSystem&apos; class represents a standpipe system which is a system of pipes within a building that provides water to fire hose connections and, in some cases, to sprinkler systems (NFPA 14).</rdfs:comment>
        <rdfs:label xml:lang="en">StandpipeSystem</rdfs:label>
    </owl:Class>
    


    <!-- https://purl.org/ffdr-ontology#StaticWaterSource -->


    <owl:Class rdf:about="https://purl.org/ffdr-ontology#StaticWaterSource">
        <rdfs:subClassOf rdf:resource="https://purl.org/ffdr-ontology#WaterSource"/>
        <rdfs:subClassOf>
            <owl:Restriction>
                <owl:onProperty rdf:resource="https://purl.org/ffdr-ontology#hasDistanceFromFDC"/>
                <owl:someValuesFrom rdf:resource="http://www.w3.org/2001/XMLSchema#double"/>
            </owl:Restriction>
        </rdfs:subClassOf>
        <rdfs:subClassOf>
            <owl:Restriction>
                <owl:onProperty rdf:resource="https://purl.org/ffdr-ontology#hasDistanceFromIncidentBuilding"/>
                <owl:someValuesFrom rdf:resource="http://www.w3.org/2001/XMLSchema#double"/>
            </owl:Restriction>
        </rdfs:subClassOf>
        <rdfs:subClassOf>
            <owl:Restriction>
                <owl:onProperty rdf:resource="https://purl.org/ffdr-ontology#hasLocation"/>
                <owl:someValuesFrom rdf:resource="http://www.w3.org/2001/XMLSchema#string"/>
            </owl:Restriction>
        </rdfs:subClassOf>
        <rdfs:subClassOf>
            <owl:Restriction>
                <owl:onProperty rdf:resource="https://purl.org/ffdr-ontology#hasType"/>
                <owl:someValuesFrom rdf:resource="http://www.w3.org/2001/XMLSchema#string"/>
            </owl:Restriction>
        </rdfs:subClassOf>
        <rdfs:comment xml:lang="en">The &apos;StaticWaterSource&apos; class represents static water sources that can be used for fire suppression.</rdfs:comment>
        <rdfs:comment xml:lang="en">Type: Lakes, ponds, cisterns, fountains, swimming pools, reservoirs, pressure tanks, and elevated tanks.</rdfs:comment>
        <rdfs:label xml:lang="en">StaticWaterSource</rdfs:label>
    </owl:Class>
    


    <!-- https://purl.org/ffdr-ontology#StructuralElement -->


    <owl:Class rdf:about="https://purl.org/ffdr-ontology#StructuralElement">
        <rdfs:subClassOf rdf:resource="https://purl.org/ffdr-ontology#BuildingComponent"/>
        <rdfs:subClassOf>
            <owl:Restriction>
                <owl:onProperty rdf:resource="https://purl.org/ffdr-ontology#hasMaterial"/>
                <owl:someValuesFrom rdf:resource="https://purl.org/ffdr-ontology#Material"/>
            </owl:Restriction>
        </rdfs:subClassOf>
        <rdfs:subClassOf>
            <owl:Restriction>
                <owl:onProperty rdf:resource="https://purl.org/ffdr-ontology#hasLocation"/>
                <owl:someValuesFrom rdf:resource="http://www.w3.org/2001/XMLSchema#string"/>
            </owl:Restriction>
        </rdfs:subClassOf>
        <rdfs:subClassOf>
            <owl:Restriction>
                <owl:onProperty rdf:resource="https://purl.org/ffdr-ontology#hasFireResistanceRating"/>
                <owl:maxQualifiedCardinality rdf:datatype="http://www.w3.org/2001/XMLSchema#nonNegativeInteger">1</owl:maxQualifiedCardinality>
                <owl:onDataRange rdf:resource="http://www.w3.org/2001/XMLSchema#double"/>
            </owl:Restriction>
        </rdfs:subClassOf>
        <rdfs:comment xml:lang="en">The &apos;StructuralElement&apos; class represents the structural elements of a building.</rdfs:comment>
        <rdfs:label xml:lang="en">StructuralElement</rdfs:label>
    </owl:Class>
    


    <!-- https://purl.org/ffdr-ontology#SurroundingStructure -->


    <owl:Class rdf:about="https://purl.org/ffdr-ontology#SurroundingStructure">
        <rdfs:subClassOf>
            <owl:Restriction>
                <owl:onProperty rdf:resource="https://purl.org/ffdr-ontology#hasDistanceFromIncidentBuilding"/>
                <owl:someValuesFrom rdf:resource="http://www.w3.org/2001/XMLSchema#double"/>
            </owl:Restriction>
        </rdfs:subClassOf>
        <rdfs:subClassOf>
            <owl:Restriction>
                <owl:onProperty rdf:resource="https://purl.org/ffdr-ontology#hasLocation"/>
                <owl:someValuesFrom rdf:resource="http://www.w3.org/2001/XMLSchema#string"/>
            </owl:Restriction>
        </rdfs:subClassOf>
        <rdfs:comment xml:lang="en">The &apos;SurroundingStructure&apos; class represents structures surrounding an incident building (the building with a fire emergency).</rdfs:comment>
        <rdfs:label xml:lang="en">SurroundingStructure</rdfs:label>
    </owl:Class>
    


    <!-- https://purl.org/ffdr-ontology#SurroundingTerrain -->


    <owl:Class rdf:about="https://purl.org/ffdr-ontology#SurroundingTerrain">
        <rdfs:subClassOf>
            <owl:Restriction>
                <owl:onProperty rdf:resource="https://purl.org/ffdr-ontology#hasSlope"/>
                <owl:someValuesFrom rdf:resource="http://www.w3.org/2001/XMLSchema#double"/>
            </owl:Restriction>
        </rdfs:subClassOf>
        <rdfs:comment xml:lang="en">The &apos;SurroundingTerrain&apos; class represents terrain surrounding an incident building (the building with a fire emergency).</rdfs:comment>
        <rdfs:label xml:lang="en">SurroundingTerrain</rdfs:label>
    </owl:Class>
    


    <!-- https://purl.org/ffdr-ontology#UtilityContactAddress -->


    <owl:Class rdf:about="https://purl.org/ffdr-ontology#UtilityContactAddress">
        <rdfs:subClassOf rdf:resource="https://purl.org/ffdr-ontology#Address"/>
        <rdfs:comment>The &apos;UtilityContactAddress&apos; class represents the address of people that manage the utilities in a building.</rdfs:comment>
        <rdfs:label xml:lang="en">UtilityContactAddress</rdfs:label>
    </owl:Class>
    


    <!-- https://purl.org/ffdr-ontology#UtilityControlPanel -->


    <owl:Class rdf:about="https://purl.org/ffdr-ontology#UtilityControlPanel">
        <rdfs:subClassOf rdf:resource="https://purl.org/ffdr-ontology#ControlPanel"/>
        <rdfs:comment xml:lang="en">The &apos;UtilityControlPanel&apos; class represents control panels used to control different utilities found in a building.</rdfs:comment>
        <rdfs:label xml:lang="en">UtilityControlPanel</rdfs:label>
    </owl:Class>
    


    <!-- https://purl.org/ffdr-ontology#Vegetation -->


    <owl:Class rdf:about="https://purl.org/ffdr-ontology#Vegetation">
        <rdfs:subClassOf rdf:resource="https://purl.org/ffdr-ontology#SurroundingStructure"/>
        <rdfs:subClassOf>
            <owl:Restriction>
                <owl:onProperty rdf:resource="https://purl.org/ffdr-ontology#hasFlammabilityLevel"/>
                <owl:someValuesFrom rdf:resource="http://www.w3.org/2001/XMLSchema#int"/>
            </owl:Restriction>
        </rdfs:subClassOf>
        <rdfs:subClassOf>
            <owl:Restriction>
                <owl:onProperty rdf:resource="https://purl.org/ffdr-ontology#hasSpecies"/>
                <owl:someValuesFrom rdf:resource="http://www.w3.org/2001/XMLSchema#string"/>
            </owl:Restriction>
        </rdfs:subClassOf>
        <rdfs:comment xml:lang="en">The &apos;vegetation&apos; class represents vegetation nearby an incident building.</rdfs:comment>
        <rdfs:label xml:lang="en">Vegetation</rdfs:label>
    </owl:Class>
    


    <!-- https://purl.org/ffdr-ontology#VerticalOpening -->


    <owl:Class rdf:about="https://purl.org/ffdr-ontology#VerticalOpening">
        <rdfs:subClassOf rdf:resource="https://purl.org/ffdr-ontology#BuildingComponent"/>
        <rdfs:subClassOf>
            <owl:Restriction>
                <owl:onProperty rdf:resource="https://purl.org/ffdr-ontology#hasShaftEnclosure"/>
                <owl:someValuesFrom rdf:resource="https://purl.org/ffdr-ontology#ShaftEnclosure"/>
            </owl:Restriction>
        </rdfs:subClassOf>
        <rdfs:subClassOf>
            <owl:Restriction>
                <owl:onProperty rdf:resource="https://purl.org/ffdr-ontology#hasDescription"/>
                <owl:someValuesFrom rdf:resource="http://www.w3.org/2001/XMLSchema#string"/>
            </owl:Restriction>
        </rdfs:subClassOf>
        <rdfs:subClassOf>
            <owl:Restriction>
                <owl:onProperty rdf:resource="https://purl.org/ffdr-ontology#hasLocation"/>
                <owl:someValuesFrom rdf:resource="http://www.w3.org/2001/XMLSchema#string"/>
            </owl:Restriction>
        </rdfs:subClassOf>
        <rdfs:comment xml:lang="en">The &apos;VerticalOpening&apos; class represents vertical Openings that may be found in a building.</rdfs:comment>
        <rdfs:label xml:lang="en">VerticalOpening</rdfs:label>
    </owl:Class>
    


    <!-- https://purl.org/ffdr-ontology#Wall -->


    <owl:Class rdf:about="https://purl.org/ffdr-ontology#Wall">
        <rdfs:subClassOf rdf:resource="https://purl.org/ffdr-ontology#NonStructuralElement"/>
        <rdfs:subClassOf>
            <owl:Restriction>
                <owl:onProperty rdf:resource="https://purl.org/ffdr-ontology#hasThickness"/>
                <owl:someValuesFrom rdf:resource="http://www.w3.org/2001/XMLSchema#double"/>
            </owl:Restriction>
        </rdfs:subClassOf>
        <rdfs:comment xml:lang="en">The &apos;Wall&apos; class represents walls in a building.</rdfs:comment>
        <rdfs:label xml:lang="en">Wall</rdfs:label>
    </owl:Class>
    


    <!-- https://purl.org/ffdr-ontology#WaterSource -->


    <owl:Class rdf:about="https://purl.org/ffdr-ontology#WaterSource">
        <rdfs:subClassOf>
            <owl:Restriction>
                <owl:onProperty rdf:resource="https://purl.org/ffdr-ontology#hasFireFlow"/>
                <owl:someValuesFrom rdf:resource="http://www.w3.org/2001/XMLSchema#double"/>
            </owl:Restriction>
        </rdfs:subClassOf>
        <rdfs:subClassOf>
            <owl:Restriction>
                <owl:onProperty rdf:resource="https://purl.org/ffdr-ontology#isFunctional"/>
                <owl:someValuesFrom rdf:resource="http://www.w3.org/2001/XMLSchema#boolean"/>
            </owl:Restriction>
        </rdfs:subClassOf>
        <rdfs:comment xml:lang="en">The &apos;WaterSource&apos; class represents different water sources that can be used for fire suppression.</rdfs:comment>
        <rdfs:label>WaterSource</rdfs:label>
    </owl:Class>
    


    <!-- https://purl.org/ffdr-ontology#WaterSupplyandSewerageSystem -->


    <owl:Class rdf:about="https://purl.org/ffdr-ontology#WaterSupplyandSewerageSystem">
        <rdfs:subClassOf rdf:resource="https://purl.org/ffdr-ontology#BuildingUtilitySystem"/>
        <rdfs:comment xml:lang="en">The &apos;WaterSupplyandSewerageSystem&apos; class represents a building&apos;s water supply and sewerage system.</rdfs:comment>
        <rdfs:label xml:lang="en">WaterSupplyandSewerageSystem</rdfs:label>
    </owl:Class>
    


    <!-- https://purl.org/ffdr-ontology#WeatherCondition -->


    <owl:Class rdf:about="https://purl.org/ffdr-ontology#WeatherCondition">
        <rdfs:subClassOf>
            <owl:Restriction>
                <owl:onProperty rdf:resource="https://purl.org/ffdr-ontology#hasPrecipitationValue"/>
                <owl:someValuesFrom rdf:resource="http://www.w3.org/2001/XMLSchema#double"/>
            </owl:Restriction>
        </rdfs:subClassOf>
        <rdfs:subClassOf>
            <owl:Restriction>
                <owl:onProperty rdf:resource="https://purl.org/ffdr-ontology#hasRelativeHumidity"/>
                <owl:someValuesFrom rdf:resource="http://www.w3.org/2001/XMLSchema#double"/>
            </owl:Restriction>
        </rdfs:subClassOf>
        <rdfs:subClassOf>
            <owl:Restriction>
                <owl:onProperty rdf:resource="https://purl.org/ffdr-ontology#hasTemperature"/>
                <owl:someValuesFrom rdf:resource="http://www.w3.org/2001/XMLSchema#double"/>
            </owl:Restriction>
        </rdfs:subClassOf>
        <rdfs:subClassOf>
            <owl:Restriction>
                <owl:onProperty rdf:resource="https://purl.org/ffdr-ontology#hasTimeMark"/>
                <owl:someValuesFrom rdf:resource="http://www.w3.org/2001/XMLSchema#dateTimeStamp"/>
            </owl:Restriction>
        </rdfs:subClassOf>
        <rdfs:subClassOf>
            <owl:Restriction>
                <owl:onProperty rdf:resource="https://purl.org/ffdr-ontology#hasWindDirection"/>
                <owl:someValuesFrom rdf:resource="http://www.w3.org/2001/XMLSchema#string"/>
            </owl:Restriction>
        </rdfs:subClassOf>
        <rdfs:subClassOf>
            <owl:Restriction>
                <owl:onProperty rdf:resource="https://purl.org/ffdr-ontology#hasWindSpeed"/>
                <owl:someValuesFrom rdf:resource="http://www.w3.org/2001/XMLSchema#double"/>
            </owl:Restriction>
        </rdfs:subClassOf>
        <rdfs:comment xml:lang="en">The &apos;WeatherCondition&apos; class represents weather-related information.</rdfs:comment>
        <rdfs:label xml:lang="en">WeatherCondition</rdfs:label>
    </owl:Class>
    


    <!-- https://purl.org/ffdr-ontology#Window -->


    <owl:Class rdf:about="https://purl.org/ffdr-ontology#Window">
        <rdfs:subClassOf rdf:resource="https://purl.org/ffdr-ontology#NonStructuralElement"/>
        <rdfs:subClassOf>
            <owl:Restriction>
                <owl:onProperty rdf:resource="https://purl.org/ffdr-ontology#hasHeight"/>
                <owl:someValuesFrom rdf:resource="http://www.w3.org/2001/XMLSchema#double"/>
            </owl:Restriction>
        </rdfs:subClassOf>
        <rdfs:subClassOf>
            <owl:Restriction>
                <owl:onProperty rdf:resource="https://purl.org/ffdr-ontology#hasOpeningDirection"/>
                <owl:someValuesFrom rdf:resource="http://www.w3.org/2001/XMLSchema#string"/>
            </owl:Restriction>
        </rdfs:subClassOf>
        <rdfs:subClassOf>
            <owl:Restriction>
                <owl:onProperty rdf:resource="https://purl.org/ffdr-ontology#isFunctional"/>
                <owl:someValuesFrom rdf:resource="http://www.w3.org/2001/XMLSchema#boolean"/>
            </owl:Restriction>
        </rdfs:subClassOf>
        <rdfs:subClassOf>
            <owl:Restriction>
                <owl:onProperty rdf:resource="https://purl.org/ffdr-ontology#isOnExterior"/>
                <owl:someValuesFrom rdf:resource="http://www.w3.org/2001/XMLSchema#boolean"/>
            </owl:Restriction>
        </rdfs:subClassOf>
        <rdfs:subClassOf>
            <owl:Restriction>
                <owl:onProperty rdf:resource="https://purl.org/ffdr-ontology#isShaftway"/>
                <owl:someValuesFrom rdf:resource="http://www.w3.org/2001/XMLSchema#boolean"/>
            </owl:Restriction>
        </rdfs:subClassOf>
        <rdfs:subClassOf>
            <owl:Restriction>
                <owl:onProperty rdf:resource="https://purl.org/ffdr-ontology#hasWidth"/>
                <owl:qualifiedCardinality rdf:datatype="http://www.w3.org/2001/XMLSchema#nonNegativeInteger">1</owl:qualifiedCardinality>
                <owl:onDataRange rdf:resource="http://www.w3.org/2001/XMLSchema#double"/>
            </owl:Restriction>
        </rdfs:subClassOf>
        <rdfs:comment xml:lang="en">The &apos;Window&apos; class represents windows in a building.</rdfs:comment>
        <rdfs:label xml:lang="en">Window</rdfs:label>
    </owl:Class>
    


    <!-- 
    ///////////////////////////////////////////////////////////////////////////////////////
    //
    // Individuals
    //
    ///////////////////////////////////////////////////////////////////////////////////////
     -->


    


    <!-- https://purl.org/ffdr-ontology#Assembly -->


    <owl:NamedIndividual rdf:about="https://purl.org/ffdr-ontology#Assembly">
        <rdf:type rdf:resource="https://purl.org/ffdr-ontology#BuildingOccupancy"/>
        <rdfs:comment xml:lang="en">The &apos;Assembly&apos; class represents assembly occupancy, which includes, among others, the use of a building for the gathering of people (IBC, 2018).</rdfs:comment>
        <rdfs:label xml:lang="en">Assembly</rdfs:label>
    </owl:NamedIndividual>
    


    <!-- https://purl.org/ffdr-ontology#Business -->


    <owl:NamedIndividual rdf:about="https://purl.org/ffdr-ontology#Business">
        <rdf:type rdf:resource="https://purl.org/ffdr-ontology#BuildingOccupancy"/>
        <rdfs:comment xml:lang="en">The &apos;Business&apos; class represents business occupancy, which includes, among others,  the use of a building for office, professional or service-type transactions, including storage of records and accounts (IBC, 2018).</rdfs:comment>
        <rdfs:label xml:lang="en">Business</rdfs:label>
    </owl:NamedIndividual>
    


    <!-- https://purl.org/ffdr-ontology#Educational -->


    <owl:NamedIndividual rdf:about="https://purl.org/ffdr-ontology#Educational">
        <rdf:type rdf:resource="https://purl.org/ffdr-ontology#BuildingOccupancy"/>
        <rdfs:comment xml:lang="en">The &apos;Educational&apos; class represents educational occupancy, which includes, among others, the use of a building for educational purposes (IBC, 2018).</rdfs:comment>
        <rdfs:label xml:lang="en">Educational</rdfs:label>
    </owl:NamedIndividual>
    


    <!-- https://purl.org/ffdr-ontology#FactoryAndIndustrial -->


    <owl:NamedIndividual rdf:about="https://purl.org/ffdr-ontology#FactoryAndIndustrial">
        <rdf:type rdf:resource="https://purl.org/ffdr-ontology#BuildingOccupancy"/>
        <rdfs:comment xml:lang="en">The &apos;FactoryAndIndustrial&apos; class represents factory and industrial occupancy, which includes, among others, the use of a building for: 
  - assembling, 
  - disassembling, 
  - fabricating, 
  - finishing, 
  - manufacturing, 
  - packaging, 
  - repair or 
  - processing 
operations that are not classified as hazardous or storage occupancy (IBC, 2018).</rdfs:comment>
        <rdfs:label xml:lang="en">FactoryAndIndustrial</rdfs:label>
    </owl:NamedIndividual>
    


    <!-- https://purl.org/ffdr-ontology#HighHazard -->


    <owl:NamedIndividual rdf:about="https://purl.org/ffdr-ontology#HighHazard">
        <rdf:type rdf:resource="https://purl.org/ffdr-ontology#BuildingOccupancy"/>
        <rdfs:comment xml:lang="en">The &apos;HighHazard&apos; class represents high-hazard occupancy, which includes, among others, the use of a building that involves the manufacturing, processing, generation, or storage of materials that constitute a physical or health hazard (IBC, 2018).</rdfs:comment>
        <rdfs:label xml:lang="en">HighHazard</rdfs:label>
    </owl:NamedIndividual>
    


    <!-- https://purl.org/ffdr-ontology#Institutional -->


    <owl:NamedIndividual rdf:about="https://purl.org/ffdr-ontology#Institutional">
        <rdf:type rdf:resource="https://purl.org/ffdr-ontology#BuildingOccupancy"/>
        <rdfs:comment xml:lang="en">The &apos;Institutional&apos; class represents institutional occupancy, which includes, among others, the use of a building where supervision is provided to people who may or may not need physical assistance for self-preservation. Additionally, it represents occupancies where the liberty of occupants is restricted (such as correction facilities) (IBC, 2018).</rdfs:comment>
        <rdfs:label xml:lang="en">Institutional</rdfs:label>
    </owl:NamedIndividual>
    


    <!-- https://purl.org/ffdr-ontology#Mercantile -->


    <owl:NamedIndividual rdf:about="https://purl.org/ffdr-ontology#Mercantile">
        <rdf:type rdf:resource="https://purl.org/ffdr-ontology#BuildingOccupancy"/>
        <rdfs:comment xml:lang="en">The &apos;Mercantile&apos; class represents mercantile occupancy, which includes, among others, the use of a building for the display and sale of merchandise (IBC, 2018).</rdfs:comment>
        <rdfs:label xml:lang="en">Mercantile</rdfs:label>
    </owl:NamedIndividual>
    


    <!-- https://purl.org/ffdr-ontology#Residential -->


    <owl:NamedIndividual rdf:about="https://purl.org/ffdr-ontology#Residential">
        <rdf:type rdf:resource="https://purl.org/ffdr-ontology#BuildingOccupancy"/>
        <rdfs:comment xml:lang="en">The &apos;Residential&apos; class represents residential occupancy, which includes, among others, the use of a building for sleeping purposes when not classified as an institutional (IBC, 2018).</rdfs:comment>
        <rdfs:label xml:lang="en">Residential</rdfs:label>
    </owl:NamedIndividual>
    


    <!-- https://purl.org/ffdr-ontology#Storage -->


    <owl:NamedIndividual rdf:about="https://purl.org/ffdr-ontology#Storage">
        <rdf:type rdf:resource="https://purl.org/ffdr-ontology#BuildingOccupancy"/>
        <rdfs:comment xml:lang="en">The &apos;Storage&apos; class represents storage occupancy, which includes, among others, the use of a building for storage that is not classified as a hazardous occupancy (IBC, 2018).</rdfs:comment>
        <rdfs:label xml:lang="en">Storage</rdfs:label>
    </owl:NamedIndividual>
    


    <!-- https://purl.org/ffdr-ontology#TypeI -->


    <owl:NamedIndividual rdf:about="https://purl.org/ffdr-ontology#TypeI">
        <rdf:type rdf:resource="https://purl.org/ffdr-ontology#ConstructionType"/>
        <hasDescription>Fire-resistive: types of construction in which the building elements are of noncombustible materials.</hasDescription>
        <hasType>Type I</hasType>
        <rdfs:label xml:lang="en">TypeI</rdfs:label>
    </owl:NamedIndividual>
    


    <!-- https://purl.org/ffdr-ontology#TypeII -->


    <owl:NamedIndividual rdf:about="https://purl.org/ffdr-ontology#TypeII">
        <rdf:type rdf:resource="https://purl.org/ffdr-ontology#ConstructionType"/>
        <hasDescription>Non-combustible: Walls, partitions, columns, floors, and roofs are noncombustible. However, they provide less fire resistance and do not withstand the effects or spreading of fire as well as Type I.</hasDescription>
        <hasType>Type II</hasType>
        <rdfs:label xml:lang="en">TypeII</rdfs:label>
    </owl:NamedIndividual>
    


    <!-- https://purl.org/ffdr-ontology#TypeIII -->


    <owl:NamedIndividual rdf:about="https://purl.org/ffdr-ontology#TypeIII">
        <rdf:type rdf:resource="https://purl.org/ffdr-ontology#ConstructionType"/>
        <hasDescription>Ordinary: construction is that type of construction in which the exterior walls are of noncombustible materials and the interior building elements are of any material.</hasDescription>
        <hasType>Type III</hasType>
        <rdfs:label xml:lang="en">TypeIII</rdfs:label>
    </owl:NamedIndividual>
    


    <!-- https://purl.org/ffdr-ontology#TypeIV -->


    <owl:NamedIndividual rdf:about="https://purl.org/ffdr-ontology#TypeIV">
        <rdf:type rdf:resource="https://purl.org/ffdr-ontology#ConstructionType"/>
        <hasDescription>(Heavy Timber: type of construction in which the exterior walls are of noncombustible materials and the interior building elements are of solid wood, laminated wood, heavy timber (HT) or structural composite lumber (SCL) without concealed spaces.</hasDescription>
        <hasType>Type IV</hasType>
        <rdfs:label xml:lang="en">TypeIV</rdfs:label>
    </owl:NamedIndividual>
    


    <!-- https://purl.org/ffdr-ontology#TypeV -->


    <owl:NamedIndividual rdf:about="https://purl.org/ffdr-ontology#TypeV">
        <rdf:type rdf:resource="https://purl.org/ffdr-ontology#ConstructionType"/>
        <hasDescription>Type of construction in which the structural elements, exterior walls and interior walls are of any materials.</hasDescription>
        <hasType>Type V</hasType>
        <rdfs:label xml:lang="en">TypeV</rdfs:label>
    </owl:NamedIndividual>
    


    <!-- https://purl.org/ffdr-ontology#UtilityAndMiscellaneous -->


    <owl:NamedIndividual rdf:about="https://purl.org/ffdr-ontology#UtilityAndMiscellaneous">
        <rdf:type rdf:resource="https://purl.org/ffdr-ontology#BuildingOccupancy"/>
        <rdfs:comment xml:lang="en">The &apos;Storage&apos; class represents storage occupancy, which includes, among others, the use of a building for storage that is not classified as a hazardous occupancy (IBC, 2018).</rdfs:comment>
        <rdfs:label xml:lang="en">UtilityAndMiscellaneous</rdfs:label>
    </owl:NamedIndividual>
    


    <!-- 
    ///////////////////////////////////////////////////////////////////////////////////////
    //
    // General axioms
    //
    ///////////////////////////////////////////////////////////////////////////////////////
     -->


    <rdf:Description>
        <rdf:type rdf:resource="http://www.w3.org/2002/07/owl#AllDisjointClasses"/>
        <owl:members rdf:parseType="Collection">
            <rdf:Description rdf:about="https://purl.org/ffdr-ontology#Address"/>
            <rdf:Description rdf:about="https://purl.org/ffdr-ontology#AirSupply"/>
            <rdf:Description rdf:about="https://purl.org/ffdr-ontology#BuildingComponent"/>
            <rdf:Description rdf:about="https://purl.org/ffdr-ontology#BuildingOccupancy"/>
            <rdf:Description rdf:about="https://purl.org/ffdr-ontology#BuildingPlan"/>
            <rdf:Description rdf:about="https://purl.org/ffdr-ontology#ConstructionType"/>
            <rdf:Description rdf:about="https://purl.org/ffdr-ontology#ControlPanel"/>
            <rdf:Description rdf:about="https://purl.org/ffdr-ontology#EmergencyServiceProvider"/>
            <rdf:Description rdf:about="https://purl.org/ffdr-ontology#FireCommandCenter"/>
            <rdf:Description rdf:about="https://purl.org/ffdr-ontology#HoseConnection"/>
            <rdf:Description rdf:about="https://purl.org/ffdr-ontology#IncidentBuilding"/>
            <rdf:Description rdf:about="https://purl.org/ffdr-ontology#IncidentSite"/>
            <rdf:Description rdf:about="https://purl.org/ffdr-ontology#Material"/>
            <rdf:Description rdf:about="https://purl.org/ffdr-ontology#RoadToIncident"/>
            <rdf:Description rdf:about="https://purl.org/ffdr-ontology#SurroundingStructure"/>
            <rdf:Description rdf:about="https://purl.org/ffdr-ontology#SurroundingTerrain"/>
            <rdf:Description rdf:about="https://purl.org/ffdr-ontology#WaterSource"/>
            <rdf:Description rdf:about="https://purl.org/ffdr-ontology#WeatherCondition"/>
        </owl:members>
    </rdf:Description>
    <rdf:Description>
        <rdf:type rdf:resource="http://www.w3.org/2002/07/owl#AllDisjointClasses"/>
        <owl:members rdf:parseType="Collection">
            <rdf:Description rdf:about="https://purl.org/ffdr-ontology#AlarmSystemAnnunciatorPanel"/>
            <rdf:Description rdf:about="https://purl.org/ffdr-ontology#DoorUnlockingSystemControlPanel"/>
            <rdf:Description rdf:about="https://purl.org/ffdr-ontology#ElevatorOverrideControlPanel"/>
            <rdf:Description rdf:about="https://purl.org/ffdr-ontology#FarsControlPanel"/>
            <rdf:Description rdf:about="https://purl.org/ffdr-ontology#FireDepartmentCommunicationSystemPanel"/>
            <rdf:Description rdf:about="https://purl.org/ffdr-ontology#MassNotificationSystemControlPanel"/>
            <rdf:Description rdf:about="https://purl.org/ffdr-ontology#SmokeControlSystemControlPanel"/>
            <rdf:Description rdf:about="https://purl.org/ffdr-ontology#UtilityControlPanel"/>
        </owl:members>
    </rdf:Description>
    <rdf:Description>
        <rdf:type rdf:resource="http://www.w3.org/2002/07/owl#AllDisjointClasses"/>
        <owl:members rdf:parseType="Collection">
            <rdf:Description rdf:about="https://purl.org/ffdr-ontology#AutomaticFireExtinguishingSystem"/>
            <rdf:Description rdf:about="https://purl.org/ffdr-ontology#EmergencyPowerOutlet"/>
            <rdf:Description rdf:about="https://purl.org/ffdr-ontology#FarsFillStation"/>
            <rdf:Description rdf:about="https://purl.org/ffdr-ontology#FireAlarmSystem"/>
            <rdf:Description rdf:about="https://purl.org/ffdr-ontology#FireDepartmentConnection"/>
            <rdf:Description rdf:about="https://purl.org/ffdr-ontology#FireHoseConnection"/>
            <rdf:Description rdf:about="https://purl.org/ffdr-ontology#FirePump"/>
            <rdf:Description rdf:about="https://purl.org/ffdr-ontology#FireandSmokeProtectionElement"/>
            <rdf:Description rdf:about="https://purl.org/ffdr-ontology#MassNotificationSystem"/>
            <rdf:Description rdf:about="https://purl.org/ffdr-ontology#PortableFireExtinguisher"/>
            <rdf:Description rdf:about="https://purl.org/ffdr-ontology#SensorDetector"/>
            <rdf:Description rdf:about="https://purl.org/ffdr-ontology#SmokeControlSystem"/>
            <rdf:Description rdf:about="https://purl.org/ffdr-ontology#SmokeandHeatRemovalSystem"/>
            <rdf:Description rdf:about="https://purl.org/ffdr-ontology#StandpipeSystem"/>
        </owl:members>
    </rdf:Description>
    <rdf:Description>
        <rdf:type rdf:resource="http://www.w3.org/2002/07/owl#AllDisjointClasses"/>
        <owl:members rdf:parseType="Collection">
            <rdf:Description rdf:about="https://purl.org/ffdr-ontology#BackUpPowerSupplySystem"/>
            <rdf:Description rdf:about="https://purl.org/ffdr-ontology#GasSupplySystem"/>
            <rdf:Description rdf:about="https://purl.org/ffdr-ontology#HvacSystem"/>
            <rdf:Description rdf:about="https://purl.org/ffdr-ontology#PrimaryPowerSupplySystem"/>
            <rdf:Description rdf:about="https://purl.org/ffdr-ontology#WaterSupplyandSewerageSystem"/>
        </owl:members>
    </rdf:Description>
    <rdf:Description>
        <rdf:type rdf:resource="http://www.w3.org/2002/07/owl#AllDisjointClasses"/>
        <owl:members rdf:parseType="Collection">
            <rdf:Description rdf:about="https://purl.org/ffdr-ontology#Building"/>
            <rdf:Description rdf:about="https://purl.org/ffdr-ontology#FireHydrant"/>
            <rdf:Description rdf:about="https://purl.org/ffdr-ontology#FireLane"/>
            <rdf:Description rdf:about="https://purl.org/ffdr-ontology#HazardousMaterial"/>
            <rdf:Description rdf:about="https://purl.org/ffdr-ontology#Obstruction"/>
            <rdf:Description rdf:about="https://purl.org/ffdr-ontology#ParkingLot"/>
            <rdf:Description rdf:about="https://purl.org/ffdr-ontology#Pipeline"/>
            <rdf:Description rdf:about="https://purl.org/ffdr-ontology#PowerLine"/>
            <rdf:Description rdf:about="https://purl.org/ffdr-ontology#Vegetation"/>
        </owl:members>
    </rdf:Description>
    <rdf:Description>
        <rdf:type rdf:resource="http://www.w3.org/2002/07/owl#AllDisjointClasses"/>
        <owl:members rdf:parseType="Collection">
            <rdf:Description rdf:about="https://purl.org/ffdr-ontology#BuildingAddress"/>
            <rdf:Description rdf:about="https://purl.org/ffdr-ontology#BuildingEngineerContactAddress"/>
            <rdf:Description rdf:about="https://purl.org/ffdr-ontology#BuildingManagerContactAddress"/>
            <rdf:Description rdf:about="https://purl.org/ffdr-ontology#EmergencyServiceProviderContactAddress"/>
            <rdf:Description rdf:about="https://purl.org/ffdr-ontology#OwnerContactAddress"/>
            <rdf:Description rdf:about="https://purl.org/ffdr-ontology#PublicSafetyAgencyContactAddress"/>
            <rdf:Description rdf:about="https://purl.org/ffdr-ontology#UtilityContactAddress"/>
        </owl:members>
    </rdf:Description>
    <rdf:Description>
        <rdf:type rdf:resource="http://www.w3.org/2002/07/owl#AllDisjointClasses"/>
        <owl:members rdf:parseType="Collection">
            <rdf:Description rdf:about="https://purl.org/ffdr-ontology#CarbonMonoxideDetector"/>
            <rdf:Description rdf:about="https://purl.org/ffdr-ontology#CbrSensor"/>
            <rdf:Description rdf:about="https://purl.org/ffdr-ontology#GasDetector"/>
        </owl:members>
    </rdf:Description>
    <rdf:Description>
        <rdf:type rdf:resource="http://www.w3.org/2002/07/owl#AllDisjointClasses"/>
        <owl:members rdf:parseType="Collection">
            <rdf:Description rdf:about="https://purl.org/ffdr-ontology#ExteriorDoor"/>
            <rdf:Description rdf:about="https://purl.org/ffdr-ontology#ExteriorWall"/>
            <rdf:Description rdf:about="https://purl.org/ffdr-ontology#ExteriorWindow"/>
            <rdf:Description rdf:about="https://purl.org/ffdr-ontology#Firewall"/>
        </owl:members>
    </rdf:Description>
    <rdf:Description>
        <rdf:type rdf:resource="http://www.w3.org/2002/07/owl#AllDisjointClasses"/>
        <owl:members rdf:parseType="Collection">
            <rdf:Description rdf:about="https://purl.org/ffdr-ontology#FireBarrier"/>
            <rdf:Description rdf:about="https://purl.org/ffdr-ontology#FirePartition"/>
            <rdf:Description rdf:about="https://purl.org/ffdr-ontology#Firewall"/>
            <rdf:Description rdf:about="https://purl.org/ffdr-ontology#ShaftEnclosure"/>
            <rdf:Description rdf:about="https://purl.org/ffdr-ontology#SmokeBarrier"/>
            <rdf:Description rdf:about="https://purl.org/ffdr-ontology#SmokePartition"/>
        </owl:members>
    </rdf:Description>
    <rdf:Description>
        <rdf:type rdf:resource="http://www.w3.org/2002/07/owl#AllDisjointClasses"/>
        <owl:members rdf:parseType="Collection">
            <rdf:Description rdf:about="https://purl.org/ffdr-ontology#FireServiceOrganization"/>
            <rdf:Description rdf:about="https://purl.org/ffdr-ontology#Hospital"/>
            <rdf:Description rdf:about="https://purl.org/ffdr-ontology#PoliceDepartment"/>
        </owl:members>
    </rdf:Description>
</rdf:RDF>



<!-- Generated by the OWL API (version 5.1.14) https://github.com/owlcs/owlapi/ -->


